@prefix dc: <http://purl.org/dc/elements/1.1/> .
@prefix foaf: <http://xmlns.com/foaf/0.1/> .
@prefix lrmer: <http://iflastandards.info/ns/lrm/lrmer> .
@prefix owl: <http://www.w3.org/2002/07/owl#> .
@prefix rdf: <http://www.w3.org/1999/02/22-rdf-syntax-ns#> .
@prefix rdfs: <http://www.w3.org/2000/01/rdf-schema#> .
@prefix reg: <http://metadataregistry.org/uri/profile/regap/> .
@prefix skos: <http://www.w3.org/2004/02/skos/core#> .
@prefix xml: <http://www.w3.org/XML/1998/namespace> .
@prefix xsd: <http://www.w3.org/2001/XMLSchema#> .

<http://iflastandards.info/ns/lrm/lrmerE10A1> a rdf:Property ;
    rdfs:label "has category of place"@en ;
    reg:lexicalAlias <http://iflastandards.info/ns/lrm/lrmerhasCategoryOfPlace> ;
    reg:name "hasCategoryOfPlace" ;
    reg:status <http://metadataregistry.org/uri/RegStatus/1001> ;
    rdfs:domain <http://iflastandards.info/ns/lrm/lrmerE10> ;
    rdfs:isDefinedBy lrmer: ;
    rdfs:subPropertyOf <http://iflastandards.info/ns/lrm/lrmerE1A1> ;
    skos:definition "Relates a place to a type to which the place belongs"@en .

<http://iflastandards.info/ns/lrm/lrmerE10A2> a rdf:Property ;
    rdfs:label "has location of place"@en ;
    reg:lexicalAlias <http://iflastandards.info/ns/lrm/lrmerhasLocationOfPlace> ;
    reg:name "hasLocationOfPlace" ;
    reg:status <http://metadataregistry.org/uri/RegStatus/1001> ;
    rdfs:comment "The level of precision used can vary according to the context."@en ;
    rdfs:domain <http://iflastandards.info/ns/lrm/lrmerE10> ;
    rdfs:isDefinedBy lrmer: ;
    skos:definition "Relates a place to a delimitation of the physical territory of the place"@en .

<http://iflastandards.info/ns/lrm/lrmerE11A1> a rdf:Property ;
    rdfs:label "has beginning"@en ;
    reg:lexicalAlias <http://iflastandards.info/ns/lrm/lrmerhasBeginning> ;
    reg:name "hasBeginning" ;
    reg:status <http://metadataregistry.org/uri/RegStatus/1001> ;
    rdfs:comment "The level of precision used can vary according to the context."@en ;
    rdfs:domain <http://iflastandards.info/ns/lrm/lrmerE11> ;
    rdfs:isDefinedBy lrmer: ;
    skos:definition "Relates a time-span to a value for the time at which the time-span started, expressed in a precise way in an authoritative external system to allow temporal positioning of events"@en .

<http://iflastandards.info/ns/lrm/lrmerE11A2> a rdf:Property ;
    rdfs:label "has ending"@en ;
    reg:lexicalAlias <http://iflastandards.info/ns/lrm/lrmerhasEnding> ;
    reg:name "hasEnding" ;
    reg:status <http://metadataregistry.org/uri/RegStatus/1001> ;
    rdfs:comment "The level of precision used can vary according to the context."@en ;
    rdfs:domain <http://iflastandards.info/ns/lrm/lrmerE11> ;
    rdfs:isDefinedBy lrmer: ;
    skos:definition "Relates a time-span to a value for the time at which the time-span ended, expressed in a precise way in an authoritative external system to allow temporal positioning of events"@en .

<http://iflastandards.info/ns/lrm/lrmerE1A2> a rdf:Property ;
    rdfs:label "has note"@en ;
    reg:lexicalAlias <http://iflastandards.info/ns/lrm/lrmerhasNote> ;
    reg:name "hasNote" ;
    reg:status <http://metadataregistry.org/uri/RegStatus/1001> ;
    rdfs:domain <http://iflastandards.info/ns/lrm/lrmerE1> ;
    rdfs:isDefinedBy lrmer: ;
    skos:definition "Relates a res to any kind of information about a res that is not recorded through the use of specific attributes and/or relationships"@en .

<http://iflastandards.info/ns/lrm/lrmerE2A1> a rdf:Property ;
    rdfs:label "has category of work"@en ;
    reg:lexicalAlias <http://iflastandards.info/ns/lrm/lrmerhasCategoryOfWork> ;
    reg:name "hasCategoryOfWork" ;
    reg:status <http://metadataregistry.org/uri/RegStatus/1001> ;
    rdfs:comment "The category attribute can characterize a given work with regard to various categorizations: - categorization as to termination intention, - categorization as to creative domain, - categorization as to form / genre, - etc."@en ;
    rdfs:domain <http://iflastandards.info/ns/lrm/lrmerE2> ;
    rdfs:isDefinedBy lrmer: ;
    rdfs:subPropertyOf <http://iflastandards.info/ns/lrm/lrmerE1A1> ;
    skos:definition "Relates a work to a type to which the work belongs"@en .

<http://iflastandards.info/ns/lrm/lrmerE2A2> a rdf:Property ;
    rdfs:label "has representative expression attribute"@en ;
    reg:lexicalAlias <http://iflastandards.info/ns/lrm/lrmerhasRepresentativeExpressionAttribute> ;
    reg:name "hasRepresentativeExpressionAttribute" ;
    reg:status <http://metadataregistry.org/uri/RegStatus/1001> ;
    rdfs:comment "Generally, the representative expression attribute will be typed and the types chosen will vary depending on the context of use (as given by the cataloguing rules, the nature of catalogue, or the category of work). Each of the attributes chosen may itself be multivalued. The values of these attributes are inferred either from particular expressions considered to best represent the work, or from characteristics abstracted from a more or less nebulous network of similar expressions. There is no requirement to precisely identify an expression or expressions which serves as source for the values of the representative expression attributes, nor does that expression need to be recorded in the case where it is identified."@en ;
    rdfs:domain <http://iflastandards.info/ns/lrm/lrmerE2> ;
    rdfs:isDefinedBy lrmer: ;
    skos:definition "Relates a work to an attribute which is deemed essential in characterizing the work and whose values are taken from a representative or canonical expression of the work"@en .

<http://iflastandards.info/ns/lrm/lrmerE3A1> a rdf:Property ;
    rdfs:label "has category of expression"@en ;
    reg:lexicalAlias <http://iflastandards.info/ns/lrm/lrmerhasCategoryOfExpression> ;
    reg:name "hasCategoryOfExpression" ;
    reg:status <http://metadataregistry.org/uri/RegStatus/1001> ;
    rdfs:comment "The category attribute can characterize a given expression with regard to various categorizations: - content type, - state of development, - format of notated music, - etc."@en ;
    rdfs:domain <http://iflastandards.info/ns/lrm/lrmerE3> ;
    rdfs:isDefinedBy lrmer: ;
    rdfs:subPropertyOf <http://iflastandards.info/ns/lrm/lrmerE1A1> ;
    skos:definition "Relates an expression to a type to which the expression belongs"@en .

<http://iflastandards.info/ns/lrm/lrmerE3A2> a rdf:Property ;
    rdfs:label "has extent of expression"@en ;
    reg:lexicalAlias <http://iflastandards.info/ns/lrm/lrmerhasExtentOfExpression> ;
    reg:name "hasExtentOfExpression" ;
    reg:status <http://metadataregistry.org/uri/RegStatus/1001> ;
    rdfs:comment "The value of the extent attribute consists of three elements: - a type of extent (e.g., length of text, envisioned duration of performance of musical notation, actual duration of recorded performance, etc.), - a number, - and a measurement unit (words, minutes, etc.). The type of extent and the measurement unit may be given implicitly. The level of precision used in recording the quantification of the extent may vary."@en ;
    rdfs:domain <http://iflastandards.info/ns/lrm/lrmerE3> ;
    rdfs:isDefinedBy lrmer: ;
    skos:definition "Relates an expression to a quantification of the extent of the expression"@en .

<http://iflastandards.info/ns/lrm/lrmerE3A3> a rdf:Property ;
    rdfs:label "has intended audience of expression"@en ;
    reg:lexicalAlias <http://iflastandards.info/ns/lrm/lrmerhasIntendedAudienceOfExpression> ;
    reg:name "hasIntendedAudienceOfExpression" ;
    reg:status <http://metadataregistry.org/uri/RegStatus/1001> ;
    rdfs:comment "The intended audience attribute can characterize a given expression by indicating groups of end-users for which expressions with those features are deemed particularly appropriate: - categorization as to age group, - categorization as to sensory impairment, - categorization as to educational level, - categorization as to occupational group, - etc."@en ;
    rdfs:domain <http://iflastandards.info/ns/lrm/lrmerE3> ;
    rdfs:isDefinedBy lrmer: ;
    skos:definition "Relates an expression to a class of users for which the expression is intended"@en .

<http://iflastandards.info/ns/lrm/lrmerE3A4> a rdf:Property ;
    rdfs:label "has use rights of the expression"@en ;
    reg:lexicalAlias <http://iflastandards.info/ns/lrm/lrmerhasUseRightsOfTheExpression> ;
    reg:name "hasUseRightsOfTheExpression" ;
    reg:status <http://metadataregistry.org/uri/RegStatus/1001> ;
    rdfs:domain <http://iflastandards.info/ns/lrm/lrmerE3> ;
    rdfs:isDefinedBy lrmer: ;
    skos:definition "Relates an expression to a class of use restrictions to which the expression is submitted"@en .

<http://iflastandards.info/ns/lrm/lrmerE3A5> a rdf:Property ;
    rdfs:label "has cartographic scale"@en ;
    reg:lexicalAlias <http://iflastandards.info/ns/lrm/lrmerhasCartographicScale> ;
    reg:name "hasCartographicScale" ;
    reg:status <http://metadataregistry.org/uri/RegStatus/1001> ;
    rdfs:comment "The cartographic scale attribute is specific to expressions of cartographic works. The cartographic scale attribute may apply to horizontal, vertical, angular, and/or other distances represented in the expression."@en ;
    rdfs:domain <http://iflastandards.info/ns/lrm/lrmerE3> ;
    rdfs:isDefinedBy lrmer: ;
    skos:definition "Relates an expression to a ratio of distances in a cartographic expression to the actual distances they represent"@en .

<http://iflastandards.info/ns/lrm/lrmerE3A6> a rdf:Property ;
    rdfs:label "has language of expression"@en ;
    reg:lexicalAlias <http://iflastandards.info/ns/lrm/lrmerhasLanguageOfExpression> ;
    reg:name "hasLanguageOfExpression" ;
    reg:status <http://metadataregistry.org/uri/RegStatus/1001> ;
    rdfs:comment "The language attribute is specific to expressions consisting solely or partially of linguistic signs (either sonic or in notated form). The language attribute of the expression may include a number of languages, each pertaining to an individual component of the expression."@en ;
    rdfs:domain <http://iflastandards.info/ns/lrm/lrmerE3> ;
    rdfs:isDefinedBy lrmer: ;
    skos:definition "Relates an expression to a language used in the expression"@en .

<http://iflastandards.info/ns/lrm/lrmerE3A7> a rdf:Property ;
    rdfs:label "has key"@en ;
    reg:lexicalAlias <http://iflastandards.info/ns/lrm/lrmerhasKey> ;
    reg:name "hasKey" ;
    reg:status <http://metadataregistry.org/uri/RegStatus/1001> ;
    rdfs:comment "The key attribute is specific to expressions of musical works. The term “key” is broadly defined to encompass various musical traditions. This attribute is not restricted to Western art music."@en ;
    rdfs:domain <http://iflastandards.info/ns/lrm/lrmerE3> ;
    rdfs:isDefinedBy lrmer: ;
    skos:definition "Relates an expression to a pitch structure (musical scale, ecclesiastic mode, raga, maqam, etc.), that characterizes the expression"@en .

<http://iflastandards.info/ns/lrm/lrmerE3A8> a rdf:Property ;
    rdfs:label "has medium of performance"@en ;
    reg:lexicalAlias <http://iflastandards.info/ns/lrm/lrmerhasMediumOfPerformance> ;
    reg:name "hasMediumOfPerformance" ;
    reg:status <http://metadataregistry.org/uri/RegStatus/1001> ;
    rdfs:comment "The medium of performance attribute is specific to expressions of musical works. The value of the medium of performance attribute includes at least one unit consisting of: - a number (implicit through the use of a singular noun, or explicitly stated), - and a type of performing tool (which may include: types of human voice tessitura, types of individual instruments, types of ensembles, etc.)."@en ;
    rdfs:domain <http://iflastandards.info/ns/lrm/lrmerE3> ;
    rdfs:isDefinedBy lrmer: ;
    skos:definition "Relates an expression to a combination of performing tools (voices, instruments, ensembles, etc.) stated, intended, or actually used in the expression"@en .

<http://iflastandards.info/ns/lrm/lrmerE4A1> a rdf:Property ;
    rdfs:label "has category of carrier"@en ;
    reg:lexicalAlias <http://iflastandards.info/ns/lrm/lrmerhasCategoryOfCarrier> ;
    reg:name "hasCategoryOfCarrier" ;
    reg:status <http://metadataregistry.org/uri/RegStatus/1001> ;
    rdfs:comment "The category of carrier attribute can characterize a given manifestation with regard to various categorizations: - categorization as to general type of carrier (e.g., sheet), - categorization as to physical material employed in manufacturing the carriers (e.g., plastic), - categorization as to the physical material that is applied to the base material of the carriers (e.g., oil paint), - categorization as to the means used to record notation, sound, or images in the production of a manifestation (e.g., analogue), - etc. The carrier for a manifestation consisting of multiple physical components may include more than one form (e.g., a filmstrip with an accompanying booklet, a separate sound disc carrying the sound track for a film, etc.)."@en ;
    rdfs:domain <http://iflastandards.info/ns/lrm/lrmerE4> ;
    rdfs:isDefinedBy lrmer: ;
    rdfs:subPropertyOf <http://iflastandards.info/ns/lrm/lrmerE1A1> ;
    skos:definition "Relates a manifestation to a type of material to which all physical carriers of the manifestation are assumed to belong"@en .

<http://iflastandards.info/ns/lrm/lrmerE4A2> a rdf:Property ;
    rdfs:label "has extent of manifestation"@en ;
    reg:lexicalAlias <http://iflastandards.info/ns/lrm/lrmerhasExtentOfManifestation> ;
    reg:name "hasExtentOfManifestation" ;
    reg:status <http://metadataregistry.org/uri/RegStatus/1001> ;
    rdfs:comment "The value of the extent attribute consists of three elements: - a type of extent (e.g., numbering of physical units, height, width, diameter, etc.), - a number, - and a measurement unit (e.g., volumes, pages, sheets, discs, reels, etc.; cm, inches, etc.; Mb/Megabytes; etc.). The type of extent and the measurement unit may be given implicitly. The level of precision used in recording the quantification of the extent may vary."@en ;
    rdfs:domain <http://iflastandards.info/ns/lrm/lrmerE4> ;
    rdfs:isDefinedBy lrmer: ;
    skos:definition "Relates a manifestation to a quantification of the extent observed on a physical carrier of the manifestation and assumed to be observable on all other physical carriers of the manifestation as well"@en .

<http://iflastandards.info/ns/lrm/lrmerE4A3> a rdf:Property ;
    rdfs:label "has intended audience of manifestation"@en ;
    reg:lexicalAlias <http://iflastandards.info/ns/lrm/lrmerhasIntendedAudienceOfManifestation> ;
    reg:name "hasIntendedAudienceOfManifestation" ;
    reg:status <http://metadataregistry.org/uri/RegStatus/1001> ;
    rdfs:comment "The intended audience attribute can characterize a given manifestation by indicating groups of end-users for which manifestations with those features are deemed particularly appropriate: - categorization as to sensory impairment (visual impairment, hearing impairment, etc.), - categorization as to specialized carriers for specific audiences (young children, etc.), - etc."@en ;
    rdfs:domain <http://iflastandards.info/ns/lrm/lrmerE4> ;
    rdfs:isDefinedBy lrmer: ;
    skos:definition "Relates a manifestation to a class of users for which the physical carriers of the manifestation are intended"@en .

<http://iflastandards.info/ns/lrm/lrmerE4A4> a rdf:Property ;
    rdfs:label "has manifestation statement"@en ;
    reg:lexicalAlias <http://iflastandards.info/ns/lrm/lrmerhasManifestationStatement> ;
    reg:name "hasManifestationStatement" ;
    reg:status <http://metadataregistry.org/uri/RegStatus/1001> ;
    rdfs:comment "The manifestation statement attribute is a statement that is usually transcribed from a source or sources present in exemplars of a manifestation. Transcription conventions are codified by each implementation. A manifestation is likely to be characterized by multiple statements of different types. In most implementations, these statements would likely be typed at a level of granularity considered appropriate for user needs. For example, the manifestation statement attribute may include transcribed elements such as: publication statement (as a whole), or alternatively, place of publication statement + publisher name statement + date of publication statement (as three individual statements)."@en ;
    rdfs:domain <http://iflastandards.info/ns/lrm/lrmerE4> ;
    rdfs:isDefinedBy lrmer: ;
    skos:definition "Relates a manifestation to a statement appearing in exemplars of the manifestation and deemed to be significant for users to understand how the resource represents itself"@en .

<http://iflastandards.info/ns/lrm/lrmerE4A5> a rdf:Property ;
    rdfs:label "has access conditions"@en ;
    reg:lexicalAlias <http://iflastandards.info/ns/lrm/lrmerhasAccessConditions> ;
    reg:name "hasAccessConditions" ;
    reg:status <http://metadataregistry.org/uri/RegStatus/1001> ;
    rdfs:comment "The access conditions attribute includes: - System requirements, - Mode of access, - etc."@en ;
    rdfs:domain <http://iflastandards.info/ns/lrm/lrmerE4> ;
    rdfs:isDefinedBy lrmer: ;
    skos:definition "Relates a manifestation to information as to how any of the carriers of the manifestation are likely to be obtained"@en .

<http://iflastandards.info/ns/lrm/lrmerE4A6> a rdf:Property ;
    rdfs:label "has use rights of the manifestation"@en ;
    reg:lexicalAlias <http://iflastandards.info/ns/lrm/lrmerhasUseRightsOfTheManifestation> ;
    reg:name "hasUseRightsOfTheManifestation" ;
    reg:status <http://metadataregistry.org/uri/RegStatus/1001> ;
    rdfs:comment "The use rights attribute includes: - Terms of availability, - Access restrictions, - etc."@en ;
    rdfs:domain <http://iflastandards.info/ns/lrm/lrmerE4> ;
    rdfs:isDefinedBy lrmer: ;
    skos:definition "Relates a manifestation to a class of use and/or access restrictions to which all carriers of the manifestation are assumed to be submitted"@en .

<http://iflastandards.info/ns/lrm/lrmerE5A1> a rdf:Property ;
    rdfs:label "has location of item"@en ;
    reg:lexicalAlias <http://iflastandards.info/ns/lrm/lrmerhasLocationOfItem> ;
    reg:name "hasLocationOfItem" ;
    reg:status <http://metadataregistry.org/uri/RegStatus/1001> ;
    rdfs:comment "This information can be specified at whatever level of precision is required in order to guide end-users in obtaining the item."@en ;
    rdfs:domain <http://iflastandards.info/ns/lrm/lrmerE5> ;
    rdfs:isDefinedBy lrmer: ;
    skos:definition "Relates an item to the collection and/or institution in which the item is held, stored, or made available for access"@en .

<http://iflastandards.info/ns/lrm/lrmerE5A2> a rdf:Property ;
    rdfs:label "has use rights of the item"@en ;
    reg:lexicalAlias <http://iflastandards.info/ns/lrm/lrmerhasUseRightsOfTheItem> ;
    reg:name "hasUseRightsOfTheItem" ;
    reg:status <http://metadataregistry.org/uri/RegStatus/1001> ;
    rdfs:domain <http://iflastandards.info/ns/lrm/lrmerE5> ;
    rdfs:isDefinedBy lrmer: ;
    skos:definition "Relates an item to a class of use and/or access restrictions to which the item is submitted"@en .

<http://iflastandards.info/ns/lrm/lrmerE6A1> a rdf:Property ;
    rdfs:label "has contact information"@en ;
    reg:lexicalAlias <http://iflastandards.info/ns/lrm/lrmerhasContactInformation> ;
    reg:name "hasContactInformation" ;
    reg:status <http://metadataregistry.org/uri/RegStatus/1001> ;
    rdfs:domain <http://iflastandards.info/ns/lrm/lrmerE6> ;
    rdfs:isDefinedBy lrmer: ;
    skos:definition "Relates an agent to information useful for communicating with or getting in contact with the agent"@en .

<http://iflastandards.info/ns/lrm/lrmerE6A2> a rdf:Property ;
    rdfs:label "has field of activity"@en ;
    reg:lexicalAlias <http://iflastandards.info/ns/lrm/lrmerhasFieldOfActivity> ;
    reg:name "hasFieldOfActivity" ;
    reg:status <http://metadataregistry.org/uri/RegStatus/1001> ;
    rdfs:domain <http://iflastandards.info/ns/lrm/lrmerE6> ;
    rdfs:isDefinedBy lrmer: ;
    skos:definition "Relates an agent to a field of endeavour, area of expertise, etc., in which the agent is engaged or was engaged"@en .

<http://iflastandards.info/ns/lrm/lrmerE6A3> a rdf:Property ;
    rdfs:label "has language of agent"@en ;
    reg:lexicalAlias <http://iflastandards.info/ns/lrm/lrmerhasLanguageOfAgent> ;
    reg:name "hasLanguageOfAgent" ;
    reg:status <http://metadataregistry.org/uri/RegStatus/1001> ;
    rdfs:comment "A given agent can use more than one language, simultaneously or over time. The type of use of a given language can be specified (e.g., use of the English language for the creation of original content, use of the English language as source language of translations, etc.)."@en ;
    rdfs:domain <http://iflastandards.info/ns/lrm/lrmerE6> ;
    rdfs:isDefinedBy lrmer: ;
    skos:definition "Relates an agent to a language used by the agent when creating an expression"@en .

<http://iflastandards.info/ns/lrm/lrmerE7A1> a rdf:Property ;
    rdfs:label "has profession or occupation"@en ;
    reg:lexicalAlias <http://iflastandards.info/ns/lrm/lrmerhasProfessionOrOccupation> ;
    reg:name "hasProfessionOrOccupation" ;
    reg:status <http://metadataregistry.org/uri/RegStatus/1001> ;
    rdfs:domain <http://iflastandards.info/ns/lrm/lrmerE7> ;
    rdfs:isDefinedBy lrmer: ;
    skos:definition "Relates a person to a profession or occupation in which the person works or worked"@en ;
    skos:scopeNote "Source documentation has \"profession / occupation\"; slash character replaced with \"or\" to improve clarity."@en .

<http://iflastandards.info/ns/lrm/lrmerE9A1> a rdf:Property ;
    rdfs:label "has category of nomen"@en ;
    reg:lexicalAlias <http://iflastandards.info/ns/lrm/lrmerhasCategoryOfNomen> ;
    reg:name "hasCategoryOfNomen" ;
    reg:status <http://metadataregistry.org/uri/RegStatus/1001> ;
    rdfs:comment "Nomens may be categorized in terms of: - the type of thing named (personal name, work title, etc.), - the source in which the nomen is attested (spine title, running title), - the function of the nomen (identifier, controlled access point, classification notation, etc.)."@en ;
    rdfs:domain <http://iflastandards.info/ns/lrm/lrmerE9> ;
    rdfs:isDefinedBy lrmer: ;
    rdfs:subPropertyOf <http://iflastandards.info/ns/lrm/lrmerE1A1> ;
    skos:definition "Relates a nomen to a type to which the nomen belongs"@en .

<http://iflastandards.info/ns/lrm/lrmerE9A2> a rdf:Property ;
    rdfs:label "has nomen string"@en ;
    reg:lexicalAlias <http://iflastandards.info/ns/lrm/lrmerhasNomenString> ;
    reg:name "hasNomenString" ;
    reg:status <http://metadataregistry.org/uri/RegStatus/1001> ;
    rdfs:comment "The string involved in a nomen can be expressed as a notation in any form, such as a combination of signs within a writing system, chemical structure symbols, mathematical notation, or by any other kind of sign, such as sounds, etc. A nomen is more than the mere string of signs that constitutes the appellation associated with a thing through the nomen. Without any contextualization, the value of the nomen string attribute is a mere literal, potentially attached to anything in the world, as opposed to the nomen itself, which as a result of the appellation relationship is attached to one and only one instance of res. For example, the nomen 'John Smith' is the appellation of one and only one John Smith in the world, while the value of the nomen string attribute that reads \"John Smith\" in the Latin alphabet is the same for all the different things in the world that happen to be named 'John Smith'."@en ;
    rdfs:domain <http://iflastandards.info/ns/lrm/lrmerE9> ;
    rdfs:isDefinedBy lrmer: ;
    skos:definition "Relates a nomen to the combination of signs that forms an appellation associated with an entity through the nomen"@en .

<http://iflastandards.info/ns/lrm/lrmerE9A3> a rdf:Property ;
    rdfs:label "has scheme"@en ;
    reg:lexicalAlias <http://iflastandards.info/ns/lrm/lrmerhasScheme> ;
    reg:name "hasScheme" ;
    reg:status <http://metadataregistry.org/uri/RegStatus/1001> ;
    rdfs:comment "The scheme attribute includes: - value encoding schemes (subject heading lists, thesauri, classification systems, name authority lists, etc.) - and syntax encoding schemes (standards for encoding dates, etc.). When the same value of one of the other nomen attributes (such as intended audience, language, script) is applicable to all the nomens in a particular scheme, the value can be implemented at the scheme level."@en ;
    rdfs:domain <http://iflastandards.info/ns/lrm/lrmerE9> ;
    rdfs:isDefinedBy lrmer: ;
    skos:definition "Relates a nomen to the scheme in which the nomen is established"@en .

<http://iflastandards.info/ns/lrm/lrmerE9A4> a rdf:Property ;
    rdfs:label "has intended audience of nomen"@en ;
    reg:lexicalAlias <http://iflastandards.info/ns/lrm/lrmerhasIntendedAudienceOfNomen> ;
    reg:name "hasIntendedAudienceOfNomen" ;
    reg:status <http://metadataregistry.org/uri/RegStatus/1001> ;
    rdfs:comment "Indicating the intended audience for a nomen can serve as a basis for a mechanism that selects a nomen from a cluster of equivalent nomens, for use in a particular context. For example, an international multi-lingual authority file can indicate the intended audience for each nomen by recording the language in which the nomen is a preferred form."@en ;
    rdfs:domain <http://iflastandards.info/ns/lrm/lrmerE9> ;
    rdfs:isDefinedBy lrmer: ;
    skos:definition "Relates a nomen to a class of users for which the nomen is considered appropriate or preferred"@en .

<http://iflastandards.info/ns/lrm/lrmerE9A5> a rdf:Property ;
    rdfs:label "has context of use"@en ;
    reg:lexicalAlias <http://iflastandards.info/ns/lrm/lrmerhasContextOfUse> ;
    reg:name "hasContextOfUse" ;
    reg:status <http://metadataregistry.org/uri/RegStatus/1001> ;
    rdfs:comment "The context of use attribute includes domains associated with a nomen used by an agent."@en ;
    rdfs:domain <http://iflastandards.info/ns/lrm/lrmerE9> ;
    rdfs:isDefinedBy lrmer: ;
    skos:definition "Relates a nomen to information as to the context(s) in which a nomen is used by the agent who is referred to through it"@en .

<http://iflastandards.info/ns/lrm/lrmerE9A6> a rdf:Property ;
    rdfs:label "has reference source"@en ;
    reg:lexicalAlias <http://iflastandards.info/ns/lrm/lrmerhasReferenceSource> ;
    reg:name "hasReferenceSource" ;
    reg:status <http://metadataregistry.org/uri/RegStatus/1001> ;
    rdfs:comment "A reference source attests to the existence of a linkage between a designation and the instance of the entity res that it serves to identify. It may clarify the validity and scope of the nomen. A reference source attribute value may refer to: - biographical dictionaries, encyclopedias, etc., - other schemes, - any publications, - etc."@en ;
    rdfs:domain <http://iflastandards.info/ns/lrm/lrmerE9> ;
    rdfs:isDefinedBy lrmer: ;
    skos:definition "Relates a nomen to a source in which there is evidence for the use of the nomen"@en .

<http://iflastandards.info/ns/lrm/lrmerE9A7> a rdf:Property ;
    rdfs:label "has language of nomen"@en ;
    reg:lexicalAlias <http://iflastandards.info/ns/lrm/lrmerhasLanguageOfNomen> ;
    reg:name "hasLanguageOfNomen" ;
    reg:status <http://metadataregistry.org/uri/RegStatus/1001> ;
    rdfs:comment "The language attribute may be viewed as recording a scheme of a particular type (that is, a natural human language) in which a nomen may be considered valid. Viewed in this way, the language attribute may be implemented as a sub-type of the scheme attribute."@en ;
    rdfs:domain <http://iflastandards.info/ns/lrm/lrmerE9> ;
    rdfs:isDefinedBy lrmer: ;
    skos:definition "Relates a nomen to the language in which the nomen is attested"@en .

<http://iflastandards.info/ns/lrm/lrmerE9A8> a rdf:Property ;
    rdfs:label "has script"@en ;
    reg:lexicalAlias <http://iflastandards.info/ns/lrm/lrmerhasScript> ;
    reg:name "hasScript" ;
    reg:status <http://metadataregistry.org/uri/RegStatus/1001> ;
    rdfs:comment "The script attribute allows the identification of the writing system used to provide a notation for the nomen. The writing system consists of the full range of the conventions used. Writing systems may be alphabetic, syllabic, ideographic, etc., or some combination of these. The script does not, however, include aspects such as the choice of font or other incidental display characteristics (for example, point size, colour) which do not encode any features which result in differences in the interpretation of the written symbols."@en ;
    rdfs:domain <http://iflastandards.info/ns/lrm/lrmerE9> ;
    rdfs:isDefinedBy lrmer: ;
    skos:definition "Relates a nomen to the script in which the nomen is notated"@en .

<http://iflastandards.info/ns/lrm/lrmerE9A9> a rdf:Property ;
    rdfs:label "has script conversion"@en ;
    reg:lexicalAlias <http://iflastandards.info/ns/lrm/lrmerhasScriptConversion> ;
    reg:name "hasScriptConversion" ;
    reg:status <http://metadataregistry.org/uri/RegStatus/1001> ;
    rdfs:comment "A script conversion attribute value may refer to: - transliterations, - script conversions that cannot be reversed, - etc."@en ;
    rdfs:domain <http://iflastandards.info/ns/lrm/lrmerE9> ;
    rdfs:isDefinedBy lrmer: ;
    skos:definition "Relates a nomen to the rule, system, or standard that was used to create a nomen that is derived on the basis of another, distinct nomen notated in another, distinct script"@en .

<http://iflastandards.info/ns/lrm/lrmerR15> a rdf:Property ;
    rdfs:label "is equivalent to"@en ;
    reg:lexicalAlias <http://iflastandards.info/ns/lrm/lrmerisEquivalentTo> ;
    reg:name "isEquivalentTo" ;
    reg:status <http://metadataregistry.org/uri/RegStatus/1001> ;
    rdfs:comment "This is a shortcut of a fully developed path: NOMEN1 is appellation of RES + RES has appellation NOMEN2. The nomens related by this relationship are functionally equivalent in meaning (assigned to the same res), but as they retain their own values in any attributes that are recorded for them, they are not interchangeable as far as usage is concerned. The equivalent nomens may differ as to crucial attributes such as scheme, language or context of use. This equivalence relationship relates instances of nomens, and not the values of the nomen string attributes for these nomens. Thus, even though it may seem counter-intuitive, two nomens that refer to different res, even if recorded with the same literal string, will not be equivalent."@en ;
    rdfs:domain <http://iflastandards.info/ns/lrm/lrmerE9> ;
    rdfs:isDefinedBy lrmer: ;
    rdfs:range <http://iflastandards.info/ns/lrm/lrmerE9> ;
    rdfs:subPropertyOf <http://iflastandards.info/ns/lrm/lrmerR1> ;
    skos:definition "Relates two nomens which are appellations of the same res"@en .

<http://iflastandards.info/ns/lrm/lrmerR29> a rdf:Property ;
    rdfs:label "has alternate"@en ;
    reg:lexicalAlias <http://iflastandards.info/ns/lrm/lrmerhasAlternate> ;
    reg:name "hasAlternate" ;
    reg:status <http://metadataregistry.org/uri/RegStatus/1001> ;
    rdfs:comment "Typical cases are when a publication, sound recording, video, etc., is issued in more than one format or when it is released simultaneously by different publishers in different countries."@en ;
    rdfs:domain <http://iflastandards.info/ns/lrm/lrmerE4> ;
    rdfs:isDefinedBy lrmer: ;
    rdfs:range <http://iflastandards.info/ns/lrm/lrmerE4> ;
    rdfs:subPropertyOf <http://iflastandards.info/ns/lrm/lrmerR1> ;
    skos:definition "Relates manifestations that effectively serve as alternatives for each other"@en .

<http://iflastandards.info/ns/lrm/lrmerR10> a rdf:Property ;
    rdfs:label "is owned by"@en ;
    reg:lexicalAlias <http://iflastandards.info/ns/lrm/lrmerisOwnedBy> ;
    reg:name "isOwnedBy" ;
    reg:status <http://metadataregistry.org/uri/RegStatus/1001> ;
    rdfs:comment "The logical connection between an item and a related agent could serve as the basis both for identifying an agent that owned or had custodianship of an item and for ensuring that all items owned by, or in the custodianship of, a particular agent are linked to that agent."@en ;
    rdfs:domain <http://iflastandards.info/ns/lrm/lrmerE5> ;
    rdfs:isDefinedBy lrmer: ;
    rdfs:range <http://iflastandards.info/ns/lrm/lrmerE6> ;
    rdfs:subPropertyOf <http://iflastandards.info/ns/lrm/lrmerR1> ;
    owl:inverseOf <http://iflastandards.info/ns/lrm/lrmerR10i> ;
    skos:definition "Relates an item to an agent that is or was the owner or custodian of that item"@en .

<http://iflastandards.info/ns/lrm/lrmerR10i> a rdf:Property ;
    rdfs:label "owns"@en ;
    reg:lexicalAlias <http://iflastandards.info/ns/lrm/lrmerowns> ;
    reg:name "owns" ;
    reg:status <http://metadataregistry.org/uri/RegStatus/1001> ;
    rdfs:comment "The logical connection between an item and a related agent could serve as the basis both for identifying an agent that owned or had custodianship of an item and for ensuring that all items owned by, or in the custodianship of, a particular agent are linked to that agent."@en ;
    rdfs:domain <http://iflastandards.info/ns/lrm/lrmerE6> ;
    rdfs:isDefinedBy lrmer: ;
    rdfs:range <http://iflastandards.info/ns/lrm/lrmerE5> ;
    rdfs:subPropertyOf <http://iflastandards.info/ns/lrm/lrmerR1> ;
    owl:inverseOf <http://iflastandards.info/ns/lrm/lrmerR10> ;
    skos:definition "Relates an agent to an item that is or was owned or in the custody of that agent"@en .

<http://iflastandards.info/ns/lrm/lrmerR11> a rdf:Property ;
    rdfs:label "was modified by"@en ;
    reg:lexicalAlias <http://iflastandards.info/ns/lrm/lrmerwasModifiedBy> ;
    reg:name "wasModifiedBy" ;
    reg:status <http://metadataregistry.org/uri/RegStatus/1001> ;
    rdfs:comment "Examples include adding annotations, adding an ex-libris, removing pages, rebinding, restoration."@en ;
    rdfs:domain <http://iflastandards.info/ns/lrm/lrmerE5> ;
    rdfs:isDefinedBy lrmer: ;
    rdfs:range <http://iflastandards.info/ns/lrm/lrmerE6> ;
    rdfs:subPropertyOf <http://iflastandards.info/ns/lrm/lrmerR1> ;
    owl:inverseOf <http://iflastandards.info/ns/lrm/lrmerR11i> ;
    skos:definition "Relates an item to an agent that made changes to this particular item without creating a new manifestation"@en .

<http://iflastandards.info/ns/lrm/lrmerR11i> a rdf:Property ;
    rdfs:label "modified"@en ;
    reg:lexicalAlias <http://iflastandards.info/ns/lrm/lrmermodified> ;
    reg:name "modified" ;
    reg:status <http://metadataregistry.org/uri/RegStatus/1001> ;
    rdfs:comment "Examples include adding annotations, adding an ex-libris, removing pages, rebinding, restoration."@en ;
    rdfs:domain <http://iflastandards.info/ns/lrm/lrmerE6> ;
    rdfs:isDefinedBy lrmer: ;
    rdfs:range <http://iflastandards.info/ns/lrm/lrmerE5> ;
    rdfs:subPropertyOf <http://iflastandards.info/ns/lrm/lrmerR1> ;
    owl:inverseOf <http://iflastandards.info/ns/lrm/lrmerR11> ;
    skos:definition "Relates an agent to an item that the agent made changes to without creating a new manifestation"@en .

<http://iflastandards.info/ns/lrm/lrmerR12> a rdf:Property ;
    rdfs:label "has as subject"@en ;
    reg:lexicalAlias <http://iflastandards.info/ns/lrm/lrmerhasAsSubject> ;
    reg:name "hasAsSubject" ;
    reg:status <http://metadataregistry.org/uri/RegStatus/1001> ;
    rdfs:comment "The logical connection between a work and a related subject entity serves as the basis both for identifying the subject of an individual work and for ensuring that all works relevant to a given subject are linked to that subject."@en ;
    rdfs:domain <http://iflastandards.info/ns/lrm/lrmerE2> ;
    rdfs:isDefinedBy lrmer: ;
    rdfs:range <http://iflastandards.info/ns/lrm/lrmerE1> ;
    rdfs:subPropertyOf <http://iflastandards.info/ns/lrm/lrmerR1> ;
    owl:inverseOf <http://iflastandards.info/ns/lrm/lrmerR12i> ;
    skos:definition "Relates a work to its topic(s)"@en .

<http://iflastandards.info/ns/lrm/lrmerR12i> a rdf:Property ;
    rdfs:label "is subject of"@en ;
    reg:lexicalAlias <http://iflastandards.info/ns/lrm/lrmerisSubjectOf> ;
    reg:name "isSubjectOf" ;
    reg:status <http://metadataregistry.org/uri/RegStatus/1001> ;
    rdfs:comment "The logical connection between a work and a related subject entity serves as the basis both for identifying the subject of an individual work and for ensuring that all works relevant to a given subject are linked to that subject."@en ;
    rdfs:domain <http://iflastandards.info/ns/lrm/lrmerE1> ;
    rdfs:isDefinedBy lrmer: ;
    rdfs:range <http://iflastandards.info/ns/lrm/lrmerE2> ;
    rdfs:subPropertyOf <http://iflastandards.info/ns/lrm/lrmerR1> ;
    owl:inverseOf <http://iflastandards.info/ns/lrm/lrmerR12> ;
    skos:definition "Relates any res to a work in which that res is a topic"@en .

<http://iflastandards.info/ns/lrm/lrmerR13> a rdf:Property ;
    rdfs:label "has appellation"@en ;
    reg:lexicalAlias <http://iflastandards.info/ns/lrm/lrmerhasAppellation> ;
    reg:name "hasAppellation" ;
    reg:status <http://metadataregistry.org/uri/RegStatus/1001> ;
    rdfs:comment "The consequence of the definition of nomen as the association between something and a designation that refers to it, is that each nomen is uniquely associated with a single res within a given scheme (which can extend from a specific local system to a natural language, through a shared authority file). The resulting cardinality of the appellation relationship is that while a single res may have many nomens, each nomen is the appellation of a single res. The fact that two instances of nomen may have the same value for their nomen string attribute does not modify this cardinality, and does not imply that such instances of nomen are actually one and the same instance of nomen associated with more than one instance of res, even if the scheme in question is a natural language. The nomen string \"Gift\" may be used to refer either to a present or to a poison, according to whether it is the nomen string value for a nomen within the English language or for a nomen in the German language: although the string nomen values look the same, we do have here two distinct instances of nomen for two distinct instances of res. Although in theory, one instance of nomen (a subclass of res) could be associated to another instance of nomen via the appellation relationship (resulting in a nomen for another nomen), in practice the general case would not be provided for in implementations. Structurally, in a system implementation where instances of the entity nomen are assigned an internal identifier (also a nomen of a specific type) this relationship would be implicit in the system design. An example of this situation could be found in a linked data implementation which assigns a URI (nomen) to instances of nomen of other types."@en ;
    rdfs:domain <http://iflastandards.info/ns/lrm/lrmerE1> ;
    rdfs:isDefinedBy lrmer: ;
    rdfs:range <http://iflastandards.info/ns/lrm/lrmerE9> ;
    rdfs:subPropertyOf <http://iflastandards.info/ns/lrm/lrmerR1> ;
    owl:inverseOf <http://iflastandards.info/ns/lrm/lrmerR13i> ;
    skos:definition "Relates an entity with a sign or combination of signs or symbols through which that entity is referred to within a given scheme or context"@en .

<http://iflastandards.info/ns/lrm/lrmerR13i> a rdf:Property ;
    rdfs:label "is appellation of"@en ;
    reg:lexicalAlias <http://iflastandards.info/ns/lrm/lrmerisAppellationOf> ;
    reg:name "isAppellationOf" ;
    reg:status <http://metadataregistry.org/uri/RegStatus/1001> ;
    rdfs:comment "The consequence of the definition of nomen as the association between something and a designation that refers to it, is that each nomen is uniquely associated with a single res within a given scheme (which can extend from a specific local system to a natural language, through a shared authority file). The resulting cardinality of the appellation relationship is that while a single res may have many nomens, each nomen is the appellation of a single res. The fact that two instances of nomen may have the same value for their nomen string attribute does not modify this cardinality, and does not imply that such instances of nomen are actually one and the same instance of nomen associated with more than one instance of res, even if the scheme in question is a natural language. The nomen string \"Gift\" may be used to refer either to a present or to a poison, according to whether it is the nomen string value for a nomen within the English language or for a nomen in the German language: although the string nomen values look the same, we do have here two distinct instances of nomen for two distinct instances of res. Although in theory, one instance of nomen (a subclass of res) could be associated to another instance of nomen via the appellation relationship (resulting in a nomen for another nomen), in practice the general case would not be provided for in implementations. Structurally, in a system implementation where instances of the entity nomen are assigned an internal identifier (also a nomen of a specific type) this relationship would be implicit in the system design. An example of this situation could be found in a linked data implementation which assigns a URI (nomen) to instances of nomen of other types."@en ;
    rdfs:domain <http://iflastandards.info/ns/lrm/lrmerE9> ;
    rdfs:isDefinedBy lrmer: ;
    rdfs:range <http://iflastandards.info/ns/lrm/lrmerE1> ;
    rdfs:subPropertyOf <http://iflastandards.info/ns/lrm/lrmerR1> ;
    owl:inverseOf <http://iflastandards.info/ns/lrm/lrmerR13> ;
    skos:definition "Relates a nomen with an entity referred through that sign or combination of signs or symbols within a given scheme or context"@en .

<http://iflastandards.info/ns/lrm/lrmerR14> a rdf:Property ;
    rdfs:label "assigned"@en ;
    reg:lexicalAlias <http://iflastandards.info/ns/lrm/lrmerassigned> ;
    reg:name "assigned" ;
    reg:status <http://metadataregistry.org/uri/RegStatus/1001> ;
    rdfs:comment "In the bibliographic context, nomen assignment is applied to the creation of subject terms, controlled access points, identifiers, etc."@en ;
    rdfs:domain <http://iflastandards.info/ns/lrm/lrmerE6> ;
    rdfs:isDefinedBy lrmer: ;
    rdfs:range <http://iflastandards.info/ns/lrm/lrmerE9> ;
    rdfs:subPropertyOf <http://iflastandards.info/ns/lrm/lrmerR1> ;
    owl:inverseOf <http://iflastandards.info/ns/lrm/lrmerR14i> ;
    skos:definition "Relates an agent with a particular nomen that was assigned by this agent"@en .

<http://iflastandards.info/ns/lrm/lrmerR14i> a rdf:Property ;
    rdfs:label "was assigned by"@en ;
    reg:lexicalAlias <http://iflastandards.info/ns/lrm/lrmerwasAssignedBy> ;
    reg:name "wasAssignedBy" ;
    reg:status <http://metadataregistry.org/uri/RegStatus/1001> ;
    rdfs:comment "In the bibliographic context, nomen assignment is applied to the creation of subject terms, controlled access points, identifiers, etc."@en ;
    rdfs:domain <http://iflastandards.info/ns/lrm/lrmerE9> ;
    rdfs:isDefinedBy lrmer: ;
    rdfs:range <http://iflastandards.info/ns/lrm/lrmerE6> ;
    rdfs:subPropertyOf <http://iflastandards.info/ns/lrm/lrmerR1> ;
    owl:inverseOf <http://iflastandards.info/ns/lrm/lrmerR14> ;
    skos:definition "Relates a nomen to an agent that assigned that particular nomen"@en .

<http://iflastandards.info/ns/lrm/lrmerR16> a rdf:Property ;
    rdfs:label "has part nomen"@en ;
    reg:lexicalAlias <http://iflastandards.info/ns/lrm/lrmerhasPartNomen> ;
    reg:name "hasPartNomen" ;
    reg:status <http://metadataregistry.org/uri/RegStatus/1001> ;
    rdfs:comment "The whole-part relationship for nomens is essential in handling the attributes of components of nomens constructed using pre-existing nomens, as such attributes as language may differ between the parts of a compound nomen."@en ;
    rdfs:domain <http://iflastandards.info/ns/lrm/lrmerE9> ;
    rdfs:isDefinedBy lrmer: ;
    rdfs:range <http://iflastandards.info/ns/lrm/lrmerE9> ;
    rdfs:subPropertyOf <http://iflastandards.info/ns/lrm/lrmerR1> ;
    owl:inverseOf <http://iflastandards.info/ns/lrm/lrmerR16i> ;
    skos:definition "Relates a nomen that is constructed using another nomen as a component to that component"@en .

<http://iflastandards.info/ns/lrm/lrmerR16i> a rdf:Property ;
    rdfs:label "is part nomen of"@en ;
    reg:lexicalAlias <http://iflastandards.info/ns/lrm/lrmerisPartNomenOf> ;
    reg:name "isPartNomenOf" ;
    reg:status <http://metadataregistry.org/uri/RegStatus/1001> ;
    rdfs:comment "The whole-part relationship for nomens is essential in handling the attributes of components of nomens constructed using pre-existing nomens, as such attributes as language may differ between the parts of a compound nomen."@en ;
    rdfs:domain <http://iflastandards.info/ns/lrm/lrmerE9> ;
    rdfs:isDefinedBy lrmer: ;
    rdfs:range <http://iflastandards.info/ns/lrm/lrmerE9> ;
    rdfs:subPropertyOf <http://iflastandards.info/ns/lrm/lrmerR1> ;
    owl:inverseOf <http://iflastandards.info/ns/lrm/lrmerR16> ;
    skos:definition "Relates a nomen to another nomen constructed using that nomen as a component"@en .

<http://iflastandards.info/ns/lrm/lrmerR17> a rdf:Property ;
    rdfs:label "is derivation nomen of"@en ;
    reg:lexicalAlias <http://iflastandards.info/ns/lrm/lrmerisDerivationNomenOf> ;
    reg:name "isDerivationNomenOf" ;
    reg:status <http://metadataregistry.org/uri/RegStatus/1001> ;
    rdfs:comment "A nomen may be derived from another due to formal modifications in the notation used (such as transliteration) or cultural or linguistic conventions (creation of abbreviated or shortened or variant forms)."@en ;
    rdfs:domain <http://iflastandards.info/ns/lrm/lrmerE9> ;
    rdfs:isDefinedBy lrmer: ;
    rdfs:range <http://iflastandards.info/ns/lrm/lrmerE9> ;
    rdfs:subPropertyOf <http://iflastandards.info/ns/lrm/lrmerR1> ;
    owl:inverseOf <http://iflastandards.info/ns/lrm/lrmerR17i> ;
    skos:definition "Relates a nomen with another nomen that was used as the basis for the first nomen, both of which are appellations of the same res"@en .

<http://iflastandards.info/ns/lrm/lrmerR17i> a rdf:Property ;
    rdfs:label "has derivation nomen"@en ;
    reg:lexicalAlias <http://iflastandards.info/ns/lrm/lrmerhasDerivationNomen> ;
    reg:name "hasDerivationNomen" ;
    reg:status <http://metadataregistry.org/uri/RegStatus/1001> ;
    rdfs:comment "A nomen may be derived from another due to formal modifications in the notation used (such as transliteration) or cultural or linguistic conventions (creation of abbreviated or shortened or variant forms)."@en ;
    rdfs:domain <http://iflastandards.info/ns/lrm/lrmerE9> ;
    rdfs:isDefinedBy lrmer: ;
    rdfs:range <http://iflastandards.info/ns/lrm/lrmerE9> ;
    rdfs:subPropertyOf <http://iflastandards.info/ns/lrm/lrmerR1> ;
    owl:inverseOf <http://iflastandards.info/ns/lrm/lrmerR17> ;
    skos:definition "Relates a nomen with another nomen for which the first nomen formed the basis, both of which are appellations of the same res"@en .

<http://iflastandards.info/ns/lrm/lrmerR18> a rdf:Property ;
    rdfs:label "has part work"@en ;
    reg:lexicalAlias <http://iflastandards.info/ns/lrm/lrmerhasPartWork> ;
    reg:name "hasPartWork" ;
    reg:status <http://metadataregistry.org/uri/RegStatus/1001> ;
    rdfs:comment "This applies when the component-to-whole relationship is an inherent aspect of the works and holds for all the expressions and manifestations of the larger work and of its component works, whether the expression or manifestation comprises the full larger work or just one or more (but not all) of the component works. Examples include movements of concertos, poems within poetry cycles, multipart novels, triptychs."@en ;
    rdfs:domain <http://iflastandards.info/ns/lrm/lrmerE2> ;
    rdfs:isDefinedBy lrmer: ;
    rdfs:range <http://iflastandards.info/ns/lrm/lrmerE2> ;
    rdfs:subPropertyOf <http://iflastandards.info/ns/lrm/lrmerR1> ;
    owl:inverseOf <http://iflastandards.info/ns/lrm/lrmerR18i> ;
    skos:definition "Relates two works, where the content of the second is a component of the first"@en .

<http://iflastandards.info/ns/lrm/lrmerR18i> a rdf:Property ;
    rdfs:label "is part work of"@en ;
    reg:lexicalAlias <http://iflastandards.info/ns/lrm/lrmerisPartWorkOf> ;
    reg:name "isPartWorkOf" ;
    reg:status <http://metadataregistry.org/uri/RegStatus/1001> ;
    rdfs:comment "This applies when the component-to-whole relationship is an inherent aspect of the works and holds for all the expressions and manifestations of the larger work and of its component works, whether the expression or manifestation comprises the full larger work or just one or more (but not all) of the component works. Examples include movements of concertos, poems within poetry cycles, multipart novels, triptychs."@en ;
    rdfs:domain <http://iflastandards.info/ns/lrm/lrmerE2> ;
    rdfs:isDefinedBy lrmer: ;
    rdfs:range <http://iflastandards.info/ns/lrm/lrmerE2> ;
    rdfs:subPropertyOf <http://iflastandards.info/ns/lrm/lrmerR1> ;
    owl:inverseOf <http://iflastandards.info/ns/lrm/lrmerR18> ;
    skos:definition "Relates two works, where the content of the first is a component of the other"@en .

<http://iflastandards.info/ns/lrm/lrmerR19> a rdf:Property ;
    rdfs:label "precedes work"@en ;
    reg:lexicalAlias <http://iflastandards.info/ns/lrm/lrmerprecedesWork> ;
    reg:name "precedesWork" ;
    reg:status <http://metadataregistry.org/uri/RegStatus/1001> ;
    rdfs:comment "The relationship is about a sequence of ideas and should not be confused with the time of creation of the respective works. As this relationship concerns the logical continuation of the content of the respective works, it does not apply to those serial works that transform over time (via major title changes, changes in media type, etc.) yet maintain a continuity in their form or numbering schemes. See the work-transformation relationship, LRM-R22, to express the relationship between one aggregating or serial work and another that modifies and continues it."@en ;
    rdfs:domain <http://iflastandards.info/ns/lrm/lrmerE2> ;
    rdfs:isDefinedBy lrmer: ;
    rdfs:range <http://iflastandards.info/ns/lrm/lrmerE2> ;
    rdfs:subPropertyOf <http://iflastandards.info/ns/lrm/lrmerR1> ;
    owl:inverseOf <http://iflastandards.info/ns/lrm/lrmerR19i> ;
    skos:definition "Relates two works where the content of the second is a logical continuation of the first"@en .

<http://iflastandards.info/ns/lrm/lrmerR19i> a rdf:Property ;
    rdfs:label "succeeds work"@en ;
    reg:lexicalAlias <http://iflastandards.info/ns/lrm/lrmersucceedsWork> ;
    reg:name "succeedsWork" ;
    reg:status <http://metadataregistry.org/uri/RegStatus/1001> ;
    rdfs:comment "The relationship is about a sequence of ideas and should not be confused with the time of creation of the respective works. As this relationship concerns the logical continuation of the content of the respective works, it does not apply to those serial works that transform over time (via major title changes, changes in media type, etc.) yet maintain a continuity in their form or numbering schemes. See the work-transformation relationship, LRM-R22, to express the relationship between one aggregating or serial work and another that modifies and continues it."@en ;
    rdfs:domain <http://iflastandards.info/ns/lrm/lrmerE2> ;
    rdfs:isDefinedBy lrmer: ;
    rdfs:range <http://iflastandards.info/ns/lrm/lrmerE2> ;
    rdfs:subPropertyOf <http://iflastandards.info/ns/lrm/lrmerR1> ;
    owl:inverseOf <http://iflastandards.info/ns/lrm/lrmerR19> ;
    skos:definition "Relates two works where the content of the first is logically continued by the second"@en .

<http://iflastandards.info/ns/lrm/lrmerR2> a rdf:Property ;
    rdfs:label "is realized through"@en ;
    reg:lexicalAlias <http://iflastandards.info/ns/lrm/lrmerisRealizedThrough> ;
    reg:name "isRealizedThrough" ;
    reg:status <http://metadataregistry.org/uri/RegStatus/1001> ;
    rdfs:comment "The logical connection between work and expression, as reflected in the model through this relationship, serves as the basis both for identifying the work represented by an individual expression and for ensuring that all expressions of a work are linked to the work. Indirectly the relationships between a work and the various expressions of that work also serve to establish a “sibling” relationship between the various expressions of the work."@en ;
    rdfs:domain <http://iflastandards.info/ns/lrm/lrmerE2> ;
    rdfs:isDefinedBy lrmer: ;
    rdfs:range <http://iflastandards.info/ns/lrm/lrmerE3> ;
    rdfs:subPropertyOf <http://iflastandards.info/ns/lrm/lrmerR1> ;
    owl:inverseOf <http://iflastandards.info/ns/lrm/lrmerR2i> ;
    skos:definition "Relates a work with any of the expressions which convey the same intellectual or artistic content"@en .

<http://iflastandards.info/ns/lrm/lrmerR20> a rdf:Property ;
    rdfs:label "accompanies or complements"@en ;
    reg:lexicalAlias <http://iflastandards.info/ns/lrm/lrmeraccompaniesOrComplements> ;
    reg:name "accompaniesOrComplements" ;
    reg:status <http://metadataregistry.org/uri/RegStatus/1001> ;
    rdfs:comment "The relationship between two works which are independent, but can also be used in conjunction with each other as complements or companions. The two works may be adding value to each other (in this case the relationship is symmetrical); in other cases one of the works is considered secondary."@en ;
    rdfs:domain <http://iflastandards.info/ns/lrm/lrmerE2> ;
    rdfs:isDefinedBy lrmer: ;
    rdfs:range <http://iflastandards.info/ns/lrm/lrmerE2> ;
    rdfs:subPropertyOf <http://iflastandards.info/ns/lrm/lrmerR1> ;
    owl:inverseOf <http://iflastandards.info/ns/lrm/lrmerR20i> ;
    skos:definition "Relates a work to another work that it accompanies or complements"@en ;
    skos:scopeNote "Source documentation has \"accompanies / complements\"; slash character replaced with \"or\" to improve clarity."@en .

<http://iflastandards.info/ns/lrm/lrmerR20i> a rdf:Property ;
    rdfs:label "is accompanied or complemented by"@en ;
    reg:lexicalAlias <http://iflastandards.info/ns/lrm/lrmerisAccompaniedOrComplementedBy> ;
    reg:name "isAccompaniedOrComplementedBy" ;
    reg:status <http://metadataregistry.org/uri/RegStatus/1001> ;
    rdfs:comment "The relationship between two works which are independent, but can also be used in conjunction with each other as complements or companions. The two works may be adding value to each other (in this case the relationship is symmetrical); in other cases one of the works is considered secondary."@en ;
    rdfs:domain <http://iflastandards.info/ns/lrm/lrmerE2> ;
    rdfs:isDefinedBy lrmer: ;
    rdfs:range <http://iflastandards.info/ns/lrm/lrmerE2> ;
    rdfs:subPropertyOf <http://iflastandards.info/ns/lrm/lrmerR1> ;
    owl:inverseOf <http://iflastandards.info/ns/lrm/lrmerR20> ;
    skos:definition "Relates a work to another work which is accompanied or complemented by the first work"@en ;
    skos:scopeNote "Source documentation has \"is accompanied / complemented by\"; slash character replaced with \"or\" to improve clarity."@en .

<http://iflastandards.info/ns/lrm/lrmerR21> a rdf:Property ;
    rdfs:label "is inspiration for"@en ;
    reg:lexicalAlias <http://iflastandards.info/ns/lrm/lrmerisInspirationFor> ;
    reg:name "isInspirationFor" ;
    reg:status <http://metadataregistry.org/uri/RegStatus/1001> ;
    rdfs:domain <http://iflastandards.info/ns/lrm/lrmerE2> ;
    rdfs:isDefinedBy lrmer: ;
    rdfs:range <http://iflastandards.info/ns/lrm/lrmerE2> ;
    rdfs:subPropertyOf <http://iflastandards.info/ns/lrm/lrmerR1> ;
    owl:inverseOf <http://iflastandards.info/ns/lrm/lrmerR21i> ;
    skos:definition "Relates two works where the content of the first served as the source of ideas for the second"@en .

<http://iflastandards.info/ns/lrm/lrmerR21i> a rdf:Property ;
    rdfs:label "is inspired by"@en ;
    reg:lexicalAlias <http://iflastandards.info/ns/lrm/lrmerisInspiredBy> ;
    reg:name "isInspiredBy" ;
    reg:status <http://metadataregistry.org/uri/RegStatus/1001> ;
    rdfs:domain <http://iflastandards.info/ns/lrm/lrmerE2> ;
    rdfs:isDefinedBy lrmer: ;
    rdfs:range <http://iflastandards.info/ns/lrm/lrmerE2> ;
    rdfs:subPropertyOf <http://iflastandards.info/ns/lrm/lrmerR1> ;
    owl:inverseOf <http://iflastandards.info/ns/lrm/lrmerR21> ;
    skos:definition "Relates two works where the source of ideas for the second originated in the content of the first"@en .

<http://iflastandards.info/ns/lrm/lrmerR22> a rdf:Property ;
    rdfs:label "is a transformation of"@en ;
    reg:lexicalAlias <http://iflastandards.info/ns/lrm/lrmerisATransformationOf> ;
    reg:name "isATransformationOf" ;
    reg:status <http://metadataregistry.org/uri/RegStatus/1001> ;
    rdfs:comment "Some transformations may be considered as being only inspired by a previous work."@en ;
    rdfs:domain <http://iflastandards.info/ns/lrm/lrmerE2> ;
    rdfs:isDefinedBy lrmer: ;
    rdfs:range <http://iflastandards.info/ns/lrm/lrmerE2> ;
    rdfs:subPropertyOf <http://iflastandards.info/ns/lrm/lrmerR1> ;
    owl:inverseOf <http://iflastandards.info/ns/lrm/lrmerR22i> ;
    skos:definition "Relates a work to a previous work from which it was created by changing the scope or editorial policy (as in a serial or aggregating work), the genre or literary form (dramatization, novelization), target audience (adaptation for children), or style (paraphrase, imitation, parody)"@en .

<http://iflastandards.info/ns/lrm/lrmerR22i> a rdf:Property ;
    rdfs:label "was transformed into"@en ;
    reg:lexicalAlias <http://iflastandards.info/ns/lrm/lrmerwasTransformedInto> ;
    reg:name "wasTransformedInto" ;
    reg:status <http://metadataregistry.org/uri/RegStatus/1001> ;
    rdfs:comment "Some transformations may be considered as being only inspired by a previous work."@en ;
    rdfs:domain <http://iflastandards.info/ns/lrm/lrmerE2> ;
    rdfs:isDefinedBy lrmer: ;
    rdfs:range <http://iflastandards.info/ns/lrm/lrmerE2> ;
    rdfs:subPropertyOf <http://iflastandards.info/ns/lrm/lrmerR1> ;
    owl:inverseOf <http://iflastandards.info/ns/lrm/lrmerR22> ;
    skos:definition "Relates a work to a new work created by changing the scope or editorial policy (as in a serial or aggregating work), the genre or literary form (dramatization, novelization), target audience (adaptation for children), or style (paraphrase, imitation, parody) of the previous work"@en .

<http://iflastandards.info/ns/lrm/lrmerR23> a rdf:Property ;
    rdfs:label "has part expression"@en ;
    reg:lexicalAlias <http://iflastandards.info/ns/lrm/lrmerhasPartExpression> ;
    reg:name "hasPartExpression" ;
    reg:status <http://metadataregistry.org/uri/RegStatus/1001> ;
    rdfs:comment "This applies when the component-to-whole relationship is an inherent aspect of the works and holds for all the expressions and manifestations of the larger work and of its component works, whether the expression or manifestation comprises the full larger work or just one or more (but not all) of the component works."@en ;
    rdfs:domain <http://iflastandards.info/ns/lrm/lrmerE3> ;
    rdfs:isDefinedBy lrmer: ;
    rdfs:range <http://iflastandards.info/ns/lrm/lrmerE3> ;
    rdfs:subPropertyOf <http://iflastandards.info/ns/lrm/lrmerR1> ;
    owl:inverseOf <http://iflastandards.info/ns/lrm/lrmerR23i> ;
    skos:definition "Relates two expressions where the second is a component of the first"@en .

<http://iflastandards.info/ns/lrm/lrmerR23i> a rdf:Property ;
    rdfs:label "is part expression of"@en ;
    reg:lexicalAlias <http://iflastandards.info/ns/lrm/lrmerisPartExpressionOf> ;
    reg:name "isPartExpressionOf" ;
    reg:status <http://metadataregistry.org/uri/RegStatus/1001> ;
    rdfs:comment "This applies when the component-to-whole relationship is an inherent aspect of the works and holds for all the expressions and manifestations of the larger work and of its component works, whether the expression or manifestation comprises the full larger work or just one or more (but not all) of the component works."@en ;
    rdfs:domain <http://iflastandards.info/ns/lrm/lrmerE3> ;
    rdfs:isDefinedBy lrmer: ;
    rdfs:range <http://iflastandards.info/ns/lrm/lrmerE3> ;
    rdfs:subPropertyOf <http://iflastandards.info/ns/lrm/lrmerR1> ;
    owl:inverseOf <http://iflastandards.info/ns/lrm/lrmerR23> ;
    skos:definition "Relates two expressions where the first is a component of the other"@en .

<http://iflastandards.info/ns/lrm/lrmerR24> a rdf:Property ;
    rdfs:label "is derivation expression of"@en ;
    reg:lexicalAlias <http://iflastandards.info/ns/lrm/lrmerisDerivationExpressionOf> ;
    reg:name "isDerivationExpressionOf" ;
    reg:status <http://metadataregistry.org/uri/RegStatus/1001> ;
    rdfs:comment "In many cases, the exact source of, for example, a translation, adaptation, revision, or arrangement is not known. If it is, it may be an interesting aspect for the end-user. The derivation relationship may be refined to provide more detailed information about the nature of the transformation."@en ;
    rdfs:domain <http://iflastandards.info/ns/lrm/lrmerE3> ;
    rdfs:isDefinedBy lrmer: ;
    rdfs:range <http://iflastandards.info/ns/lrm/lrmerE3> ;
    rdfs:subPropertyOf <http://iflastandards.info/ns/lrm/lrmerR1> ;
    owl:inverseOf <http://iflastandards.info/ns/lrm/lrmerR24i> ;
    skos:definition "Relates two expressions of the same work, where the second was used as the source for the other"@en .

<http://iflastandards.info/ns/lrm/lrmerR24i> a rdf:Property ;
    rdfs:label "has derivation expression"@en ;
    reg:lexicalAlias <http://iflastandards.info/ns/lrm/lrmerhasDerivationExpression> ;
    reg:name "hasDerivationExpression" ;
    reg:status <http://metadataregistry.org/uri/RegStatus/1001> ;
    rdfs:comment "In many cases, the exact source of, for example, a translation, adaptation, revision, or arrangement is not known. If it is, it may be an interesting aspect for the end-user. The derivation relationship may be refined to provide more detailed information about the nature of the transformation."@en ;
    rdfs:domain <http://iflastandards.info/ns/lrm/lrmerE3> ;
    rdfs:isDefinedBy lrmer: ;
    rdfs:range <http://iflastandards.info/ns/lrm/lrmerE3> ;
    rdfs:subPropertyOf <http://iflastandards.info/ns/lrm/lrmerR1> ;
    owl:inverseOf <http://iflastandards.info/ns/lrm/lrmerR24> ;
    skos:definition "Relates two expressions of the same work, where the first was used as the source for the other"@en .

<http://iflastandards.info/ns/lrm/lrmerR25> a rdf:Property ;
    rdfs:label "was aggregated by"@en ;
    reg:lexicalAlias <http://iflastandards.info/ns/lrm/lrmerwasAggregatedBy> ;
    reg:name "wasAggregatedBy" ;
    reg:status <http://metadataregistry.org/uri/RegStatus/1001> ;
    rdfs:comment "An aggregating expression will select multiple specific expressions of other works so that they can be embodied together in an aggregate manifestation. An expression may be chosen by multiple aggregating expressions. This is a shortcut of the relationships illustrated in Figure 5.8, the general model for aggregates. EXPRESSION1 is embodied in MANIFESTATION (aggregate) + MANIFESTATION (aggregate) embodies (aggregating) EXPRESSION. Unlike the whole-part relationship between expressions, the expressions selected to appear together in the aggregate manifestation do not become components of the aggregating expression. Furthermore, the relationship between these expressions is not an inherent feature of the works that these expressions realize, and thus is does not hold in other expressions of those works."@en ;
    rdfs:domain <http://iflastandards.info/ns/lrm/lrmerE3> ;
    rdfs:isDefinedBy lrmer: ;
    rdfs:range <http://iflastandards.info/ns/lrm/lrmerE3> ;
    rdfs:subPropertyOf <http://iflastandards.info/ns/lrm/lrmerR1> ;
    owl:inverseOf <http://iflastandards.info/ns/lrm/lrmerR25i> ;
    skos:definition "Relates a specific expression of a work chosen as part of the plan of an aggregating expression to the aggregating expression"@en .

<http://iflastandards.info/ns/lrm/lrmerR25i> a rdf:Property ;
    rdfs:label "aggregated"@en ;
    reg:lexicalAlias <http://iflastandards.info/ns/lrm/lrmeraggregated> ;
    reg:name "aggregated" ;
    reg:status <http://metadataregistry.org/uri/RegStatus/1001> ;
    rdfs:comment "An aggregating expression will select multiple specific expressions of other works so that they can be embodied together in an aggregate manifestation. An expression may be chosen by multiple aggregating expressions. This is a shortcut of the relationships illustrated in Figure 5.8, the general model for aggregates. EXPRESSION1 is embodied in MANIFESTATION (aggregate) + MANIFESTATION (aggregate) embodies (aggregating) EXPRESSION. Unlike the whole-part relationship between expressions, the expressions selected to appear together in the aggregate manifestation do not become components of the aggregating expression. Furthermore, the relationship between these expressions is not an inherent feature of the works that these expressions realize, and thus is does not hold in other expressions of those works."@en ;
    rdfs:domain <http://iflastandards.info/ns/lrm/lrmerE3> ;
    rdfs:isDefinedBy lrmer: ;
    rdfs:range <http://iflastandards.info/ns/lrm/lrmerE3> ;
    rdfs:subPropertyOf <http://iflastandards.info/ns/lrm/lrmerR1> ;
    owl:inverseOf <http://iflastandards.info/ns/lrm/lrmerR25> ;
    skos:definition "Relates an aggregating expression to a specific expression of a work that was chosen as part of the plan of the aggregating expression"@en .

<http://iflastandards.info/ns/lrm/lrmerR26> a rdf:Property ;
    rdfs:label "has part manifestation"@en ;
    reg:lexicalAlias <http://iflastandards.info/ns/lrm/lrmerhasPartManifestation> ;
    reg:name "hasPartManifestation" ;
    reg:status <http://metadataregistry.org/uri/RegStatus/1001> ;
    rdfs:comment "In some cases the components of a manifestation are based on physical considerations relating to the carrier in which the manifestation is intended to be issued (for example, a recording is too long to fit on a single disc and is issued in a two-disc boxed set). An alternate manifestation on another carrier may not display the same components. However, in the case when the component-to-whole relationship is an inherent aspect of the works it holds for all the expressions and manifestations of the larger work and of its component works, whether the expression or manifestation comprises the full larger work or just one or more (but not all) of the component works."@en ;
    rdfs:domain <http://iflastandards.info/ns/lrm/lrmerE4> ;
    rdfs:isDefinedBy lrmer: ;
    rdfs:range <http://iflastandards.info/ns/lrm/lrmerE4> ;
    rdfs:subPropertyOf <http://iflastandards.info/ns/lrm/lrmerR1> ;
    owl:inverseOf <http://iflastandards.info/ns/lrm/lrmerR26i> ;
    skos:definition "Relates two manifestations where the second is a component of the first"@en .

<http://iflastandards.info/ns/lrm/lrmerR26i> a rdf:Property ;
    rdfs:label "is part manifestation of"@en ;
    reg:lexicalAlias <http://iflastandards.info/ns/lrm/lrmerisPartManifestationOf> ;
    reg:name "isPartManifestationOf" ;
    reg:status <http://metadataregistry.org/uri/RegStatus/1001> ;
    rdfs:comment "In some cases the components of a manifestation are based on physical considerations relating to the carrier in which the manifestation is intended to be issued (for example, a recording is too long to fit on a single disc and is issued in a two-disc boxed set). An alternate manifestation on another carrier may not display the same components. However, in the case when the component-to-whole relationship is an inherent aspect of the works it holds for all the expressions and manifestations of the larger work and of its component works, whether the expression or manifestation comprises the full larger work or just one or more (but not all) of the component works."@en ;
    rdfs:domain <http://iflastandards.info/ns/lrm/lrmerE4> ;
    rdfs:isDefinedBy lrmer: ;
    rdfs:range <http://iflastandards.info/ns/lrm/lrmerE4> ;
    rdfs:subPropertyOf <http://iflastandards.info/ns/lrm/lrmerR1> ;
    owl:inverseOf <http://iflastandards.info/ns/lrm/lrmerR26> ;
    skos:definition "Relates two manifestations where the first is a component of the other"@en .

<http://iflastandards.info/ns/lrm/lrmerR27> a rdf:Property ;
    rdfs:label "has reproduction manifestation"@en ;
    reg:lexicalAlias <http://iflastandards.info/ns/lrm/lrmerhasReproductionManifestation> ;
    reg:name "hasReproductionManifestation" ;
    reg:status <http://metadataregistry.org/uri/RegStatus/1001> ;
    rdfs:comment "Generally, for reprints and reissues no specific item of the source manifestation is singled out as the source of the reproduction. Furthermore, in these cases, although a particular item may have been used as a source of reproduction, this item should be considered to represent the source manifestation as a whole. The process of reproduction always results in a new manifestation, even when only a single item was produced from that manifestation."@en ;
    rdfs:domain <http://iflastandards.info/ns/lrm/lrmerE4> ;
    rdfs:isDefinedBy lrmer: ;
    rdfs:range <http://iflastandards.info/ns/lrm/lrmerE4> ;
    rdfs:subPropertyOf <http://iflastandards.info/ns/lrm/lrmerR1> ;
    owl:inverseOf <http://iflastandards.info/ns/lrm/lrmerR27i> ;
    skos:definition "Relates two manifestations providing the end-user with exactly the same content and where an earlier manifestation has provided a source for the creation of a subsequent manifestation, such as facsimiles, reproductions, reprints, and reissues"@en .

<http://iflastandards.info/ns/lrm/lrmerR27i> a rdf:Property ;
    rdfs:label "is reproduction manifestation of"@en ;
    reg:lexicalAlias <http://iflastandards.info/ns/lrm/lrmerisReproductionManifestationOf> ;
    reg:name "isReproductionManifestationOf" ;
    reg:status <http://metadataregistry.org/uri/RegStatus/1001> ;
    rdfs:comment "Generally, for reprints and reissues no specific item of the source manifestation is singled out as the source of the reproduction. Furthermore, in these cases, although a particular item may have been used as a source of reproduction, this item should be considered to represent the source manifestation as a whole. The process of reproduction always results in a new manifestation, even when only a single item was produced from that manifestation."@en ;
    rdfs:domain <http://iflastandards.info/ns/lrm/lrmerE4> ;
    rdfs:isDefinedBy lrmer: ;
    rdfs:range <http://iflastandards.info/ns/lrm/lrmerE4> ;
    rdfs:subPropertyOf <http://iflastandards.info/ns/lrm/lrmerR1> ;
    owl:inverseOf <http://iflastandards.info/ns/lrm/lrmerR27> ;
    skos:definition "Relates two manifestations providing the end-user with exactly the same content and where a subsequent manifestation was created using an earlier manifestation as a source, such as facsimiles, reproductions, reprints, and reissues"@en .

<http://iflastandards.info/ns/lrm/lrmerR28> a rdf:Property ;
    rdfs:label "has reproduction item"@en ;
    reg:lexicalAlias <http://iflastandards.info/ns/lrm/lrmerhasReproductionItem> ;
    reg:name "hasReproductionItem" ;
    reg:status <http://metadataregistry.org/uri/RegStatus/1001> ;
    rdfs:comment "In this case, the particular item used as a source of reproduction is significant, either by its provenance or due to item-specific characteristics such as annotations or ownership markings. The process of reproduction always results in a new manifestation, even when only a single item was produced from that manifestation."@en ;
    rdfs:domain <http://iflastandards.info/ns/lrm/lrmerE5> ;
    rdfs:isDefinedBy lrmer: ;
    rdfs:range <http://iflastandards.info/ns/lrm/lrmerE4> ;
    rdfs:subPropertyOf <http://iflastandards.info/ns/lrm/lrmerR1> ;
    owl:inverseOf <http://iflastandards.info/ns/lrm/lrmerR28i> ;
    skos:definition "Relates an item of one manifestation and another manifestation providing the end-user with exactly the same content and where a specific item has provided a source for the creation of a subsequent manifestation"@en .

<http://iflastandards.info/ns/lrm/lrmerR28i> a rdf:Property ;
    rdfs:label "is reproduction item of"@en ;
    reg:lexicalAlias <http://iflastandards.info/ns/lrm/lrmerisReproductionItemOf> ;
    reg:name "isReproductionItemOf" ;
    reg:status <http://metadataregistry.org/uri/RegStatus/1001> ;
    rdfs:comment "In this case, the particular item used as a source of reproduction is significant, either by its provenance or due to item-specific characteristics such as annotations or ownership markings. The process of reproduction always results in a new manifestation, even when only a single item was produced from that manifestation."@en ;
    rdfs:domain <http://iflastandards.info/ns/lrm/lrmerE4> ;
    rdfs:isDefinedBy lrmer: ;
    rdfs:range <http://iflastandards.info/ns/lrm/lrmerE5> ;
    rdfs:subPropertyOf <http://iflastandards.info/ns/lrm/lrmerR1> ;
    owl:inverseOf <http://iflastandards.info/ns/lrm/lrmerR28> ;
    skos:definition "Relates a manifestation and a specific item of another manifestation which provided a source for the creation of the subsequent manifestation providing the end-user with exactly the same content"@en .

<http://iflastandards.info/ns/lrm/lrmerR2i> a rdf:Property ;
    rdfs:label "realizes"@en ;
    reg:lexicalAlias <http://iflastandards.info/ns/lrm/lrmerrealizes> ;
    reg:name "realizes" ;
    reg:status <http://metadataregistry.org/uri/RegStatus/1001> ;
    rdfs:comment "The logical connection between work and expression, as reflected in the model through this relationship, serves as the basis both for identifying the work represented by an individual expression and for ensuring that all expressions of a work are linked to the work. Indirectly the relationships between a work and the various expressions of that work also serve to establish a “sibling” relationship between the various expressions of the work."@en ;
    rdfs:domain <http://iflastandards.info/ns/lrm/lrmerE3> ;
    rdfs:isDefinedBy lrmer: ;
    rdfs:range <http://iflastandards.info/ns/lrm/lrmerE2> ;
    rdfs:subPropertyOf <http://iflastandards.info/ns/lrm/lrmerR1> ;
    owl:inverseOf <http://iflastandards.info/ns/lrm/lrmerR2> ;
    skos:definition "Relates an expression with the work whose intellectual or artistic content it conveys"@en .

<http://iflastandards.info/ns/lrm/lrmerR3> a rdf:Property ;
    rdfs:label "is embodied in"@en ;
    reg:lexicalAlias <http://iflastandards.info/ns/lrm/lrmerisEmbodiedIn> ;
    reg:name "isEmbodiedIn" ;
    reg:status <http://metadataregistry.org/uri/RegStatus/1001> ;
    rdfs:comment "A manifestation may embody one or more expressions and any expression may be embodied in one or more manifestations. This logical connection serves as the basis both for identifying the specific expression or expressions of a work or works embodied in an individual manifestation and for ensuring that all manifestations of the same expression are linked back to that expression."@en ;
    rdfs:domain <http://iflastandards.info/ns/lrm/lrmerE3> ;
    rdfs:isDefinedBy lrmer: ;
    rdfs:range <http://iflastandards.info/ns/lrm/lrmerE4> ;
    rdfs:subPropertyOf <http://iflastandards.info/ns/lrm/lrmerR1> ;
    owl:inverseOf <http://iflastandards.info/ns/lrm/lrmerR3i> ;
    skos:definition "Relates an expression with a manifestation in which the expression appears"@en .

<http://iflastandards.info/ns/lrm/lrmerR30> a rdf:Property ;
    rdfs:label "is member of"@en ;
    reg:lexicalAlias <http://iflastandards.info/ns/lrm/lrmerisMemberOf> ;
    reg:name "isMemberOf" ;
    reg:status <http://metadataregistry.org/uri/RegStatus/1001> ;
    rdfs:comment "A person may explicitly join an organization or association. A person may implicitly become a member of a family by birth, adoption, marriage, etc. A collective agent may join another collective agent as a member."@en ;
    rdfs:domain <http://iflastandards.info/ns/lrm/lrmerE6> ;
    rdfs:isDefinedBy lrmer: ;
    rdfs:range <http://iflastandards.info/ns/lrm/lrmerE8> ;
    rdfs:subPropertyOf <http://iflastandards.info/ns/lrm/lrmerR1> ;
    owl:inverseOf <http://iflastandards.info/ns/lrm/lrmerR30i> ;
    skos:definition "Relates an agent and a collective agent that the agent joined as a member"@en .

<http://iflastandards.info/ns/lrm/lrmerR30i> a rdf:Property ;
    rdfs:label "has member"@en ;
    reg:lexicalAlias <http://iflastandards.info/ns/lrm/lrmerhasMember> ;
    reg:name "hasMember" ;
    reg:status <http://metadataregistry.org/uri/RegStatus/1001> ;
    rdfs:comment "A person may explicitly join an organization or association. A person may implicitly become a member of a family by birth, adoption, marriage, etc. A collective agent may join another collective agent as a member."@en ;
    rdfs:domain <http://iflastandards.info/ns/lrm/lrmerE8> ;
    rdfs:isDefinedBy lrmer: ;
    rdfs:range <http://iflastandards.info/ns/lrm/lrmerE6> ;
    rdfs:subPropertyOf <http://iflastandards.info/ns/lrm/lrmerR1> ;
    owl:inverseOf <http://iflastandards.info/ns/lrm/lrmerR30> ;
    skos:definition "Relates a collective agent to an agent that joined the collective agent as a member"@en .

<http://iflastandards.info/ns/lrm/lrmerR31> a rdf:Property ;
    rdfs:label "has part collective agent"@en ;
    reg:lexicalAlias <http://iflastandards.info/ns/lrm/lrmerhasPartCollectiveAgent> ;
    reg:name "hasPartCollectiveAgent" ;
    reg:status <http://metadataregistry.org/uri/RegStatus/1001> ;
    rdfs:comment "This is a relationship between two collective agents where one is a component of the other"@en ;
    rdfs:domain <http://iflastandards.info/ns/lrm/lrmerE8> ;
    rdfs:isDefinedBy lrmer: ;
    rdfs:range <http://iflastandards.info/ns/lrm/lrmerE8> ;
    rdfs:subPropertyOf <http://iflastandards.info/ns/lrm/lrmerR1> ;
    owl:inverseOf <http://iflastandards.info/ns/lrm/lrmerR31i> ;
    skos:definition "Relates two collective agents where the second is a component of the first"@en .

<http://iflastandards.info/ns/lrm/lrmerR31i> a rdf:Property ;
    rdfs:label "is part collective agent of"@en ;
    reg:lexicalAlias <http://iflastandards.info/ns/lrm/lrmerisPartCollectiveAgentOf> ;
    reg:name "isPartCollectiveAgentOf" ;
    reg:status <http://metadataregistry.org/uri/RegStatus/1001> ;
    rdfs:comment "This is a relationship between two collective agents where one is a component of the other"@en ;
    rdfs:domain <http://iflastandards.info/ns/lrm/lrmerE8> ;
    rdfs:isDefinedBy lrmer: ;
    rdfs:range <http://iflastandards.info/ns/lrm/lrmerE8> ;
    rdfs:subPropertyOf <http://iflastandards.info/ns/lrm/lrmerR1> ;
    owl:inverseOf <http://iflastandards.info/ns/lrm/lrmerR31> ;
    skos:definition "Relates two collective agents where the first is a component of the other"@en .

<http://iflastandards.info/ns/lrm/lrmerR32> a rdf:Property ;
    rdfs:label "precedes collective agent"@en ;
    reg:lexicalAlias <http://iflastandards.info/ns/lrm/lrmerprecedesCollectiveAgent> ;
    reg:name "precedesCollectiveAgent" ;
    reg:status <http://metadataregistry.org/uri/RegStatus/1001> ;
    rdfs:comment "A single instance of this relationship can record a simple transformation of a single collective agent into a single successor. Multiple instances of this relationship can be used together to capture the more complex mergers and splits that can occur between and among collective agents."@en ;
    rdfs:domain <http://iflastandards.info/ns/lrm/lrmerE8> ;
    rdfs:isDefinedBy lrmer: ;
    rdfs:range <http://iflastandards.info/ns/lrm/lrmerE8> ;
    rdfs:subPropertyOf <http://iflastandards.info/ns/lrm/lrmerR1> ;
    owl:inverseOf <http://iflastandards.info/ns/lrm/lrmerR32i> ;
    skos:definition "Relates two collective agents where the first was transformed into the second"@en .

<http://iflastandards.info/ns/lrm/lrmerR32i> a rdf:Property ;
    rdfs:label "succeeds collective agent"@en ;
    reg:lexicalAlias <http://iflastandards.info/ns/lrm/lrmersucceedsCollectiveAgent> ;
    reg:name "succeedsCollectiveAgent" ;
    reg:status <http://metadataregistry.org/uri/RegStatus/1001> ;
    rdfs:comment "A single instance of this relationship can record a simple transformation of a single collective agent into a single successor. Multiple instances of this relationship can be used together to capture the more complex mergers and splits that can occur between and among collective agents."@en ;
    rdfs:domain <http://iflastandards.info/ns/lrm/lrmerE8> ;
    rdfs:isDefinedBy lrmer: ;
    rdfs:range <http://iflastandards.info/ns/lrm/lrmerE8> ;
    rdfs:subPropertyOf <http://iflastandards.info/ns/lrm/lrmerR1> ;
    owl:inverseOf <http://iflastandards.info/ns/lrm/lrmerR32> ;
    skos:definition "Relates two collective agents where the second came into being as a transformation of the first"@en .

<http://iflastandards.info/ns/lrm/lrmerR33> a rdf:Property ;
    rdfs:label "has association with place"@en ;
    reg:lexicalAlias <http://iflastandards.info/ns/lrm/lrmerhasAssociationWithPlace> ;
    reg:name "hasAssociationWithPlace" ;
    reg:status <http://metadataregistry.org/uri/RegStatus/1001> ;
    rdfs:comment "In most implementations this relationship would be refined to reflect the exact nature of the association, for example, place of work conception or creation, place of expression creation (e.g., place of musical performance), place of publication or manufacture, current or former location of an item, and location of an agent."@en ;
    rdfs:domain <http://iflastandards.info/ns/lrm/lrmerE1> ;
    rdfs:isDefinedBy lrmer: ;
    rdfs:range <http://iflastandards.info/ns/lrm/lrmerE10> ;
    rdfs:subPropertyOf <http://iflastandards.info/ns/lrm/lrmerR1> ;
    owl:inverseOf <http://iflastandards.info/ns/lrm/lrmerR33i> ;
    skos:definition "Relates any entity with a given extent of space"@en .

<http://iflastandards.info/ns/lrm/lrmerR33i> a rdf:Property ;
    rdfs:label "is associated with place"@en ;
    reg:lexicalAlias <http://iflastandards.info/ns/lrm/lrmerisAssociatedWithPlace> ;
    reg:name "isAssociatedWithPlace" ;
    reg:status <http://metadataregistry.org/uri/RegStatus/1001> ;
    rdfs:comment "In most implementations this relationship would be refined to reflect the exact nature of the association, for example, place of work conception or creation, place of expression creation (e.g., place of musical performance), place of publication or manufacture, current or former location of an item, and location of an agent."@en ;
    rdfs:domain <http://iflastandards.info/ns/lrm/lrmerE10> ;
    rdfs:isDefinedBy lrmer: ;
    rdfs:range <http://iflastandards.info/ns/lrm/lrmerE1> ;
    rdfs:subPropertyOf <http://iflastandards.info/ns/lrm/lrmerR1> ;
    owl:inverseOf <http://iflastandards.info/ns/lrm/lrmerR33> ;
    skos:definition "Relates a place with any entity"@en .

<http://iflastandards.info/ns/lrm/lrmerR34> a rdf:Property ;
    rdfs:label "has part place"@en ;
    reg:lexicalAlias <http://iflastandards.info/ns/lrm/lrmerhasPartPlace> ;
    reg:name "hasPartPlace" ;
    reg:status <http://metadataregistry.org/uri/RegStatus/1001> ;
    rdfs:comment "This is a relationship between two places where one is a component of the other"@en ;
    rdfs:domain <http://iflastandards.info/ns/lrm/lrmerE10> ;
    rdfs:isDefinedBy lrmer: ;
    rdfs:range <http://iflastandards.info/ns/lrm/lrmerE10> ;
    rdfs:subPropertyOf <http://iflastandards.info/ns/lrm/lrmerR1> ;
    owl:inverseOf <http://iflastandards.info/ns/lrm/lrmerR34i> ;
    skos:definition "Relates two places where the second is a component of the first"@en .

<http://iflastandards.info/ns/lrm/lrmerR34i> a rdf:Property ;
    rdfs:label "is part place of"@en ;
    reg:lexicalAlias <http://iflastandards.info/ns/lrm/lrmerisPartPlaceOf> ;
    reg:name "isPartPlaceOf" ;
    reg:status <http://metadataregistry.org/uri/RegStatus/1001> ;
    rdfs:comment "This is a relationship between two places where one is a component of the other"@en ;
    rdfs:domain <http://iflastandards.info/ns/lrm/lrmerE10> ;
    rdfs:isDefinedBy lrmer: ;
    rdfs:range <http://iflastandards.info/ns/lrm/lrmerE10> ;
    rdfs:subPropertyOf <http://iflastandards.info/ns/lrm/lrmerR1> ;
    owl:inverseOf <http://iflastandards.info/ns/lrm/lrmerR34> ;
    skos:definition "Relates two places where the first is a component of the other"@en .

<http://iflastandards.info/ns/lrm/lrmerR35> a rdf:Property ;
    rdfs:label "has association with time-span"@en ;
    reg:lexicalAlias <http://iflastandards.info/ns/lrm/lrmerHasAssociationWithTime-span> ;
    reg:name "HasAssociationWithTime-span" ;
    reg:status <http://metadataregistry.org/uri/RegStatus/1001> ;
    rdfs:comment "In most implementations this relationship would be refined to reflect the exact nature of the association, for example, time of work conception or creation, time of expression creation (e.g., date/time of musical performance), time of publication or manufacture, period of ownership of an item, date of birth of a person, time of validity of the nomen for a particular res."@en ;
    rdfs:domain <http://iflastandards.info/ns/lrm/lrmerE1> ;
    rdfs:isDefinedBy lrmer: ;
    rdfs:range <http://iflastandards.info/ns/lrm/lrmerE11> ;
    rdfs:subPropertyOf <http://iflastandards.info/ns/lrm/lrmerR1> ;
    owl:inverseOf <http://iflastandards.info/ns/lrm/lrmerR35i> ;
    skos:definition "Relates any entity with a temporal extent"@en .

<http://iflastandards.info/ns/lrm/lrmerR35i> a rdf:Property ;
    rdfs:label "is associated with time-span"@en ;
    reg:lexicalAlias <http://iflastandards.info/ns/lrm/lrmerIsAssociatedWithTime-span> ;
    reg:name "IsAssociatedWithTime-span" ;
    reg:status <http://metadataregistry.org/uri/RegStatus/1001> ;
    rdfs:comment "In most implementations this relationship would be refined to reflect the exact nature of the association, for example, time of work conception or creation, time of expression creation (e.g., date/time of musical performance), time of publication or manufacture, period of ownership of an item, date of birth of a person, time of validity of the nomen for a particular res."@en ;
    rdfs:domain <http://iflastandards.info/ns/lrm/lrmerE11> ;
    rdfs:isDefinedBy lrmer: ;
    rdfs:range <http://iflastandards.info/ns/lrm/lrmerE1> ;
    rdfs:subPropertyOf <http://iflastandards.info/ns/lrm/lrmerR1> ;
    owl:inverseOf <http://iflastandards.info/ns/lrm/lrmerR35> ;
    skos:definition "Relates a time-span with any entity"@en .

<http://iflastandards.info/ns/lrm/lrmerR36> a rdf:Property ;
    rdfs:label "has part time-span"@en ;
    reg:lexicalAlias <http://iflastandards.info/ns/lrm/lrmerhasPartTime-span> ;
    reg:name "hasPartTime-span" ;
    reg:status <http://metadataregistry.org/uri/RegStatus/1001> ;
    rdfs:comment "This is a relationship between two time-spans where one is a component of the other"@en ;
    rdfs:domain <http://iflastandards.info/ns/lrm/lrmerE11> ;
    rdfs:isDefinedBy lrmer: ;
    rdfs:range <http://iflastandards.info/ns/lrm/lrmerE11> ;
    rdfs:subPropertyOf <http://iflastandards.info/ns/lrm/lrmerR1> ;
    owl:inverseOf <http://iflastandards.info/ns/lrm/lrmerR36i> ;
    skos:definition "Relates two time-spans where the second is a component of the first"@en .

<http://iflastandards.info/ns/lrm/lrmerR36i> a rdf:Property ;
    rdfs:label "is part time-span of"@en ;
    reg:lexicalAlias <http://iflastandards.info/ns/lrm/lrmerIsPartTime-spanOf> ;
    reg:name "IsPartTime-spanOf" ;
    reg:status <http://metadataregistry.org/uri/RegStatus/1001> ;
    rdfs:comment "This is a relationship between two time-spans where one is a component of the other"@en ;
    rdfs:domain <http://iflastandards.info/ns/lrm/lrmerE11> ;
    rdfs:isDefinedBy lrmer: ;
    rdfs:range <http://iflastandards.info/ns/lrm/lrmerE11> ;
    rdfs:subPropertyOf <http://iflastandards.info/ns/lrm/lrmerR1> ;
    owl:inverseOf <http://iflastandards.info/ns/lrm/lrmerR36> ;
    skos:definition "Relates two time-spans where the first is a component of the other"@en .

<http://iflastandards.info/ns/lrm/lrmerR3i> a rdf:Property ;
    rdfs:label "embodies"@en ;
    reg:lexicalAlias <http://iflastandards.info/ns/lrm/lrmerembodies> ;
    reg:name "embodies" ;
    reg:status <http://metadataregistry.org/uri/RegStatus/1001> ;
    rdfs:comment "A manifestation may embody one or more expressions and any expression may be embodied in one or more manifestations. This logical connection serves as the basis both for identifying the specific expression or expressions of a work or works embodied in an individual manifestation and for ensuring that all manifestations of the same expression are linked back to that expression."@en ;
    rdfs:domain <http://iflastandards.info/ns/lrm/lrmerE4> ;
    rdfs:isDefinedBy lrmer: ;
    rdfs:range <http://iflastandards.info/ns/lrm/lrmerE3> ;
    rdfs:subPropertyOf <http://iflastandards.info/ns/lrm/lrmerR1> ;
    owl:inverseOf <http://iflastandards.info/ns/lrm/lrmerR3> ;
    skos:definition "Relates a manifestation with an expression which appears in the manifestation"@en .

<http://iflastandards.info/ns/lrm/lrmerR4> a rdf:Property ;
    rdfs:label "is exemplified by"@en ;
    reg:lexicalAlias <http://iflastandards.info/ns/lrm/lrmerisExemplifiedBy> ;
    reg:name "isExemplifiedBy" ;
    reg:status <http://metadataregistry.org/uri/RegStatus/1001> ;
    rdfs:comment "The logical connection serves as the basis both for identifying the manifestation exemplified by an individual item and for ensuring that all items of the same manifestation are linked to that manifestation. Indirectly the relationships between a manifestation and the various items exemplifying that manifestation also serve to establish a “sibling” relationship between the various items of a manifestation."@en ;
    rdfs:domain <http://iflastandards.info/ns/lrm/lrmerE4> ;
    rdfs:isDefinedBy lrmer: ;
    rdfs:range <http://iflastandards.info/ns/lrm/lrmerE5> ;
    rdfs:subPropertyOf <http://iflastandards.info/ns/lrm/lrmerR1> ;
    owl:inverseOf <http://iflastandards.info/ns/lrm/lrmerR4i> ;
    skos:definition "Relates a manifestation with any item that reflects the characteristics of that manifestation"@en .

<http://iflastandards.info/ns/lrm/lrmerR4i> a rdf:Property ;
    rdfs:label "exemplifies"@en ;
    reg:lexicalAlias <http://iflastandards.info/ns/lrm/lrmerexemplifies> ;
    reg:name "exemplifies" ;
    reg:status <http://metadataregistry.org/uri/RegStatus/1001> ;
    rdfs:comment "The logical connection serves as the basis both for identifying the manifestation exemplified by an individual item and for ensuring that all items of the same manifestation are linked to that manifestation. Indirectly the relationships between a manifestation and the various items exemplifying that manifestation also serve to establish a “sibling” relationship between the various items of a manifestation."@en ;
    rdfs:domain <http://iflastandards.info/ns/lrm/lrmerE5> ;
    rdfs:isDefinedBy lrmer: ;
    rdfs:range <http://iflastandards.info/ns/lrm/lrmerE4> ;
    rdfs:subPropertyOf <http://iflastandards.info/ns/lrm/lrmerR1> ;
    owl:inverseOf <http://iflastandards.info/ns/lrm/lrmerR4> ;
    skos:definition "Relates an item with the manifestation whose characteristics are reflected in the item"@en .

<http://iflastandards.info/ns/lrm/lrmerR5> a rdf:Property ;
    rdfs:label "was created by work"@en ;
    reg:lexicalAlias <http://iflastandards.info/ns/lrm/lrmerwasCreatedByWork> ;
    reg:name "wasCreatedByWork" ;
    reg:status <http://metadataregistry.org/uri/RegStatus/1001> ;
    rdfs:comment "The logical connection between a work and a related agent serves as the basis both for identifying an agent responsible for an individual work and for ensuring that all works by a particular agent are linked to that agent."@en ;
    rdfs:domain <http://iflastandards.info/ns/lrm/lrmerE2> ;
    rdfs:isDefinedBy lrmer: ;
    rdfs:range <http://iflastandards.info/ns/lrm/lrmerE6> ;
    rdfs:subPropertyOf <http://iflastandards.info/ns/lrm/lrmerR1> ;
    owl:inverseOf <http://iflastandards.info/ns/lrm/lrmerR5i> ;
    skos:definition "Relates a work to an agent responsible for the creation of the intellectual or artistic content"@en .

<http://iflastandards.info/ns/lrm/lrmerR5i> a rdf:Property ;
    rdfs:label "created work"@en ;
    reg:lexicalAlias <http://iflastandards.info/ns/lrm/lrmercreatedWork> ;
    reg:name "createdWork" ;
    reg:status <http://metadataregistry.org/uri/RegStatus/1001> ;
    rdfs:comment "The logical connection between a work and a related agent serves as the basis both for identifying an agent responsible for an individual work and for ensuring that all works by a particular agent are linked to that agent."@en ;
    rdfs:domain <http://iflastandards.info/ns/lrm/lrmerE6> ;
    rdfs:isDefinedBy lrmer: ;
    rdfs:range <http://iflastandards.info/ns/lrm/lrmerE2> ;
    rdfs:subPropertyOf <http://iflastandards.info/ns/lrm/lrmerR1> ;
    owl:inverseOf <http://iflastandards.info/ns/lrm/lrmerR5> ;
    skos:definition "Relates an agent to a work for which the agent is responsible for the creation of intellectual or artistic content"@en .

<http://iflastandards.info/ns/lrm/lrmerR6> a rdf:Property ;
    rdfs:label "was created by expression"@en ;
    reg:lexicalAlias <http://iflastandards.info/ns/lrm/lrmerwasCreatedByExpression> ;
    reg:name "wasCreatedByExpression" ;
    reg:status <http://metadataregistry.org/uri/RegStatus/1001> ;
    rdfs:comment "This relationship applies both to the creation of the original expression and any subsequent modifications such as translations, revisions and performances. An agent responsible for the intellectual or artistic content of a work is responsible for the conception of the work as an abstract entity; an agent responsible for the expression of the work is responsible for the specifics of the intellectual or artistic realization or execution of the expression. The logical connection between an expression and a related agent serves as the basis both for identifying an agent responsible for an individual expression and for ensuring that all expressions realized by an agent are linked to that agent."@en ;
    rdfs:domain <http://iflastandards.info/ns/lrm/lrmerE3> ;
    rdfs:isDefinedBy lrmer: ;
    rdfs:range <http://iflastandards.info/ns/lrm/lrmerE6> ;
    rdfs:subPropertyOf <http://iflastandards.info/ns/lrm/lrmerR1> ;
    owl:inverseOf <http://iflastandards.info/ns/lrm/lrmerR6i> ;
    skos:definition "Relates an expression to an agent responsible for the realization of a work"@en .

<http://iflastandards.info/ns/lrm/lrmerR6i> a rdf:Property ;
    rdfs:label "created expression"@en ;
    reg:lexicalAlias <http://iflastandards.info/ns/lrm/lrmercreatedExpression> ;
    reg:name "createdExpression" ;
    reg:status <http://metadataregistry.org/uri/RegStatus/1001> ;
    rdfs:comment "This relationship applies both to the creation of the original expression and any subsequent modifications such as translations, revisions and performances. An agent responsible for the intellectual or artistic content of a work is responsible for the conception of the work as an abstract entity; an agent responsible for the expression of the work is responsible for the specifics of the intellectual or artistic realization or execution of the expression. The logical connection between an expression and a related agent serves as the basis both for identifying an agent responsible for an individual expression and for ensuring that all expressions realized by an agent are linked to that agent."@en ;
    rdfs:domain <http://iflastandards.info/ns/lrm/lrmerE6> ;
    rdfs:isDefinedBy lrmer: ;
    rdfs:range <http://iflastandards.info/ns/lrm/lrmerE3> ;
    rdfs:subPropertyOf <http://iflastandards.info/ns/lrm/lrmerR1> ;
    owl:inverseOf <http://iflastandards.info/ns/lrm/lrmerR6> ;
    skos:definition "Relates an agent to an expression in which the agent is responsible for the realization of a work"@en .

<http://iflastandards.info/ns/lrm/lrmerR7> a rdf:Property ;
    rdfs:label "was created by manifestation"@en ;
    reg:lexicalAlias <http://iflastandards.info/ns/lrm/lrmerwasCreatedByManifestation> ;
    reg:name "wasCreatedByManifestation" ;
    reg:status <http://metadataregistry.org/uri/RegStatus/1001> ;
    rdfs:comment "For a manifestation, the notion of creation broadly includes the publication process for published manifestations. The logical connection between a manifestation and a related agent serves as the basis both for identifying an agent responsible for creating a manifestation and for ensuring that all manifestations created by an agent are linked to that agent."@en ;
    rdfs:domain <http://iflastandards.info/ns/lrm/lrmerE4> ;
    rdfs:isDefinedBy lrmer: ;
    rdfs:range <http://iflastandards.info/ns/lrm/lrmerE6> ;
    rdfs:subPropertyOf <http://iflastandards.info/ns/lrm/lrmerR1> ;
    owl:inverseOf <http://iflastandards.info/ns/lrm/lrmerR7i> ;
    skos:definition "Relates a manifestation to an agent responsible for creating the manifestation"@en .

<http://iflastandards.info/ns/lrm/lrmerR7i> a rdf:Property ;
    rdfs:label "created manifestation"@en ;
    reg:lexicalAlias <http://iflastandards.info/ns/lrm/lrmercreatedManifestation> ;
    reg:name "createdManifestation" ;
    reg:status <http://metadataregistry.org/uri/RegStatus/1001> ;
    rdfs:comment "For a manifestation, the notion of creation broadly includes the publication process for published manifestations. The logical connection between a manifestation and a related agent serves as the basis both for identifying an agent responsible for creating a manifestation and for ensuring that all manifestations created by an agent are linked to that agent."@en ;
    rdfs:domain <http://iflastandards.info/ns/lrm/lrmerE6> ;
    rdfs:isDefinedBy lrmer: ;
    rdfs:range <http://iflastandards.info/ns/lrm/lrmerE4> ;
    rdfs:subPropertyOf <http://iflastandards.info/ns/lrm/lrmerR1> ;
    owl:inverseOf <http://iflastandards.info/ns/lrm/lrmerR7> ;
    skos:definition "Relates an agent to a manifestation that the agent is responsible for creating"@en .

<http://iflastandards.info/ns/lrm/lrmerR8> a rdf:Property ;
    rdfs:label "was manufactured by"@en ;
    reg:lexicalAlias <http://iflastandards.info/ns/lrm/lrmerwasManufacturedBy> ;
    reg:name "wasManufacturedBy" ;
    reg:status <http://metadataregistry.org/uri/RegStatus/1001> ;
    rdfs:comment "The manifestation may be manufactured or produced through industrial processes or through artisanal methods."@en ;
    rdfs:domain <http://iflastandards.info/ns/lrm/lrmerE4> ;
    rdfs:isDefinedBy lrmer: ;
    rdfs:range <http://iflastandards.info/ns/lrm/lrmerE6> ;
    rdfs:subPropertyOf <http://iflastandards.info/ns/lrm/lrmerR1> ;
    owl:inverseOf <http://iflastandards.info/ns/lrm/lrmerR8i> ;
    skos:definition "Relates a manifestation to an agent responsible for the fabrication, production or manufacture of the items of that manifestation"@en .

<http://iflastandards.info/ns/lrm/lrmerR8i> a rdf:Property ;
    rdfs:label "manufactured"@en ;
    reg:lexicalAlias <http://iflastandards.info/ns/lrm/lrmermanufactured> ;
    reg:name "manufactured" ;
    reg:status <http://metadataregistry.org/uri/RegStatus/1001> ;
    rdfs:comment "The manifestation may be manufactured or produced through industrial processes or through artisanal methods."@en ;
    rdfs:domain <http://iflastandards.info/ns/lrm/lrmerE6> ;
    rdfs:isDefinedBy lrmer: ;
    rdfs:range <http://iflastandards.info/ns/lrm/lrmerE4> ;
    rdfs:subPropertyOf <http://iflastandards.info/ns/lrm/lrmerR1> ;
    owl:inverseOf <http://iflastandards.info/ns/lrm/lrmerR8> ;
    skos:definition "Relates an agent to a manifestation for which the agent is responsible for the fabrication, production or manufacture of items"@en .

<http://iflastandards.info/ns/lrm/lrmerR9> a rdf:Property ;
    rdfs:label "is distributed by"@en ;
    reg:lexicalAlias <http://iflastandards.info/ns/lrm/lrmerisDistributedBy> ;
    reg:name "isDistributedBy" ;
    reg:status <http://metadataregistry.org/uri/RegStatus/1001> ;
    rdfs:comment "The items can be made available through the traditional distribution processes for physical items, or by making electronic items available for download, streaming, etc."@en ;
    rdfs:domain <http://iflastandards.info/ns/lrm/lrmerE4> ;
    rdfs:isDefinedBy lrmer: ;
    rdfs:range <http://iflastandards.info/ns/lrm/lrmerE6> ;
    rdfs:subPropertyOf <http://iflastandards.info/ns/lrm/lrmerR1> ;
    owl:inverseOf <http://iflastandards.info/ns/lrm/lrmerR9i> ;
    skos:definition "Relates a manifestation to an agent responsible for making items of that manifestation available"@en .

<http://iflastandards.info/ns/lrm/lrmerR9i> a rdf:Property ;
    rdfs:label "distributes"@en ;
    reg:lexicalAlias <http://iflastandards.info/ns/lrm/lrmerdistributes> ;
    reg:name "distributes" ;
    reg:status <http://metadataregistry.org/uri/RegStatus/1001> ;
    rdfs:comment "The items can be made available through the traditional distribution processes for physical items, or by making electronic items available for download, streaming, etc."@en ;
    rdfs:domain <http://iflastandards.info/ns/lrm/lrmerE6> ;
    rdfs:isDefinedBy lrmer: ;
    rdfs:range <http://iflastandards.info/ns/lrm/lrmerE4> ;
    rdfs:subPropertyOf <http://iflastandards.info/ns/lrm/lrmerR1> ;
    owl:inverseOf <http://iflastandards.info/ns/lrm/lrmerR9> ;
    skos:definition "Relates an agent to a manifestation for which the agent is responsible for making items of that manifestation available"@en .

<http://iflastandards.info/ns/lrm/lrmerE7> a owl:Class ;
    rdfs:label "Person"@en ;
    reg:lexicalAlias <http://iflastandards.info/ns/lrm/lrmerPerson> ;
    reg:name "Person" ;
    reg:status <http://metadataregistry.org/uri/RegStatus/1001> ;
    rdfs:comment "The entity person is restricted to real persons who live or are assumed to have lived. Strict proof of the existence of a person is not required, as long as there is a general acceptance of their probable historicity. However, figures generally considered fictional (for example, Kermit the Frog), literary (for example, Miss Jane Marple) or purely legendary (for example, the wizard Merlin) are not instances of the entity person."@en ;
    rdfs:isDefinedBy lrmer: ;
    rdfs:subClassOf <http://iflastandards.info/ns/lrm/lrmerE6> ;
    owl:disjointWith <http://iflastandards.info/ns/lrm/lrmerE8> ;
    skos:definition "An individual human being"@en .

<http://iflastandards.info/ns/lrm/lrmerE1A1> a rdf:Property ;
    rdfs:label "has category of res"@en ;
    reg:lexicalAlias <http://iflastandards.info/ns/lrm/lrmerhasCategoryOfRes> ;
    reg:name "hasCategoryOfRes" ;
    reg:status <http://metadataregistry.org/uri/RegStatus/1001> ;
    rdfs:domain <http://iflastandards.info/ns/lrm/lrmerE1> ;
    rdfs:isDefinedBy lrmer: ;
    skos:definition "Relates a res to a type to which the res belongs"@en .

<http://iflastandards.info/ns/lrm/lrmerE8> a owl:Class ;
    rdfs:label "Collective Agent"@en ;
    reg:lexicalAlias <http://iflastandards.info/ns/lrm/lrmerCollectiveAgent> ;
    reg:name "CollectiveAgent" ;
    reg:status <http://metadataregistry.org/uri/RegStatus/1001> ;
    rdfs:comment "The entity collective agent designates a wide range of named groups of persons that bear a particular name and have the potential of acting together as a unit. In addition to families, commercial or corporate entities and other legally registered bodies, the entity collective agent includes organizations and associations, musical, artistic or performing groups, governments, and any of their sub-units. The membership of many types of collective agents will continue to evolve over time. Occasional groups and groups that are constituted as meetings, conferences, congresses, expeditions, exhibitions, festivals, fairs, etc., also fall under the definition of collective agent as long as they are identified by a particular name and can act as a unit. Joint pseudonyms or collective pseudonyms are nomens that refer to instances of the collective agent entity as the agent behind the identity consists of two or more persons bearing a particular name and acting as a unit, despite having chosen to be identified by a name culturally associated with individual persons. A gathering of people is considered a collective agent only when it exhibits organizational characteristics that permit them to perform actions that reflect agency with respect to instances of entities of bibliographic interest (such as approving a report, publishing the proceedings of a conference). These collective actions may be performed by representatives selected by the whole, rather than by all individual members acting together. Groups of persons that do not qualify as agents (for example, national, religious, cultural or ethnic groups, such as Italian-Canadians, or gatherings referred to by a general descriptive term instead of a particular name) are not instances of the entity collective agent. The essential distinction between a collective agent and a gathering of people which is not an instance of the entity collective agent, is that the name used by the instance of the entity must be a specific name and not just a generic description for the gathering. Families and corporate bodies are specific types of collective agents that may be relevant in a particular bibliographic application."@en ;
    rdfs:isDefinedBy lrmer: ;
    rdfs:subClassOf <http://iflastandards.info/ns/lrm/lrmerE6> ;
    owl:disjointWith <http://iflastandards.info/ns/lrm/lrmerE7> ;
    skos:definition "A gathering or organization of persons bearing a particular name and capable of acting as a unit"@en .

<http://iflastandards.info/ns/lrm/lrmerE10> a owl:Class ;
    rdfs:label "Place"@en ;
    reg:lexicalAlias <http://iflastandards.info/ns/lrm/lrmerPlace> ;
    reg:name "Place" ;
    reg:status <http://metadataregistry.org/uri/RegStatus/1001> ;
    rdfs:comment "The entity place, as relevant in a bibliographic context, is a cultural construction; it is the human identification of a geographic area or extent of space. Places are usually identified through a physical object (a geographical feature or a man-made object), or due to their relevance with regards to a particular agent (geopolitical entities such as countries, cities), or as the location of an event. The place as an extent of space is distinct from any governing bodies that exercise jurisdiction in that territory. The government responsible for a territory is a collective agent. Places can be contemporary or historical, on Earth or extra-terrestrial. Imaginary, legendary or fictional places are not instances of the place entity. A place can have fuzzy boundaries. The boundaries of a place can change over time (such as a city that absorbs adjacent suburbs) without changing the identity of the place for bibliographic purposes. As it can be a moving frame of reference, the entity place is not necessarily identified by its geospatial coordinates alone."@en ;
    rdfs:isDefinedBy lrmer: ;
    rdfs:subClassOf <http://iflastandards.info/ns/lrm/lrmerE1> ;
    owl:disjointWith <http://iflastandards.info/ns/lrm/lrmerE11>,
        <http://iflastandards.info/ns/lrm/lrmerE2>,
        <http://iflastandards.info/ns/lrm/lrmerE3>,
        <http://iflastandards.info/ns/lrm/lrmerE4>,
        <http://iflastandards.info/ns/lrm/lrmerE5>,
        <http://iflastandards.info/ns/lrm/lrmerE6>,
        <http://iflastandards.info/ns/lrm/lrmerE9> ;
    skos:definition "A given extent of space"@en .

<http://iflastandards.info/ns/lrm/lrmerE11> a owl:Class ;
    rdfs:label "Time-span"@en ;
    reg:lexicalAlias <http://iflastandards.info/ns/lrm/lrmerTime-span> ;
    reg:name "Time-span" ;
    reg:status <http://metadataregistry.org/uri/RegStatus/1001> ;
    rdfs:comment "A time-span is a period of time that can be identified by specifying its beginning and end. The resulting duration can be associated with actions or occurrences that happened during that period of time. Even a very precise time-span has a measurable duration, however brief it may be. In library implementations, the instances of time-span considered useful in bibliographic or authority data are often expressed in years (year of birth of a person, year of death of a person, year a corporate body ceased to exist, year of publication of a manifestation), even though the associated event took place during only a portion of the year. The information available to the cataloguer, or the inherent characteristics of the time-span being identified, will be reflected in the degree of precision used in recording of a temporal extent. For example, '14th century' may be sufficiently precise in recording the beginning of the Renaissance, while a decade may be more appropriate when identifying the beginning of a musical style. Dates serve as the appellations or nomens for time-spans in different calendar or time-keeping systems. Time-spans can also be referred to by more general terms, such as for ages, geological eras, or epochs."@en ;
    rdfs:isDefinedBy lrmer: ;
    rdfs:subClassOf <http://iflastandards.info/ns/lrm/lrmerE1> ;
    owl:disjointWith <http://iflastandards.info/ns/lrm/lrmerE10>,
        <http://iflastandards.info/ns/lrm/lrmerE2>,
        <http://iflastandards.info/ns/lrm/lrmerE3>,
        <http://iflastandards.info/ns/lrm/lrmerE4>,
        <http://iflastandards.info/ns/lrm/lrmerE5>,
        <http://iflastandards.info/ns/lrm/lrmerE6>,
        <http://iflastandards.info/ns/lrm/lrmerE9> ;
    skos:definition "A temporal extent having a beginning, an end and a duration"@en .

<http://iflastandards.info/ns/lrm/lrmerE5> a owl:Class ;
    rdfs:label "Item"@en ;
    reg:lexicalAlias <http://iflastandards.info/ns/lrm/lrmerItem> ;
    reg:name "Item" ;
    reg:status <http://metadataregistry.org/uri/RegStatus/1001> ;
    rdfs:comment "In terms of intellectual or artistic content and physical form, an item exemplifying a manifestation normally reflects all the characteristics that define the manifestation itself. An item is in many instances a single physical object, but in other cases, an item may consist of multiple physical pieces or objects. An item may be a part of a larger physical object, for example, when a file is stored on a disc which also contains other files, the portion of the disc holding the file is the physical carrier or item."@en ;
    rdfs:isDefinedBy lrmer: ;
    rdfs:subClassOf <http://iflastandards.info/ns/lrm/lrmerE1> ;
    owl:disjointWith <http://iflastandards.info/ns/lrm/lrmerE10>,
        <http://iflastandards.info/ns/lrm/lrmerE11>,
        <http://iflastandards.info/ns/lrm/lrmerE2>,
        <http://iflastandards.info/ns/lrm/lrmerE3>,
        <http://iflastandards.info/ns/lrm/lrmerE4>,
        <http://iflastandards.info/ns/lrm/lrmerE6>,
        <http://iflastandards.info/ns/lrm/lrmerE9> ;
    skos:definition "An object or objects carrying signs intended to convey intellectual or artistic content"@en .

<http://iflastandards.info/ns/lrm/lrmerE1> a owl:Class ;
    rdfs:label "Res"@en ;
    reg:lexicalAlias <http://iflastandards.info/ns/lrm/lrmerRes> ;
    reg:name "Res"@en ;
    reg:status <http://metadataregistry.org/uri/RegStatus/1001> ;
    rdfs:comment "Res (“thing” in Latin) is the top entity in the model. Res includes both material or physical things and concepts. Everything considered relevant to the bibliographic universe, which is the universe of discourse in this case, is included. Res is a superclass of all the other entities that are explicitly defined, as well as of any other entities not specifically labelled."@en ;
    rdfs:isDefinedBy lrmer: ;
    skos:definition "Any entity in the universe of discourse"@en .

<http://iflastandards.info/ns/lrm/lrmerE6> a owl:Class ;
    rdfs:label "Agent"@en ;
    reg:lexicalAlias <http://iflastandards.info/ns/lrm/lrmerAgent> ;
    reg:name "Agent" ;
    reg:status <http://metadataregistry.org/uri/RegStatus/1001> ;
    rdfs:comment "The entity agent is a superclass strictly equivalent to the union of the entities person and collective agent. It is defined to reduce redundancy in the model by providing a single entity to serve as the domain or range of certain relationships that apply to all specific types of agents. Being an agent requires having, or having had, the potential of intentional relationships with instances of entities of bibliographic interest (works, expressions, manifestations, items), whether that specific agent has ever done so or not. Human beings are directly or indirectly the motive force behind all such actions taken by all agents. Automatons (such as, weather recording devices, software translation programs, etc.), sometimes referred to as technological agents, are in this model viewed as tools used and set up by an actual agent."@en ;
    rdfs:isDefinedBy lrmer: ;
    rdfs:subClassOf <http://iflastandards.info/ns/lrm/lrmerE1> ;
    owl:disjointWith <http://iflastandards.info/ns/lrm/lrmerE10>,
        <http://iflastandards.info/ns/lrm/lrmerE11>,
        <http://iflastandards.info/ns/lrm/lrmerE2>,
        <http://iflastandards.info/ns/lrm/lrmerE3>,
        <http://iflastandards.info/ns/lrm/lrmerE4>,
        <http://iflastandards.info/ns/lrm/lrmerE5>,
        <http://iflastandards.info/ns/lrm/lrmerE9> ;
    skos:definition "An entity capable of deliberate actions, of being granted rights, and of being held accountable for its actions"@en .

<http://iflastandards.info/ns/lrm/lrmerE9> a owl:Class ;
    rdfs:label "Nomen"@en ;
    reg:lexicalAlias <http://iflastandards.info/ns/lrm/lrmerNomen> ;
    reg:name "Nomen" ;
    reg:status <http://metadataregistry.org/uri/RegStatus/1001> ;
    rdfs:comment "A nomen associates whatever appellation (i.e., combination of signs) is used to refer to an instance of any entity found in the bibliographic universe with that entity. Any entity referred to in the universe of discourse is named through at least one nomen. An arbitrary combination of signs or symbols cannot be regarded as an appellation or designation until it is associated with something in some context. In that sense, the nomen entity can be understood as the reification of a relationship between an instance of res and a string. The string itself does not constitute an instance of the nomen entity but is modelled as the value of the nomen string attribute of an instance of the nomen entity. Two instances of the nomen entity can have perfectly identical values for their nomen string attribute and yet remain distinct, as long as they either refer to distinct instances of the res entity, or have distinct values for one or more of their other attributes (while referring to the same instance of the res entity). A nomen associates a combination of signs with an instance of an entity on the basis of a cultural or linguistic convention: by associating a nomen string with a res, the nomen establishes a meaning that is not inherent in the nomen string itself. Depending on context of use, nomens having identical values for their nomen string attribute can involve instances of different entities in the real world even within the same language (polysemy and homonymy). Conversely, the same instance of an entity can be referred to through any number of nomens (synonymy). In the controlled environment of a bibliographic information system, though, synonymy is avoided and the nomen string attribute values of nomens would generally be disambiguated, so that each nomen string is associated with only one instance of the res entity within the specific scheme. The identity of a nomen is determined by the combination of the res it involves, the choice and order of the symbols used within its nomen string attribute, and the values of all of its other attributes. Variation in the symbols used (such as transliteration into another script) or variation in their ordering usually results in a different nomen, but variation in the visual representation of the symbols present in the nomen string attribute value (such as different fonts that may be used to present alpha-numeric or character strings) does not result in a different nomen string. Nomens are assigned and associated with instances of entities either formally (such as by bibliographic agencies) or informally through common usage. When nomens are assigned formally, the construction of the nomen string attribute value may follow predetermined rules. A nomen string attribute value may consist of components or parts. In this case, the corresponding nomen can be viewed as being derived from two or more pre-existing nomens, and this derivation process may be governed by rules (for example, the ordering of name-title access points for works, the citation order in a faceted classification scheme, or the order of subdivisions in a subject heading system). For example, a new nomen for a person may be derived by combining a pre-existing nomen for that person and a nomen for the time-span of that person’s lifetime; similarly, a new nomen for a work may be derived by combining a nomen for a person who authored that work, and a pre-existing nomen for that work."@en ;
    rdfs:isDefinedBy lrmer: ;
    rdfs:subClassOf <http://iflastandards.info/ns/lrm/lrmerE1> ;
    owl:disjointWith <http://iflastandards.info/ns/lrm/lrmerE10>,
        <http://iflastandards.info/ns/lrm/lrmerE11>,
        <http://iflastandards.info/ns/lrm/lrmerE2>,
        <http://iflastandards.info/ns/lrm/lrmerE3>,
        <http://iflastandards.info/ns/lrm/lrmerE4>,
        <http://iflastandards.info/ns/lrm/lrmerE5>,
        <http://iflastandards.info/ns/lrm/lrmerE6> ;
    skos:definition "An association between an entity and a designation that refers to it"@en .

<http://iflastandards.info/ns/lrm/lrmerE3> a owl:Class ;
    rdfs:label "Expression"@en ;
    reg:lexicalAlias <http://iflastandards.info/ns/lrm/lrmerExpression> ;
    reg:name "Expression" ;
    reg:status <http://metadataregistry.org/uri/RegStatus/1001> ;
    rdfs:comment "An expression is a distinct combination of signs of any form or nature (including visual, aural or gestural signs) intended to convey intellectual or artistic content and identifiable as such. The term “sign” is intended here in the meaning used in semiotics. An expression is an abstract entity distinct from the carriers used to record it. An expression is the specific intellectual or artistic form that a work takes each time it is “realized”. Expression encompasses, for example, the specific words, sentences, paragraphs, etc. that result from the realization of a work in the form of a text, or the particular sounds, phrasing, etc. resulting from the realization of a musical work. The boundaries of the entity expression are defined, however, so as to exclude incidental aspects of physical form, such as typeface and page layout for a text, unless, due to the nature of the work, these are integral to the intellectual or artistic realization of the work as such. An expression comes into existence simultaneously with the creation of its first manifestation, no expression can exist without there being (or there having been at some point in the past) at least one manifestation. The process of abstraction leading to the identification of the entity expression indicates that the intellectual or artistic content embodied in one manifestation is in fact the same, or substantially the same, as that embodied in another manifestation even though the physical embodiment may differ and differing attributes of the manifestations may obscure the fact that the content is similar in both. On a practical level, the degree to which bibliographic distinctions are made between variant expressions of a work will depend to some extent on the nature of the work itself, on the anticipated needs of users and on what the cataloguer can reasonably be expected to recognize from the instance of the manifestation being described. Variations within substantially the same expression (e.g., slight variations that can be noticed between two states of the same edition in the case of hand press production) would be ignored in most applications. However, for some applications of the model (e.g., comprehensive databases of early printed texts, complete listings of the states of prints), each variation may be viewed as a different expression. Inasmuch as the form of expression is an inherent characteristic of the expression, any change in form (e.g., from written notation to spoken word) results in a new expression. Similarly, changes in the intellectual conventions or instruments that are employed to express a work (e.g., translation of a textual work from one language to another) result in the production of a new expression. If a text is revised or modified, the resulting expression is considered to be a new expression of the work. Minor changes, such as corrections of spelling and punctuation, etc., may be considered as variations within the same expression. When an expression of a work is accompanied by augmentations, such as illustrations, notes, glosses, etc. that are not integral to the intellectual or artistic realization of the work, such augmentations are considered to be separate expressions of their own separate work(s). Such augmentations may, or may not, be considered significant enough to warrant distinct bibliographic identification."@en ;
    rdfs:isDefinedBy lrmer: ;
    rdfs:subClassOf <http://iflastandards.info/ns/lrm/lrmerE1> ;
    owl:disjointWith <http://iflastandards.info/ns/lrm/lrmerE10>,
        <http://iflastandards.info/ns/lrm/lrmerE11>,
        <http://iflastandards.info/ns/lrm/lrmerE2>,
        <http://iflastandards.info/ns/lrm/lrmerE4>,
        <http://iflastandards.info/ns/lrm/lrmerE5>,
        <http://iflastandards.info/ns/lrm/lrmerE6>,
        <http://iflastandards.info/ns/lrm/lrmerE9> ;
    skos:definition "A distinct combination of signs conveying intellectual or artistic content"@en .

<http://iflastandards.info/ns/lrm/lrmerE2> a owl:Class ;
    rdfs:label "Work"@en ;
    reg:lexicalAlias <http://iflastandards.info/ns/lrm/lrmerWork> ;
    reg:name "Work" ;
    reg:status <http://metadataregistry.org/uri/RegStatus/1001> ;
    rdfs:comment "A work is an abstract entity that permits the grouping of expressions that are considered functional equivalents or near equivalents. A work is a conceptual object, no single material object can be identified as the work. The essence of the work is the constellation of concepts and ideas that form the shared content of what we define to be expressions of the same work. A work is perceived through the identification of the commonality of content between and among various expressions. However, similarity of factual or thematic content alone is not enough to group several expressions as realizing the same instance of work. For example, two textbooks both presenting an introduction to calculus, or two oil paintings of the same view (even if painted by the same artist), would be considered distinct works if independent intellectual or artistic effort was involved in their creation. In the case of aggregating works and serial works, the essence of the work is the concept or plan for the selection, assembly and ordering of the expressions of other works to be embodied in the resulting aggregate manifestation. A work comes into existence simultaneously with the creation of its first expression, no work can exist without there being (or there having been at some point in the past) at least one expression of the work. A work can be recognized retrospectively from an examination of the individual realizations or expressions of the work. The work consists of the intellectual or artistic creation that lies behind all the various expressions of the work. As a result, the content identified with an instance of work can evolve as new expressions of it are created. Bibliographic and cultural conventions play a crucial role in determining the exact boundaries between similar instances of works. User needs are the basis for determining whether instances of expression are considered to belong to the same instance of work. When the majority of users, for most general purposes, would regard the expression instances as being intellectually equivalent, then these expressions are considered to be expressions of the same work. Generally, when a significant degree of independent intellectual or artistic effort is involved in the production of an expression, the result is viewed as a new work with a transformation relationship to the source work. Thus paraphrases, rewritings, adaptations for children, parodies, musical variations on a theme and free transcriptions of a musical composition are usually considered to represent new works. Similarly, adaptations of a work from one literary or art form to another (e.g., dramatizations, adaptations from one medium of the graphic arts to another, etc.) are considered to represent new works. Abstracts, digests and summaries are also considered to represent new works."@en ;
    rdfs:isDefinedBy lrmer: ;
    rdfs:subClassOf <http://iflastandards.info/ns/lrm/lrmerE1> ;
    owl:disjointWith <http://iflastandards.info/ns/lrm/lrmerE10>,
        <http://iflastandards.info/ns/lrm/lrmerE11>,
        <http://iflastandards.info/ns/lrm/lrmerE3>,
        <http://iflastandards.info/ns/lrm/lrmerE4>,
        <http://iflastandards.info/ns/lrm/lrmerE5>,
        <http://iflastandards.info/ns/lrm/lrmerE6>,
        <http://iflastandards.info/ns/lrm/lrmerE9> ;
    skos:definition "The intellectual or artistic content of a distinct creation"@en .

<http://iflastandards.info/ns/lrm/lrmerE4> a owl:Class ;
    rdfs:label "Manifestation"@en ;
    reg:lexicalAlias <http://iflastandards.info/ns/lrm/lrmerManifestation> ;
    reg:name "Manifestation" ;
    reg:status <http://metadataregistry.org/uri/RegStatus/1001> ;
    rdfs:comment "A manifestation results from the capture of one or more expressions onto a carrier or set of carriers. As an entity, manifestation represents the common characteristics shared by those carriers, in respect to both intellectual or artistic content and physical form. A manifestation is recognized from the common characteristics exhibited by the items resulting from the same production process. The specification of the production process is an intrinsic part of the manifestation. The production may be explicitly planned so as to take place over time, as, for example, in printing on demand. The production plan may involve aspects that are not under the direct control of the producer, such as the specific digital storage media onto which an online file is downloaded by different end-users. Whatever storage media is used, the downloaded files are instances of the same manifestation as the online file. Production processes cover the range from formal industrial processes to artisanal or artistic processes. A production process may result in a set of multiple items that are interchangeable for most purposes. The manifestation can be defined by the specific properties and attributes that any item belonging to that manifestation should portray. In other cases, such as for holograph manuscripts, many artisanal or artistic productions or reproductions for preservation purposes, the intention is that the production process result in a single, unique item. The manifestation in this case is the singleton set (a set with a single member) that captures the idea of the item in question. The boundaries between one manifestation and another are drawn on the basis of both intellectual or artistic content and physical form. When the production process involves changes in physical form, the resulting product is considered a new manifestation. Changes in physical form include changes affecting display characteristics that are incidental to the conception of the work (e.g., a change in typeface, size of font, page layout, etc.), changes in physical medium (e.g., a change from paper to microfilm as the medium of conveyance), and changes in the container (e.g., a change from cassette to cartridge as the container for a tape). Where the production process involves a publisher, producer, distributor, etc., and there are changes signalled in the product that are related to publication, marketing, etc. (e.g., a change in publisher, repackaging, etc.), the resulting product may be considered a new manifestation. Whenever the production process involves modifications, additions, deletions, etc. (other than minor changes to spelling, punctuation, etc.) that affect the intellectual or artistic content, the result is a new expression of the work which is embodied in a new manifestation. On a practical level, the degree to which distinctions between manifestations are accounted for in catalogues will depend to some extent on the anticipated needs of users and on the differences that the cataloguer can reasonably be expected to recognize. Certain minor variations or differences in packaging may not be considered bibliographically significant and will not warrant the recognition of a new manifestation. Changes that occur deliberately or inadvertently during the production process that affect the items result, strictly speaking, in a new manifestation of the same expression. A manifestation resulting from such a change may be identified as a particular “state” or “issue” of the publication. Changes that occur to an individual item after the production process is complete (damage, wear and tear, the loss of a page, repairs, rebinding into multiple volumes, etc.) are not considered to result in a new manifestation. That item is simply considered to be an exemplar of the manifestation that no longer fully reflects the original production plan. However, when multiple items from different manifestations are physically combined or joined (books or pamphlets bound together, audio tapes spliced together, etc.) the result is a new singleton manifestation."@en ;
    rdfs:isDefinedBy lrmer: ;
    rdfs:subClassOf <http://iflastandards.info/ns/lrm/lrmerE1> ;
    owl:disjointWith <http://iflastandards.info/ns/lrm/lrmerE10>,
        <http://iflastandards.info/ns/lrm/lrmerE11>,
        <http://iflastandards.info/ns/lrm/lrmerE2>,
        <http://iflastandards.info/ns/lrm/lrmerE3>,
        <http://iflastandards.info/ns/lrm/lrmerE5>,
        <http://iflastandards.info/ns/lrm/lrmerE6>,
        <http://iflastandards.info/ns/lrm/lrmerE9> ;
    skos:definition "A set of all carriers that are assumed to share the same characteristics as to intellectual or artistic content and aspects of physical form. That set is defined by both the overall content and the production plan for its carrier or carriers"@en .

<http://iflastandards.info/ns/lrm/lrmerR1> a rdf:Property ;
    rdfs:label "is associated with res"@en ;
    reg:lexicalAlias <http://iflastandards.info/ns/lrm/lrmerisAssociatedWithRes> ;
    reg:name "isAssociatedWithRes"@en ;
    reg:status <http://metadataregistry.org/uri/RegStatus/1001> ;
    rdfs:comment "This is a general relationship valid for all entities in the bibliographic universe. In general, specific refinements would be defined to carry more precise semantics."@en ;
    rdfs:domain <http://iflastandards.info/ns/lrm/lrmerE1> ;
    rdfs:isDefinedBy lrmer: ;
    rdfs:range <http://iflastandards.info/ns/lrm/lrmerE1> ;
    skos:definition "Relates two res that have an association of any kind"@en .

lrmer: dc:title "LRMer (IFLA Library Reference Model Entity Relationship)"@en ;
    skos:note """IFLA LRM is a high-level conceptual reference model developed within an entity-relationship modelling framework. It is the consolidation of the separately developed IFLA conceptual models: FRBR, FRAD, FRSAD.

IFLA LRM was developed to resolve inconsistencies between the three separate models. Every user task, entity, attribute and relationship from the original three models was examined, definitions had to be revised, but also some remodeling was required in order to develop a meaningful consolidation. The result is a single, streamlined, and logically consistent model that covers all aspects of bibliographic data and that at the same time brings the modelling up-to-date with current conceptual modelling practices.

IFLA LRM was designed to be used in linked data environments and to support and promote the use of bibliographic data in linked data environments.
"""@en ;
    foaf:homepage <https://www.ifla.org/publications/node/11412> .

<http://metadataregistry.org/uri/RegStatus/1001> a skos:Concept ;
    skos:prefLabel "Published"@en .

