@prefix rdf: <http://www.w3.org/1999/02/22-rdf-syntax-ns#> .
@prefix dc: <http://purl.org/dc/elements/1.1/> .
@prefix foaf: <http://xmlns.com/foaf/0.1/> .
@prefix lrmer: <http://iflastandards.info/ns/lrm/lrmer> .
@prefix owl: <http://www.w3.org/2002/07/owl#> .
@prefix rdfs: <http://www.w3.org/2000/01/rdf-schema#> .
@prefix reg: <http://metadataregistry.org/uri/profile/regap/> .
@prefix skos: <http://www.w3.org/2004/02/skos/core#> .

<http://iflastandards.info/ns/lrm/lrmer>
    dc:title "LRMer (IFLA Library Reference Model Entity Relationship)"@en ;
    skos:note """IFLA LRM is a high-level conceptual reference model developed within an entity-relationship modelling framework. It is the consolidation of the separately developed IFLA conceptual models: FRBR, FRAD, FRSAD.

IFLA LRM was developed to resolve inconsistencies between the three separate models. Every user task, entity, attribute and relationship from the original three models was examined, definitions had to be revised, but also some remodeling was required in order to develop a meaningful consolidation. The result is a single, streamlined, and logically consistent model that covers all aspects of bibliographic data and that at the same time brings the modelling up-to-date with current conceptual modelling practices.

IFLA LRM was designed to be used in linked data environments and to support and promote the use of bibliographic data in linked data environments.
"""@en ;
    foaf:homepage <https://www.ifla.org/publications/node/11412> .

lrmer:E1
    reg:lexicalAlias lrmer:Res ;
    reg:name "Res"@en ;
    reg:status <http://metadataregistry.org/uri/RegStatus/1001> ;
    a owl:Class ;
    rdfs:comment "Res (“thing” in Latin) is the top entity in the model. Res includes both material or physical things and concepts. Everything considered relevant to the bibliographic universe, which is the universe of discourse in this case, is included. Res is a superclass of all the other entities that are explicitly defined, as well as of any other entities not specifically labelled."@en ;
    rdfs:isDefinedBy <http://iflastandards.info/ns/lrm/lrmer> ;
    rdfs:label "Res"@en ;
    skos:definition "Any entity in the universe of discourse"@en .

lrmer:E10
    reg:lexicalAlias lrmer:Place ;
    reg:name "Place" ;
    reg:status <http://metadataregistry.org/uri/RegStatus/1001> ;
    a owl:Class ;
    rdfs:comment "The entity place, as relevant in a bibliographic context, is a cultural construction; it is the human identification of a geographic area or extent of space. Places are usually identified through a physical object (a geographical feature or a man-made object), or due to their relevance with regards to a particular agent (geopolitical entities such as countries, cities), or as the location of an event. The place as an extent of space is distinct from any governing bodies that exercise jurisdiction in that territory. The government responsible for a territory is a collective agent. Places can be contemporary or historical, on Earth or extra-terrestrial. Imaginary, legendary or fictional places are not instances of the place entity. A place can have fuzzy boundaries. The boundaries of a place can change over time (such as a city that absorbs adjacent suburbs) without changing the identity of the place for bibliographic purposes. As it can be a moving frame of reference, the entity place is not necessarily identified by its geospatial coordinates alone."@en ;
    rdfs:isDefinedBy <http://iflastandards.info/ns/lrm/lrmer> ;
    rdfs:label "Place"@en ;
    rdfs:subClassOf lrmer:E1 ;
    owl:disjointWith lrmer:E11, lrmer:E2, lrmer:E3, lrmer:E4, lrmer:E5, lrmer:E6, lrmer:E9 ;
    skos:definition "A given extent of space"@en .

lrmer:E10A1
    reg:lexicalAlias lrmer:hasCategoryOfPlace ;
    reg:name "hasCategoryOfPlace" ;
    reg:status <http://metadataregistry.org/uri/RegStatus/1001> ;
    a rdf:Property ;
    rdfs:domain lrmer:E10 ;
    rdfs:isDefinedBy <http://iflastandards.info/ns/lrm/lrmer> ;
    rdfs:label "has category of place"@en ;
    rdfs:subPropertyOf lrmer:E1A1 ;
    skos:definition "Relates a place to a type to which the place belongs"@en .

lrmer:E10A2
    reg:lexicalAlias lrmer:hasLocationOfPlace ;
    reg:name "hasLocationOfPlace" ;
    reg:status <http://metadataregistry.org/uri/RegStatus/1001> ;
    a rdf:Property ;
    rdfs:comment "The level of precision used can vary according to the context."@en ;
    rdfs:domain lrmer:E10 ;
    rdfs:isDefinedBy <http://iflastandards.info/ns/lrm/lrmer> ;
    rdfs:label "has location of place"@en ;
    skos:definition "Relates a place to a delimitation of the physical territory of the place"@en .

lrmer:E11
    reg:lexicalAlias lrmer:Time-span ;
    reg:name "Time-span" ;
    reg:status <http://metadataregistry.org/uri/RegStatus/1001> ;
    a owl:Class ;
    rdfs:comment "A time-span is a period of time that can be identified by specifying its beginning and end. The resulting duration can be associated with actions or occurrences that happened during that period of time. Even a very precise time-span has a measurable duration, however brief it may be. In library implementations, the instances of time-span considered useful in bibliographic or authority data are often expressed in years (year of birth of a person, year of death of a person, year a corporate body ceased to exist, year of publication of a manifestation), even though the associated event took place during only a portion of the year. The information available to the cataloguer, or the inherent characteristics of the time-span being identified, will be reflected in the degree of precision used in recording of a temporal extent. For example, '14th century' may be sufficiently precise in recording the beginning of the Renaissance, while a decade may be more appropriate when identifying the beginning of a musical style. Dates serve as the appellations or nomens for time-spans in different calendar or time-keeping systems. Time-spans can also be referred to by more general terms, such as for ages, geological eras, or epochs."@en ;
    rdfs:isDefinedBy <http://iflastandards.info/ns/lrm/lrmer> ;
    rdfs:label "Time-span"@en ;
    rdfs:subClassOf lrmer:E1 ;
    owl:disjointWith lrmer:E10, lrmer:E2, lrmer:E3, lrmer:E4, lrmer:E5, lrmer:E6, lrmer:E9 ;
    skos:definition "A temporal extent having a beginning, an end and a duration"@en .

lrmer:E11A1
    reg:lexicalAlias lrmer:hasBeginning ;
    reg:name "hasBeginning" ;
    reg:status <http://metadataregistry.org/uri/RegStatus/1001> ;
    a rdf:Property ;
    rdfs:comment "The level of precision used can vary according to the context."@en ;
    rdfs:domain lrmer:E11 ;
    rdfs:isDefinedBy <http://iflastandards.info/ns/lrm/lrmer> ;
    rdfs:label "has beginning"@en ;
    skos:definition "Relates a time-span to a value for the time at which the time-span started, expressed in a precise way in an authoritative external system to allow temporal positioning of events"@en .

lrmer:E11A2
    reg:lexicalAlias lrmer:hasEnding ;
    reg:name "hasEnding" ;
    reg:status <http://metadataregistry.org/uri/RegStatus/1001> ;
    a rdf:Property ;
    rdfs:comment "The level of precision used can vary according to the context."@en ;
    rdfs:domain lrmer:E11 ;
    rdfs:isDefinedBy <http://iflastandards.info/ns/lrm/lrmer> ;
    rdfs:label "has ending"@en ;
    skos:definition "Relates a time-span to a value for the time at which the time-span ended, expressed in a precise way in an authoritative external system to allow temporal positioning of events"@en .

lrmer:E1A1
    reg:lexicalAlias lrmer:hasCategoryOfRes ;
    reg:name "hasCategoryOfRes" ;
    reg:status <http://metadataregistry.org/uri/RegStatus/1001> ;
    a rdf:Property ;
    rdfs:domain lrmer:E1 ;
    rdfs:isDefinedBy <http://iflastandards.info/ns/lrm/lrmer> ;
    rdfs:label "has category of res"@en ;
    skos:definition "Relates a res to a type to which the res belongs"@en .

lrmer:E1A2
    reg:lexicalAlias lrmer:hasNote ;
    reg:name "hasNote" ;
    reg:status <http://metadataregistry.org/uri/RegStatus/1001> ;
    a rdf:Property ;
    rdfs:domain lrmer:E1 ;
    rdfs:isDefinedBy <http://iflastandards.info/ns/lrm/lrmer> ;
    rdfs:label "has note"@en ;
    skos:definition "Relates a res to any kind of information about a res that is not recorded through the use of specific attributes and/or relationships"@en .

lrmer:E2
    reg:lexicalAlias lrmer:Work ;
    reg:name "Work" ;
    reg:status <http://metadataregistry.org/uri/RegStatus/1001> ;
    a owl:Class ;
    rdfs:comment "A work is an abstract entity that permits the grouping of expressions that are considered functional equivalents or near equivalents. A work is a conceptual object, no single material object can be identified as the work. The essence of the work is the constellation of concepts and ideas that form the shared content of what we define to be expressions of the same work. A work is perceived through the identification of the commonality of content between and among various expressions. However, similarity of factual or thematic content alone is not enough to group several expressions as realizing the same instance of work. For example, two textbooks both presenting an introduction to calculus, or two oil paintings of the same view (even if painted by the same artist), would be considered distinct works if independent intellectual or artistic effort was involved in their creation. In the case of aggregating works and serial works, the essence of the work is the concept or plan for the selection, assembly and ordering of the expressions of other works to be embodied in the resulting aggregate manifestation. A work comes into existence simultaneously with the creation of its first expression, no work can exist without there being (or there having been at some point in the past) at least one expression of the work. A work can be recognized retrospectively from an examination of the individual realizations or expressions of the work. The work consists of the intellectual or artistic creation that lies behind all the various expressions of the work. As a result, the content identified with an instance of work can evolve as new expressions of it are created. Bibliographic and cultural conventions play a crucial role in determining the exact boundaries between similar instances of works. User needs are the basis for determining whether instances of expression are considered to belong to the same instance of work. When the majority of users, for most general purposes, would regard the expression instances as being intellectually equivalent, then these expressions are considered to be expressions of the same work. Generally, when a significant degree of independent intellectual or artistic effort is involved in the production of an expression, the result is viewed as a new work with a transformation relationship to the source work. Thus paraphrases, rewritings, adaptations for children, parodies, musical variations on a theme and free transcriptions of a musical composition are usually considered to represent new works. Similarly, adaptations of a work from one literary or art form to another (e.g., dramatizations, adaptations from one medium of the graphic arts to another, etc.) are considered to represent new works. Abstracts, digests and summaries are also considered to represent new works."@en ;
    rdfs:isDefinedBy <http://iflastandards.info/ns/lrm/lrmer> ;
    rdfs:label "Work"@en ;
    rdfs:subClassOf lrmer:E1 ;
    owl:disjointWith lrmer:E10, lrmer:E11, lrmer:E3, lrmer:E4, lrmer:E5, lrmer:E6, lrmer:E9 ;
    skos:definition "The intellectual or artistic content of a distinct creation"@en .

lrmer:E2A1
    reg:lexicalAlias lrmer:hasCategoryOfWork ;
    reg:name "hasCategoryOfWork" ;
    reg:status <http://metadataregistry.org/uri/RegStatus/1001> ;
    a rdf:Property ;
    rdfs:comment "The category attribute can characterize a given work with regard to various categorizations: - categorization as to termination intention, - categorization as to creative domain, - categorization as to form / genre, - etc."@en ;
    rdfs:domain lrmer:E2 ;
    rdfs:isDefinedBy <http://iflastandards.info/ns/lrm/lrmer> ;
    rdfs:label "has category of work"@en ;
    rdfs:subPropertyOf lrmer:E1A1 ;
    skos:definition "Relates a work to a type to which the work belongs"@en .

lrmer:E2A2
    reg:lexicalAlias lrmer:hasRepresentativeExpressionAttribute ;
    reg:name "hasRepresentativeExpressionAttribute" ;
    reg:status <http://metadataregistry.org/uri/RegStatus/1001> ;
    a rdf:Property ;
    rdfs:comment "Generally, the representative expression attribute will be typed and the types chosen will vary depending on the context of use (as given by the cataloguing rules, the nature of catalogue, or the category of work). Each of the attributes chosen may itself be multivalued. The values of these attributes are inferred either from particular expressions considered to best represent the work, or from characteristics abstracted from a more or less nebulous network of similar expressions. There is no requirement to precisely identify an expression or expressions which serves as source for the values of the representative expression attributes, nor does that expression need to be recorded in the case where it is identified."@en ;
    rdfs:domain lrmer:E2 ;
    rdfs:isDefinedBy <http://iflastandards.info/ns/lrm/lrmer> ;
    rdfs:label "has representative expression attribute"@en ;
    skos:definition "Relates a work to an attribute which is deemed essential in characterizing the work and whose values are taken from a representative or canonical expression of the work"@en .

lrmer:E3
    reg:lexicalAlias lrmer:Expression ;
    reg:name "Expression" ;
    reg:status <http://metadataregistry.org/uri/RegStatus/1001> ;
    a owl:Class ;
    rdfs:comment "An expression is a distinct combination of signs of any form or nature (including visual, aural or gestural signs) intended to convey intellectual or artistic content and identifiable as such. The term “sign” is intended here in the meaning used in semiotics. An expression is an abstract entity distinct from the carriers used to record it. An expression is the specific intellectual or artistic form that a work takes each time it is “realized”. Expression encompasses, for example, the specific words, sentences, paragraphs, etc. that result from the realization of a work in the form of a text, or the particular sounds, phrasing, etc. resulting from the realization of a musical work. The boundaries of the entity expression are defined, however, so as to exclude incidental aspects of physical form, such as typeface and page layout for a text, unless, due to the nature of the work, these are integral to the intellectual or artistic realization of the work as such. An expression comes into existence simultaneously with the creation of its first manifestation, no expression can exist without there being (or there having been at some point in the past) at least one manifestation. The process of abstraction leading to the identification of the entity expression indicates that the intellectual or artistic content embodied in one manifestation is in fact the same, or substantially the same, as that embodied in another manifestation even though the physical embodiment may differ and differing attributes of the manifestations may obscure the fact that the content is similar in both. On a practical level, the degree to which bibliographic distinctions are made between variant expressions of a work will depend to some extent on the nature of the work itself, on the anticipated needs of users and on what the cataloguer can reasonably be expected to recognize from the instance of the manifestation being described. Variations within substantially the same expression (e.g., slight variations that can be noticed between two states of the same edition in the case of hand press production) would be ignored in most applications. However, for some applications of the model (e.g., comprehensive databases of early printed texts, complete listings of the states of prints), each variation may be viewed as a different expression. Inasmuch as the form of expression is an inherent characteristic of the expression, any change in form (e.g., from written notation to spoken word) results in a new expression. Similarly, changes in the intellectual conventions or instruments that are employed to express a work (e.g., translation of a textual work from one language to another) result in the production of a new expression. If a text is revised or modified, the resulting expression is considered to be a new expression of the work. Minor changes, such as corrections of spelling and punctuation, etc., may be considered as variations within the same expression. When an expression of a work is accompanied by augmentations, such as illustrations, notes, glosses, etc. that are not integral to the intellectual or artistic realization of the work, such augmentations are considered to be separate expressions of their own separate work(s). Such augmentations may, or may not, be considered significant enough to warrant distinct bibliographic identification."@en ;
    rdfs:isDefinedBy <http://iflastandards.info/ns/lrm/lrmer> ;
    rdfs:label "Expression"@en ;
    rdfs:subClassOf lrmer:E1 ;
    owl:disjointWith lrmer:E10, lrmer:E11, lrmer:E2, lrmer:E4, lrmer:E5, lrmer:E6, lrmer:E9 ;
    skos:definition "A distinct combination of signs conveying intellectual or artistic content"@en .

lrmer:E3A1
    reg:lexicalAlias lrmer:hasCategoryOfExpression ;
    reg:name "hasCategoryOfExpression" ;
    reg:status <http://metadataregistry.org/uri/RegStatus/1001> ;
    a rdf:Property ;
    rdfs:comment "The category attribute can characterize a given expression with regard to various categorizations: - content type, - state of development, - format of notated music, - etc."@en ;
    rdfs:domain lrmer:E3 ;
    rdfs:isDefinedBy <http://iflastandards.info/ns/lrm/lrmer> ;
    rdfs:label "has category of expression"@en ;
    rdfs:subPropertyOf lrmer:E1A1 ;
    skos:definition "Relates an expression to a type to which the expression belongs"@en .

lrmer:E3A2
    reg:lexicalAlias lrmer:hasExtentOfExpression ;
    reg:name "hasExtentOfExpression" ;
    reg:status <http://metadataregistry.org/uri/RegStatus/1001> ;
    a rdf:Property ;
    rdfs:comment "The value of the extent attribute consists of three elements: - a type of extent (e.g., length of text, envisioned duration of performance of musical notation, actual duration of recorded performance, etc.), - a number, - and a measurement unit (words, minutes, etc.). The type of extent and the measurement unit may be given implicitly. The level of precision used in recording the quantification of the extent may vary."@en ;
    rdfs:domain lrmer:E3 ;
    rdfs:isDefinedBy <http://iflastandards.info/ns/lrm/lrmer> ;
    rdfs:label "has extent of expression"@en ;
    skos:definition "Relates an expression to a quantification of the extent of the expression"@en .

lrmer:E3A3
    reg:lexicalAlias lrmer:hasIntendedAudienceOfExpression ;
    reg:name "hasIntendedAudienceOfExpression" ;
    reg:status <http://metadataregistry.org/uri/RegStatus/1001> ;
    a rdf:Property ;
    rdfs:comment "The intended audience attribute can characterize a given expression by indicating groups of end-users for which expressions with those features are deemed particularly appropriate: - categorization as to age group, - categorization as to sensory impairment, - categorization as to educational level, - categorization as to occupational group, - etc."@en ;
    rdfs:domain lrmer:E3 ;
    rdfs:isDefinedBy <http://iflastandards.info/ns/lrm/lrmer> ;
    rdfs:label "has intended audience of expression"@en ;
    skos:definition "Relates an expression to a class of users for which the expression is intended"@en .

lrmer:E3A4
    reg:lexicalAlias lrmer:hasUseRightsOfTheExpression ;
    reg:name "hasUseRightsOfTheExpression" ;
    reg:status <http://metadataregistry.org/uri/RegStatus/1001> ;
    a rdf:Property ;
    rdfs:domain lrmer:E3 ;
    rdfs:isDefinedBy <http://iflastandards.info/ns/lrm/lrmer> ;
    rdfs:label "has use rights of the expression"@en ;
    skos:definition "Relates an expression to a class of use restrictions to which the expression is submitted"@en .

lrmer:E3A5
    reg:lexicalAlias lrmer:hasCartographicScale ;
    reg:name "hasCartographicScale" ;
    reg:status <http://metadataregistry.org/uri/RegStatus/1001> ;
    a rdf:Property ;
    rdfs:comment "The cartographic scale attribute is specific to expressions of cartographic works. The cartographic scale attribute may apply to horizontal, vertical, angular, and/or other distances represented in the expression."@en ;
    rdfs:domain lrmer:E3 ;
    rdfs:isDefinedBy <http://iflastandards.info/ns/lrm/lrmer> ;
    rdfs:label "has cartographic scale"@en ;
    skos:definition "Relates an expression to a ratio of distances in a cartographic expression to the actual distances they represent"@en .

lrmer:E3A6
    reg:lexicalAlias lrmer:hasLanguageOfExpression ;
    reg:name "hasLanguageOfExpression" ;
    reg:status <http://metadataregistry.org/uri/RegStatus/1001> ;
    a rdf:Property ;
    rdfs:comment "The language attribute is specific to expressions consisting solely or partially of linguistic signs (either sonic or in notated form). The language attribute of the expression may include a number of languages, each pertaining to an individual component of the expression."@en ;
    rdfs:domain lrmer:E3 ;
    rdfs:isDefinedBy <http://iflastandards.info/ns/lrm/lrmer> ;
    rdfs:label "has language of expression"@en ;
    skos:definition "Relates an expression to a language used in the expression"@en .

lrmer:E3A7
    reg:lexicalAlias lrmer:hasKey ;
    reg:name "hasKey" ;
    reg:status <http://metadataregistry.org/uri/RegStatus/1001> ;
    a rdf:Property ;
    rdfs:comment "The key attribute is specific to expressions of musical works. The term “key” is broadly defined to encompass various musical traditions. This attribute is not restricted to Western art music."@en ;
    rdfs:domain lrmer:E3 ;
    rdfs:isDefinedBy <http://iflastandards.info/ns/lrm/lrmer> ;
    rdfs:label "has key"@en ;
    skos:definition "Relates an expression to a pitch structure (musical scale, ecclesiastic mode, raga, maqam, etc.), that characterizes the expression"@en .

lrmer:E3A8
    reg:lexicalAlias lrmer:hasMediumOfPerformance ;
    reg:name "hasMediumOfPerformance" ;
    reg:status <http://metadataregistry.org/uri/RegStatus/1001> ;
    a rdf:Property ;
    rdfs:comment "The medium of performance attribute is specific to expressions of musical works. The value of the medium of performance attribute includes at least one unit consisting of: - a number (implicit through the use of a singular noun, or explicitly stated), - and a type of performing tool (which may include: types of human voice tessitura, types of individual instruments, types of ensembles, etc.)."@en ;
    rdfs:domain lrmer:E3 ;
    rdfs:isDefinedBy <http://iflastandards.info/ns/lrm/lrmer> ;
    rdfs:label "has medium of performance"@en ;
    skos:definition "Relates an expression to a combination of performing tools (voices, instruments, ensembles, etc.) stated, intended, or actually used in the expression"@en .

lrmer:E4
    reg:lexicalAlias lrmer:Manifestation ;
    reg:name "Manifestation" ;
    reg:status <http://metadataregistry.org/uri/RegStatus/1001> ;
    a owl:Class ;
    rdfs:comment "A manifestation results from the capture of one or more expressions onto a carrier or set of carriers. As an entity, manifestation represents the common characteristics shared by those carriers, in respect to both intellectual or artistic content and physical form. A manifestation is recognized from the common characteristics exhibited by the items resulting from the same production process. The specification of the production process is an intrinsic part of the manifestation. The production may be explicitly planned so as to take place over time, as, for example, in printing on demand. The production plan may involve aspects that are not under the direct control of the producer, such as the specific digital storage media onto which an online file is downloaded by different end-users. Whatever storage media is used, the downloaded files are instances of the same manifestation as the online file. Production processes cover the range from formal industrial processes to artisanal or artistic processes. A production process may result in a set of multiple items that are interchangeable for most purposes. The manifestation can be defined by the specific properties and attributes that any item belonging to that manifestation should portray. In other cases, such as for holograph manuscripts, many artisanal or artistic productions or reproductions for preservation purposes, the intention is that the production process result in a single, unique item. The manifestation in this case is the singleton set (a set with a single member) that captures the idea of the item in question. The boundaries between one manifestation and another are drawn on the basis of both intellectual or artistic content and physical form. When the production process involves changes in physical form, the resulting product is considered a new manifestation. Changes in physical form include changes affecting display characteristics that are incidental to the conception of the work (e.g., a change in typeface, size of font, page layout, etc.), changes in physical medium (e.g., a change from paper to microfilm as the medium of conveyance), and changes in the container (e.g., a change from cassette to cartridge as the container for a tape). Where the production process involves a publisher, producer, distributor, etc., and there are changes signalled in the product that are related to publication, marketing, etc. (e.g., a change in publisher, repackaging, etc.), the resulting product may be considered a new manifestation. Whenever the production process involves modifications, additions, deletions, etc. (other than minor changes to spelling, punctuation, etc.) that affect the intellectual or artistic content, the result is a new expression of the work which is embodied in a new manifestation. On a practical level, the degree to which distinctions between manifestations are accounted for in catalogues will depend to some extent on the anticipated needs of users and on the differences that the cataloguer can reasonably be expected to recognize. Certain minor variations or differences in packaging may not be considered bibliographically significant and will not warrant the recognition of a new manifestation. Changes that occur deliberately or inadvertently during the production process that affect the items result, strictly speaking, in a new manifestation of the same expression. A manifestation resulting from such a change may be identified as a particular “state” or “issue” of the publication. Changes that occur to an individual item after the production process is complete (damage, wear and tear, the loss of a page, repairs, rebinding into multiple volumes, etc.) are not considered to result in a new manifestation. That item is simply considered to be an exemplar of the manifestation that no longer fully reflects the original production plan. However, when multiple items from different manifestations are physically combined or joined (books or pamphlets bound together, audio tapes spliced together, etc.) the result is a new singleton manifestation."@en ;
    rdfs:isDefinedBy <http://iflastandards.info/ns/lrm/lrmer> ;
    rdfs:label "Manifestation"@en ;
    rdfs:subClassOf lrmer:E1 ;
    owl:disjointWith lrmer:E10, lrmer:E11, lrmer:E2, lrmer:E3, lrmer:E5, lrmer:E6, lrmer:E9 ;
    skos:definition "A set of all carriers that are assumed to share the same characteristics as to intellectual or artistic content and aspects of physical form. That set is defined by both the overall content and the production plan for its carrier or carriers"@en .

lrmer:E4A1
    reg:lexicalAlias lrmer:hasCategoryOfCarrier ;
    reg:name "hasCategoryOfCarrier" ;
    reg:status <http://metadataregistry.org/uri/RegStatus/1001> ;
    a rdf:Property ;
    rdfs:comment "The category of carrier attribute can characterize a given manifestation with regard to various categorizations: - categorization as to general type of carrier (e.g., sheet), - categorization as to physical material employed in manufacturing the carriers (e.g., plastic), - categorization as to the physical material that is applied to the base material of the carriers (e.g., oil paint), - categorization as to the means used to record notation, sound, or images in the production of a manifestation (e.g., analogue), - etc. The carrier for a manifestation consisting of multiple physical components may include more than one form (e.g., a filmstrip with an accompanying booklet, a separate sound disc carrying the sound track for a film, etc.)."@en ;
    rdfs:domain lrmer:E4 ;
    rdfs:isDefinedBy <http://iflastandards.info/ns/lrm/lrmer> ;
    rdfs:label "has category of carrier"@en ;
    rdfs:subPropertyOf lrmer:E1A1 ;
    skos:definition "Relates a manifestation to a type of material to which all physical carriers of the manifestation are assumed to belong"@en .

lrmer:E4A2
    reg:lexicalAlias lrmer:hasExtentOfManifestation ;
    reg:name "hasExtentOfManifestation" ;
    reg:status <http://metadataregistry.org/uri/RegStatus/1001> ;
    a rdf:Property ;
    rdfs:comment "The value of the extent attribute consists of three elements: - a type of extent (e.g., numbering of physical units, height, width, diameter, etc.), - a number, - and a measurement unit (e.g., volumes, pages, sheets, discs, reels, etc.; cm, inches, etc.; Mb/Megabytes; etc.). The type of extent and the measurement unit may be given implicitly. The level of precision used in recording the quantification of the extent may vary."@en ;
    rdfs:domain lrmer:E4 ;
    rdfs:isDefinedBy <http://iflastandards.info/ns/lrm/lrmer> ;
    rdfs:label "has extent of manifestation"@en ;
    skos:definition "Relates a manifestation to a quantification of the extent observed on a physical carrier of the manifestation and assumed to be observable on all other physical carriers of the manifestation as well"@en .

lrmer:E4A3
    reg:lexicalAlias lrmer:hasIntendedAudienceOfManifestation ;
    reg:name "hasIntendedAudienceOfManifestation" ;
    reg:status <http://metadataregistry.org/uri/RegStatus/1001> ;
    a rdf:Property ;
    rdfs:comment "The intended audience attribute can characterize a given manifestation by indicating groups of end-users for which manifestations with those features are deemed particularly appropriate: - categorization as to sensory impairment (visual impairment, hearing impairment, etc.), - categorization as to specialized carriers for specific audiences (young children, etc.), - etc."@en ;
    rdfs:domain lrmer:E4 ;
    rdfs:isDefinedBy <http://iflastandards.info/ns/lrm/lrmer> ;
    rdfs:label "has intended audience of manifestation"@en ;
    skos:definition "Relates a manifestation to a class of users for which the physical carriers of the manifestation are intended"@en .

lrmer:E4A4
    reg:lexicalAlias lrmer:hasManifestationStatement ;
    reg:name "hasManifestationStatement" ;
    reg:status <http://metadataregistry.org/uri/RegStatus/1001> ;
    a rdf:Property ;
    rdfs:comment "The manifestation statement attribute is a statement that is usually transcribed from a source or sources present in exemplars of a manifestation. Transcription conventions are codified by each implementation. A manifestation is likely to be characterized by multiple statements of different types. In most implementations, these statements would likely be typed at a level of granularity considered appropriate for user needs. For example, the manifestation statement attribute may include transcribed elements such as: publication statement (as a whole), or alternatively, place of publication statement + publisher name statement + date of publication statement (as three individual statements)."@en ;
    rdfs:domain lrmer:E4 ;
    rdfs:isDefinedBy <http://iflastandards.info/ns/lrm/lrmer> ;
    rdfs:label "has manifestation statement"@en ;
    skos:definition "Relates a manifestation to a statement appearing in exemplars of the manifestation and deemed to be significant for users to understand how the resource represents itself"@en .

lrmer:E4A5
    reg:lexicalAlias lrmer:hasAccessConditions ;
    reg:name "hasAccessConditions" ;
    reg:status <http://metadataregistry.org/uri/RegStatus/1001> ;
    a rdf:Property ;
    rdfs:comment "The access conditions attribute includes: - System requirements, - Mode of access, - etc."@en ;
    rdfs:domain lrmer:E4 ;
    rdfs:isDefinedBy <http://iflastandards.info/ns/lrm/lrmer> ;
    rdfs:label "has access conditions"@en ;
    skos:definition "Relates a manifestation to information as to how any of the carriers of the manifestation are likely to be obtained"@en .

lrmer:E4A6
    reg:lexicalAlias lrmer:hasUseRightsOfTheManifestation ;
    reg:name "hasUseRightsOfTheManifestation" ;
    reg:status <http://metadataregistry.org/uri/RegStatus/1001> ;
    a rdf:Property ;
    rdfs:comment "The use rights attribute includes: - Terms of availability, - Access restrictions, - etc."@en ;
    rdfs:domain lrmer:E4 ;
    rdfs:isDefinedBy <http://iflastandards.info/ns/lrm/lrmer> ;
    rdfs:label "has use rights of the manifestation"@en ;
    skos:definition "Relates a manifestation to a class of use and/or access restrictions to which all carriers of the manifestation are assumed to be submitted"@en .

lrmer:E5
    reg:lexicalAlias lrmer:Item ;
    reg:name "Item" ;
    reg:status <http://metadataregistry.org/uri/RegStatus/1001> ;
    a owl:Class ;
    rdfs:comment "In terms of intellectual or artistic content and physical form, an item exemplifying a manifestation normally reflects all the characteristics that define the manifestation itself. An item is in many instances a single physical object, but in other cases, an item may consist of multiple physical pieces or objects. An item may be a part of a larger physical object, for example, when a file is stored on a disc which also contains other files, the portion of the disc holding the file is the physical carrier or item."@en ;
    rdfs:isDefinedBy <http://iflastandards.info/ns/lrm/lrmer> ;
    rdfs:label "Item"@en ;
    rdfs:subClassOf lrmer:E1 ;
    owl:disjointWith lrmer:E10, lrmer:E11, lrmer:E2, lrmer:E3, lrmer:E4, lrmer:E6, lrmer:E9 ;
    skos:definition "An object or objects carrying signs intended to convey intellectual or artistic content"@en .

lrmer:E5A1
    reg:lexicalAlias lrmer:hasLocationOfItem ;
    reg:name "hasLocationOfItem" ;
    reg:status <http://metadataregistry.org/uri/RegStatus/1001> ;
    a rdf:Property ;
    rdfs:comment "This information can be specified at whatever level of precision is required in order to guide end-users in obtaining the item."@en ;
    rdfs:domain lrmer:E5 ;
    rdfs:isDefinedBy <http://iflastandards.info/ns/lrm/lrmer> ;
    rdfs:label "has location of item"@en ;
    skos:definition "Relates an item to the collection and/or institution in which the item is held, stored, or made available for access"@en .

lrmer:E5A2
    reg:lexicalAlias lrmer:hasUseRightsOfTheItem ;
    reg:name "hasUseRightsOfTheItem" ;
    reg:status <http://metadataregistry.org/uri/RegStatus/1001> ;
    a rdf:Property ;
    rdfs:domain lrmer:E5 ;
    rdfs:isDefinedBy <http://iflastandards.info/ns/lrm/lrmer> ;
    rdfs:label "has use rights of the item"@en ;
    skos:definition "Relates an item to a class of use and/or access restrictions to which the item is submitted"@en .

lrmer:E6
    reg:lexicalAlias lrmer:Agent ;
    reg:name "Agent" ;
    reg:status <http://metadataregistry.org/uri/RegStatus/1001> ;
    a owl:Class ;
    rdfs:comment "The entity agent is a superclass strictly equivalent to the union of the entities person and collective agent. It is defined to reduce redundancy in the model by providing a single entity to serve as the domain or range of certain relationships that apply to all specific types of agents. Being an agent requires having, or having had, the potential of intentional relationships with instances of entities of bibliographic interest (works, expressions, manifestations, items), whether that specific agent has ever done so or not. Human beings are directly or indirectly the motive force behind all such actions taken by all agents. Automatons (such as, weather recording devices, software translation programs, etc.), sometimes referred to as technological agents, are in this model viewed as tools used and set up by an actual agent."@en ;
    rdfs:isDefinedBy <http://iflastandards.info/ns/lrm/lrmer> ;
    rdfs:label "Agent"@en ;
    rdfs:subClassOf lrmer:E1 ;
    owl:disjointWith lrmer:E10, lrmer:E11, lrmer:E2, lrmer:E3, lrmer:E4, lrmer:E5, lrmer:E9 ;
    skos:definition "An entity capable of deliberate actions, of being granted rights, and of being held accountable for its actions"@en .

lrmer:E6A1
    reg:lexicalAlias lrmer:hasContactInformation ;
    reg:name "hasContactInformation" ;
    reg:status <http://metadataregistry.org/uri/RegStatus/1001> ;
    a rdf:Property ;
    rdfs:domain lrmer:E6 ;
    rdfs:isDefinedBy <http://iflastandards.info/ns/lrm/lrmer> ;
    rdfs:label "has contact information"@en ;
    skos:definition "Relates an agent to information useful for communicating with or getting in contact with the agent"@en .

lrmer:E6A2
    reg:lexicalAlias lrmer:hasFieldOfActivity ;
    reg:name "hasFieldOfActivity" ;
    reg:status <http://metadataregistry.org/uri/RegStatus/1001> ;
    a rdf:Property ;
    rdfs:domain lrmer:E6 ;
    rdfs:isDefinedBy <http://iflastandards.info/ns/lrm/lrmer> ;
    rdfs:label "has field of activity"@en ;
    skos:definition "Relates an agent to a field of endeavour, area of expertise, etc., in which the agent is engaged or was engaged"@en .

lrmer:E6A3
    reg:lexicalAlias lrmer:hasLanguageOfAgent ;
    reg:name "hasLanguageOfAgent" ;
    reg:status <http://metadataregistry.org/uri/RegStatus/1001> ;
    a rdf:Property ;
    rdfs:comment "A given agent can use more than one language, simultaneously or over time. The type of use of a given language can be specified (e.g., use of the English language for the creation of original content, use of the English language as source language of translations, etc.)."@en ;
    rdfs:domain lrmer:E6 ;
    rdfs:isDefinedBy <http://iflastandards.info/ns/lrm/lrmer> ;
    rdfs:label "has language of agent"@en ;
    skos:definition "Relates an agent to a language used by the agent when creating an expression"@en .

lrmer:E7
    reg:lexicalAlias lrmer:Person ;
    reg:name "Person" ;
    reg:status <http://metadataregistry.org/uri/RegStatus/1001> ;
    a owl:Class ;
    rdfs:comment "The entity person is restricted to real persons who live or are assumed to have lived. Strict proof of the existence of a person is not required, as long as there is a general acceptance of their probable historicity. However, figures generally considered fictional (for example, Kermit the Frog), literary (for example, Miss Jane Marple) or purely legendary (for example, the wizard Merlin) are not instances of the entity person."@en ;
    rdfs:isDefinedBy <http://iflastandards.info/ns/lrm/lrmer> ;
    rdfs:label "Person"@en ;
    rdfs:subClassOf lrmer:E6 ;
    owl:disjointWith lrmer:E8 ;
    skos:definition "An individual human being"@en .

lrmer:E7A1
    reg:lexicalAlias lrmer:hasProfessionOrOccupation ;
    reg:name "hasProfessionOrOccupation" ;
    reg:status <http://metadataregistry.org/uri/RegStatus/1001> ;
    a rdf:Property ;
    rdfs:domain lrmer:E7 ;
    rdfs:isDefinedBy <http://iflastandards.info/ns/lrm/lrmer> ;
    rdfs:label "has profession or occupation"@en ;
    skos:definition "Relates a person to a profession or occupation in which the person works or worked"@en ;
    skos:scopeNote "Source documentation has \"profession / occupation\"; slash character replaced with \"or\" to improve clarity."@en .

lrmer:E8
    reg:lexicalAlias lrmer:CollectiveAgent ;
    reg:name "CollectiveAgent" ;
    reg:status <http://metadataregistry.org/uri/RegStatus/1001> ;
    a owl:Class ;
    rdfs:comment "The entity collective agent designates a wide range of named groups of persons that bear a particular name and have the potential of acting together as a unit. In addition to families, commercial or corporate entities and other legally registered bodies, the entity collective agent includes organizations and associations, musical, artistic or performing groups, governments, and any of their sub-units. The membership of many types of collective agents will continue to evolve over time. Occasional groups and groups that are constituted as meetings, conferences, congresses, expeditions, exhibitions, festivals, fairs, etc., also fall under the definition of collective agent as long as they are identified by a particular name and can act as a unit. Joint pseudonyms or collective pseudonyms are nomens that refer to instances of the collective agent entity as the agent behind the identity consists of two or more persons bearing a particular name and acting as a unit, despite having chosen to be identified by a name culturally associated with individual persons. A gathering of people is considered a collective agent only when it exhibits organizational characteristics that permit them to perform actions that reflect agency with respect to instances of entities of bibliographic interest (such as approving a report, publishing the proceedings of a conference). These collective actions may be performed by representatives selected by the whole, rather than by all individual members acting together. Groups of persons that do not qualify as agents (for example, national, religious, cultural or ethnic groups, such as Italian-Canadians, or gatherings referred to by a general descriptive term instead of a particular name) are not instances of the entity collective agent. The essential distinction between a collective agent and a gathering of people which is not an instance of the entity collective agent, is that the name used by the instance of the entity must be a specific name and not just a generic description for the gathering. Families and corporate bodies are specific types of collective agents that may be relevant in a particular bibliographic application."@en ;
    rdfs:isDefinedBy <http://iflastandards.info/ns/lrm/lrmer> ;
    rdfs:label "Collective Agent"@en ;
    rdfs:subClassOf lrmer:E6 ;
    owl:disjointWith lrmer:E7 ;
    skos:definition "A gathering or organization of persons bearing a particular name and capable of acting as a unit"@en .

lrmer:E9
    reg:lexicalAlias lrmer:Nomen ;
    reg:name "Nomen" ;
    reg:status <http://metadataregistry.org/uri/RegStatus/1001> ;
    a owl:Class ;
    rdfs:comment "A nomen associates whatever appellation (i.e., combination of signs) is used to refer to an instance of any entity found in the bibliographic universe with that entity. Any entity referred to in the universe of discourse is named through at least one nomen. An arbitrary combination of signs or symbols cannot be regarded as an appellation or designation until it is associated with something in some context. In that sense, the nomen entity can be understood as the reification of a relationship between an instance of res and a string. The string itself does not constitute an instance of the nomen entity but is modelled as the value of the nomen string attribute of an instance of the nomen entity. Two instances of the nomen entity can have perfectly identical values for their nomen string attribute and yet remain distinct, as long as they either refer to distinct instances of the res entity, or have distinct values for one or more of their other attributes (while referring to the same instance of the res entity). A nomen associates a combination of signs with an instance of an entity on the basis of a cultural or linguistic convention: by associating a nomen string with a res, the nomen establishes a meaning that is not inherent in the nomen string itself. Depending on context of use, nomens having identical values for their nomen string attribute can involve instances of different entities in the real world even within the same language (polysemy and homonymy). Conversely, the same instance of an entity can be referred to through any number of nomens (synonymy). In the controlled environment of a bibliographic information system, though, synonymy is avoided and the nomen string attribute values of nomens would generally be disambiguated, so that each nomen string is associated with only one instance of the res entity within the specific scheme. The identity of a nomen is determined by the combination of the res it involves, the choice and order of the symbols used within its nomen string attribute, and the values of all of its other attributes. Variation in the symbols used (such as transliteration into another script) or variation in their ordering usually results in a different nomen, but variation in the visual representation of the symbols present in the nomen string attribute value (such as different fonts that may be used to present alpha-numeric or character strings) does not result in a different nomen string. Nomens are assigned and associated with instances of entities either formally (such as by bibliographic agencies) or informally through common usage. When nomens are assigned formally, the construction of the nomen string attribute value may follow predetermined rules. A nomen string attribute value may consist of components or parts. In this case, the corresponding nomen can be viewed as being derived from two or more pre-existing nomens, and this derivation process may be governed by rules (for example, the ordering of name-title access points for works, the citation order in a faceted classification scheme, or the order of subdivisions in a subject heading system). For example, a new nomen for a person may be derived by combining a pre-existing nomen for that person and a nomen for the time-span of that person’s lifetime; similarly, a new nomen for a work may be derived by combining a nomen for a person who authored that work, and a pre-existing nomen for that work."@en ;
    rdfs:isDefinedBy <http://iflastandards.info/ns/lrm/lrmer> ;
    rdfs:label "Nomen"@en ;
    rdfs:subClassOf lrmer:E1 ;
    owl:disjointWith lrmer:E10, lrmer:E11, lrmer:E2, lrmer:E3, lrmer:E4, lrmer:E5, lrmer:E6 ;
    skos:definition "An association between an entity and a designation that refers to it"@en .

lrmer:E9A1
    reg:lexicalAlias lrmer:hasCategoryOfNomen ;
    reg:name "hasCategoryOfNomen" ;
    reg:status <http://metadataregistry.org/uri/RegStatus/1001> ;
    a rdf:Property ;
    rdfs:comment "Nomens may be categorized in terms of: - the type of thing named (personal name, work title, etc.), - the source in which the nomen is attested (spine title, running title), - the function of the nomen (identifier, controlled access point, classification notation, etc.)."@en ;
    rdfs:domain lrmer:E9 ;
    rdfs:isDefinedBy <http://iflastandards.info/ns/lrm/lrmer> ;
    rdfs:label "has category of nomen"@en ;
    rdfs:subPropertyOf lrmer:E1A1 ;
    skos:definition "Relates a nomen to a type to which the nomen belongs"@en .

lrmer:E9A2
    reg:lexicalAlias lrmer:hasNomenString ;
    reg:name "hasNomenString" ;
    reg:status <http://metadataregistry.org/uri/RegStatus/1001> ;
    a rdf:Property ;
    rdfs:comment "The string involved in a nomen can be expressed as a notation in any form, such as a combination of signs within a writing system, chemical structure symbols, mathematical notation, or by any other kind of sign, such as sounds, etc. A nomen is more than the mere string of signs that constitutes the appellation associated with a thing through the nomen. Without any contextualization, the value of the nomen string attribute is a mere literal, potentially attached to anything in the world, as opposed to the nomen itself, which as a result of the appellation relationship is attached to one and only one instance of res. For example, the nomen 'John Smith' is the appellation of one and only one John Smith in the world, while the value of the nomen string attribute that reads \"John Smith\" in the Latin alphabet is the same for all the different things in the world that happen to be named 'John Smith'."@en ;
    rdfs:domain lrmer:E9 ;
    rdfs:isDefinedBy <http://iflastandards.info/ns/lrm/lrmer> ;
    rdfs:label "has nomen string"@en ;
    skos:definition "Relates a nomen to the combination of signs that forms an appellation associated with an entity through the nomen"@en .

lrmer:E9A3
    reg:lexicalAlias lrmer:hasScheme ;
    reg:name "hasScheme" ;
    reg:status <http://metadataregistry.org/uri/RegStatus/1001> ;
    a rdf:Property ;
    rdfs:comment "The scheme attribute includes: - value encoding schemes (subject heading lists, thesauri, classification systems, name authority lists, etc.) - and syntax encoding schemes (standards for encoding dates, etc.). When the same value of one of the other nomen attributes (such as intended audience, language, script) is applicable to all the nomens in a particular scheme, the value can be implemented at the scheme level."@en ;
    rdfs:domain lrmer:E9 ;
    rdfs:isDefinedBy <http://iflastandards.info/ns/lrm/lrmer> ;
    rdfs:label "has scheme"@en ;
    skos:definition "Relates a nomen to the scheme in which the nomen is established"@en .

lrmer:E9A4
    reg:lexicalAlias lrmer:hasIntendedAudienceOfNomen ;
    reg:name "hasIntendedAudienceOfNomen" ;
    reg:status <http://metadataregistry.org/uri/RegStatus/1001> ;
    a rdf:Property ;
    rdfs:comment "Indicating the intended audience for a nomen can serve as a basis for a mechanism that selects a nomen from a cluster of equivalent nomens, for use in a particular context. For example, an international multi-lingual authority file can indicate the intended audience for each nomen by recording the language in which the nomen is a preferred form."@en ;
    rdfs:domain lrmer:E9 ;
    rdfs:isDefinedBy <http://iflastandards.info/ns/lrm/lrmer> ;
    rdfs:label "has intended audience of nomen"@en ;
    skos:definition "Relates a nomen to a class of users for which the nomen is considered appropriate or preferred"@en .

lrmer:E9A5
    reg:lexicalAlias lrmer:hasContextOfUse ;
    reg:name "hasContextOfUse" ;
    reg:status <http://metadataregistry.org/uri/RegStatus/1001> ;
    a rdf:Property ;
    rdfs:comment "The context of use attribute includes domains associated with a nomen used by an agent."@en ;
    rdfs:domain lrmer:E9 ;
    rdfs:isDefinedBy <http://iflastandards.info/ns/lrm/lrmer> ;
    rdfs:label "has context of use"@en ;
    skos:definition "Relates a nomen to information as to the context(s) in which a nomen is used by the agent who is referred to through it"@en .

lrmer:E9A6
    reg:lexicalAlias lrmer:hasReferenceSource ;
    reg:name "hasReferenceSource" ;
    reg:status <http://metadataregistry.org/uri/RegStatus/1001> ;
    a rdf:Property ;
    rdfs:comment "A reference source attests to the existence of a linkage between a designation and the instance of the entity res that it serves to identify. It may clarify the validity and scope of the nomen. A reference source attribute value may refer to: - biographical dictionaries, encyclopedias, etc., - other schemes, - any publications, - etc."@en ;
    rdfs:domain lrmer:E9 ;
    rdfs:isDefinedBy <http://iflastandards.info/ns/lrm/lrmer> ;
    rdfs:label "has reference source"@en ;
    skos:definition "Relates a nomen to a source in which there is evidence for the use of the nomen"@en .

lrmer:E9A7
    reg:lexicalAlias lrmer:hasLanguageOfNomen ;
    reg:name "hasLanguageOfNomen" ;
    reg:status <http://metadataregistry.org/uri/RegStatus/1001> ;
    a rdf:Property ;
    rdfs:comment "The language attribute may be viewed as recording a scheme of a particular type (that is, a natural human language) in which a nomen may be considered valid. Viewed in this way, the language attribute may be implemented as a sub-type of the scheme attribute."@en ;
    rdfs:domain lrmer:E9 ;
    rdfs:isDefinedBy <http://iflastandards.info/ns/lrm/lrmer> ;
    rdfs:label "has language of nomen"@en ;
    skos:definition "Relates a nomen to the language in which the nomen is attested"@en .

lrmer:E9A8
    reg:lexicalAlias lrmer:hasScript ;
    reg:name "hasScript" ;
    reg:status <http://metadataregistry.org/uri/RegStatus/1001> ;
    a rdf:Property ;
    rdfs:comment "The script attribute allows the identification of the writing system used to provide a notation for the nomen. The writing system consists of the full range of the conventions used. Writing systems may be alphabetic, syllabic, ideographic, etc., or some combination of these. The script does not, however, include aspects such as the choice of font or other incidental display characteristics (for example, point size, colour) which do not encode any features which result in differences in the interpretation of the written symbols."@en ;
    rdfs:domain lrmer:E9 ;
    rdfs:isDefinedBy <http://iflastandards.info/ns/lrm/lrmer> ;
    rdfs:label "has script"@en ;
    skos:definition "Relates a nomen to the script in which the nomen is notated"@en .

lrmer:E9A9
    reg:lexicalAlias lrmer:hasScriptConversion ;
    reg:name "hasScriptConversion" ;
    reg:status <http://metadataregistry.org/uri/RegStatus/1001> ;
    a rdf:Property ;
    rdfs:comment "A script conversion attribute value may refer to: - transliterations, - script conversions that cannot be reversed, - etc."@en ;
    rdfs:domain lrmer:E9 ;
    rdfs:isDefinedBy <http://iflastandards.info/ns/lrm/lrmer> ;
    rdfs:label "has script conversion"@en ;
    skos:definition "Relates a nomen to the rule, system, or standard that was used to create a nomen that is derived on the basis of another, distinct nomen notated in another, distinct script"@en .

lrmer:R1
    reg:lexicalAlias lrmer:isAssociatedWithRes ;
    reg:name "isAssociatedWithRes"@en ;
    reg:status <http://metadataregistry.org/uri/RegStatus/1001> ;
    a rdf:Property ;
    rdfs:comment "This is a general relationship valid for all entities in the bibliographic universe. In general, specific refinements would be defined to carry more precise semantics."@en ;
    rdfs:domain lrmer:E1 ;
    rdfs:isDefinedBy <http://iflastandards.info/ns/lrm/lrmer> ;
    rdfs:label "is associated with res"@en ;
    rdfs:range lrmer:E1 ;
    skos:definition "Relates two res that have an association of any kind"@en .

lrmer:R10
    reg:lexicalAlias lrmer:isOwnedBy ;
    reg:name "isOwnedBy" ;
    reg:status <http://metadataregistry.org/uri/RegStatus/1001> ;
    a rdf:Property ;
    rdfs:comment "The logical connection between an item and a related agent could serve as the basis both for identifying an agent that owned or had custodianship of an item and for ensuring that all items owned by, or in the custodianship of, a particular agent are linked to that agent."@en ;
    rdfs:domain lrmer:E5 ;
    rdfs:isDefinedBy <http://iflastandards.info/ns/lrm/lrmer> ;
    rdfs:label "is owned by"@en ;
    rdfs:range lrmer:E6 ;
    rdfs:subPropertyOf lrmer:R1 ;
    owl:inverseOf lrmer:R10i ;
    skos:definition "Relates an item to an agent that is or was the owner or custodian of that item"@en .

lrmer:R10i
    reg:lexicalAlias lrmer:owns ;
    reg:name "owns" ;
    reg:status <http://metadataregistry.org/uri/RegStatus/1001> ;
    a rdf:Property ;
    rdfs:comment "The logical connection between an item and a related agent could serve as the basis both for identifying an agent that owned or had custodianship of an item and for ensuring that all items owned by, or in the custodianship of, a particular agent are linked to that agent."@en ;
    rdfs:domain lrmer:E6 ;
    rdfs:isDefinedBy <http://iflastandards.info/ns/lrm/lrmer> ;
    rdfs:label "owns"@en ;
    rdfs:range lrmer:E5 ;
    rdfs:subPropertyOf lrmer:R1 ;
    owl:inverseOf lrmer:R10 ;
    skos:definition "Relates an agent to an item that is or was owned or in the custody of that agent"@en .

lrmer:R11
    reg:lexicalAlias lrmer:wasModifiedBy ;
    reg:name "wasModifiedBy" ;
    reg:status <http://metadataregistry.org/uri/RegStatus/1001> ;
    a rdf:Property ;
    rdfs:comment "Examples include adding annotations, adding an ex-libris, removing pages, rebinding, restoration."@en ;
    rdfs:domain lrmer:E5 ;
    rdfs:isDefinedBy <http://iflastandards.info/ns/lrm/lrmer> ;
    rdfs:label "was modified by"@en ;
    rdfs:range lrmer:E6 ;
    rdfs:subPropertyOf lrmer:R1 ;
    owl:inverseOf lrmer:R11i ;
    skos:definition "Relates an item to an agent that made changes to this particular item without creating a new manifestation"@en .

lrmer:R11i
    reg:lexicalAlias lrmer:modified ;
    reg:name "modified" ;
    reg:status <http://metadataregistry.org/uri/RegStatus/1001> ;
    a rdf:Property ;
    rdfs:comment "Examples include adding annotations, adding an ex-libris, removing pages, rebinding, restoration."@en ;
    rdfs:domain lrmer:E6 ;
    rdfs:isDefinedBy <http://iflastandards.info/ns/lrm/lrmer> ;
    rdfs:label "modified"@en ;
    rdfs:range lrmer:E5 ;
    rdfs:subPropertyOf lrmer:R1 ;
    owl:inverseOf lrmer:R11 ;
    skos:definition "Relates an agent to an item that the agent made changes to without creating a new manifestation"@en .

lrmer:R12
    reg:lexicalAlias lrmer:hasAsSubject ;
    reg:name "hasAsSubject" ;
    reg:status <http://metadataregistry.org/uri/RegStatus/1001> ;
    a rdf:Property ;
    rdfs:comment "The logical connection between a work and a related subject entity serves as the basis both for identifying the subject of an individual work and for ensuring that all works relevant to a given subject are linked to that subject."@en ;
    rdfs:domain lrmer:E2 ;
    rdfs:isDefinedBy <http://iflastandards.info/ns/lrm/lrmer> ;
    rdfs:label "has as subject"@en ;
    rdfs:range lrmer:E1 ;
    rdfs:subPropertyOf lrmer:R1 ;
    owl:inverseOf lrmer:R12i ;
    skos:definition "Relates a work to its topic(s)"@en .

lrmer:R12i
    reg:lexicalAlias lrmer:isSubjectOf ;
    reg:name "isSubjectOf" ;
    reg:status <http://metadataregistry.org/uri/RegStatus/1001> ;
    a rdf:Property ;
    rdfs:comment "The logical connection between a work and a related subject entity serves as the basis both for identifying the subject of an individual work and for ensuring that all works relevant to a given subject are linked to that subject."@en ;
    rdfs:domain lrmer:E1 ;
    rdfs:isDefinedBy <http://iflastandards.info/ns/lrm/lrmer> ;
    rdfs:label "is subject of"@en ;
    rdfs:range lrmer:E2 ;
    rdfs:subPropertyOf lrmer:R1 ;
    owl:inverseOf lrmer:R12 ;
    skos:definition "Relates any res to a work in which that res is a topic"@en .

lrmer:R13
    reg:lexicalAlias lrmer:hasAppellation ;
    reg:name "hasAppellation" ;
    reg:status <http://metadataregistry.org/uri/RegStatus/1001> ;
    a rdf:Property ;
    rdfs:comment "The consequence of the definition of nomen as the association between something and a designation that refers to it, is that each nomen is uniquely associated with a single res within a given scheme (which can extend from a specific local system to a natural language, through a shared authority file). The resulting cardinality of the appellation relationship is that while a single res may have many nomens, each nomen is the appellation of a single res. The fact that two instances of nomen may have the same value for their nomen string attribute does not modify this cardinality, and does not imply that such instances of nomen are actually one and the same instance of nomen associated with more than one instance of res, even if the scheme in question is a natural language. The nomen string \"Gift\" may be used to refer either to a present or to a poison, according to whether it is the nomen string value for a nomen within the English language or for a nomen in the German language: although the string nomen values look the same, we do have here two distinct instances of nomen for two distinct instances of res. Although in theory, one instance of nomen (a subclass of res) could be associated to another instance of nomen via the appellation relationship (resulting in a nomen for another nomen), in practice the general case would not be provided for in implementations. Structurally, in a system implementation where instances of the entity nomen are assigned an internal identifier (also a nomen of a specific type) this relationship would be implicit in the system design. An example of this situation could be found in a linked data implementation which assigns a URI (nomen) to instances of nomen of other types."@en ;
    rdfs:domain lrmer:E1 ;
    rdfs:isDefinedBy <http://iflastandards.info/ns/lrm/lrmer> ;
    rdfs:label "has appellation"@en ;
    rdfs:range lrmer:E9 ;
    rdfs:subPropertyOf lrmer:R1 ;
    owl:inverseOf lrmer:R13i ;
    skos:definition "Relates an entity with a sign or combination of signs or symbols through which that entity is referred to within a given scheme or context"@en .

lrmer:R13i
    reg:lexicalAlias lrmer:isAppellationOf ;
    reg:name "isAppellationOf" ;
    reg:status <http://metadataregistry.org/uri/RegStatus/1001> ;
    a rdf:Property ;
    rdfs:comment "The consequence of the definition of nomen as the association between something and a designation that refers to it, is that each nomen is uniquely associated with a single res within a given scheme (which can extend from a specific local system to a natural language, through a shared authority file). The resulting cardinality of the appellation relationship is that while a single res may have many nomens, each nomen is the appellation of a single res. The fact that two instances of nomen may have the same value for their nomen string attribute does not modify this cardinality, and does not imply that such instances of nomen are actually one and the same instance of nomen associated with more than one instance of res, even if the scheme in question is a natural language. The nomen string \"Gift\" may be used to refer either to a present or to a poison, according to whether it is the nomen string value for a nomen within the English language or for a nomen in the German language: although the string nomen values look the same, we do have here two distinct instances of nomen for two distinct instances of res. Although in theory, one instance of nomen (a subclass of res) could be associated to another instance of nomen via the appellation relationship (resulting in a nomen for another nomen), in practice the general case would not be provided for in implementations. Structurally, in a system implementation where instances of the entity nomen are assigned an internal identifier (also a nomen of a specific type) this relationship would be implicit in the system design. An example of this situation could be found in a linked data implementation which assigns a URI (nomen) to instances of nomen of other types."@en ;
    rdfs:domain lrmer:E9 ;
    rdfs:isDefinedBy <http://iflastandards.info/ns/lrm/lrmer> ;
    rdfs:label "is appellation of"@en ;
    rdfs:range lrmer:E1 ;
    rdfs:subPropertyOf lrmer:R1 ;
    owl:inverseOf lrmer:R13 ;
    skos:definition "Relates a nomen with an entity referred through that sign or combination of signs or symbols within a given scheme or context"@en .

lrmer:R14
    reg:lexicalAlias lrmer:assigned ;
    reg:name "assigned" ;
    reg:status <http://metadataregistry.org/uri/RegStatus/1001> ;
    a rdf:Property ;
    rdfs:comment "In the bibliographic context, nomen assignment is applied to the creation of subject terms, controlled access points, identifiers, etc."@en ;
    rdfs:domain lrmer:E6 ;
    rdfs:isDefinedBy <http://iflastandards.info/ns/lrm/lrmer> ;
    rdfs:label "assigned"@en ;
    rdfs:range lrmer:E9 ;
    rdfs:subPropertyOf lrmer:R1 ;
    owl:inverseOf lrmer:R14i ;
    skos:definition "Relates an agent with a particular nomen that was assigned by this agent"@en .

lrmer:R14i
    reg:lexicalAlias lrmer:wasAssignedBy ;
    reg:name "wasAssignedBy" ;
    reg:status <http://metadataregistry.org/uri/RegStatus/1001> ;
    a rdf:Property ;
    rdfs:comment "In the bibliographic context, nomen assignment is applied to the creation of subject terms, controlled access points, identifiers, etc."@en ;
    rdfs:domain lrmer:E9 ;
    rdfs:isDefinedBy <http://iflastandards.info/ns/lrm/lrmer> ;
    rdfs:label "was assigned by"@en ;
    rdfs:range lrmer:E6 ;
    rdfs:subPropertyOf lrmer:R1 ;
    owl:inverseOf lrmer:R14 ;
    skos:definition "Relates a nomen to an agent that assigned that particular nomen"@en .

lrmer:R15
    reg:lexicalAlias lrmer:isEquivalentTo ;
    reg:name "isEquivalentTo" ;
    reg:status <http://metadataregistry.org/uri/RegStatus/1001> ;
    a rdf:Property ;
    rdfs:comment "This is a shortcut of a fully developed path: NOMEN1 is appellation of RES + RES has appellation NOMEN2. The nomens related by this relationship are functionally equivalent in meaning (assigned to the same res), but as they retain their own values in any attributes that are recorded for them, they are not interchangeable as far as usage is concerned. The equivalent nomens may differ as to crucial attributes such as scheme, language or context of use. This equivalence relationship relates instances of nomens, and not the values of the nomen string attributes for these nomens. Thus, even though it may seem counter-intuitive, two nomens that refer to different res, even if recorded with the same literal string, will not be equivalent."@en ;
    rdfs:domain lrmer:E9 ;
    rdfs:isDefinedBy <http://iflastandards.info/ns/lrm/lrmer> ;
    rdfs:label "is equivalent to"@en ;
    rdfs:range lrmer:E9 ;
    rdfs:subPropertyOf lrmer:R1 ;
    skos:definition "Relates two nomens which are appellations of the same res"@en .

lrmer:R16
    reg:lexicalAlias lrmer:hasPartNomen ;
    reg:name "hasPartNomen" ;
    reg:status <http://metadataregistry.org/uri/RegStatus/1001> ;
    a rdf:Property ;
    rdfs:comment "The whole-part relationship for nomens is essential in handling the attributes of components of nomens constructed using pre-existing nomens, as such attributes as language may differ between the parts of a compound nomen."@en ;
    rdfs:domain lrmer:E9 ;
    rdfs:isDefinedBy <http://iflastandards.info/ns/lrm/lrmer> ;
    rdfs:label "has part nomen"@en ;
    rdfs:range lrmer:E9 ;
    rdfs:subPropertyOf lrmer:R1 ;
    owl:inverseOf lrmer:R16i ;
    skos:definition "Relates a nomen that is constructed using another nomen as a component to that component"@en .

lrmer:R16i
    reg:lexicalAlias lrmer:isPartNomenOf ;
    reg:name "isPartNomenOf" ;
    reg:status <http://metadataregistry.org/uri/RegStatus/1001> ;
    a rdf:Property ;
    rdfs:comment "The whole-part relationship for nomens is essential in handling the attributes of components of nomens constructed using pre-existing nomens, as such attributes as language may differ between the parts of a compound nomen."@en ;
    rdfs:domain lrmer:E9 ;
    rdfs:isDefinedBy <http://iflastandards.info/ns/lrm/lrmer> ;
    rdfs:label "is part nomen of"@en ;
    rdfs:range lrmer:E9 ;
    rdfs:subPropertyOf lrmer:R1 ;
    owl:inverseOf lrmer:R16 ;
    skos:definition "Relates a nomen to another nomen constructed using that nomen as a component"@en .

lrmer:R17
    reg:lexicalAlias lrmer:isDerivationNomenOf ;
    reg:name "isDerivationNomenOf" ;
    reg:status <http://metadataregistry.org/uri/RegStatus/1001> ;
    a rdf:Property ;
    rdfs:comment "A nomen may be derived from another due to formal modifications in the notation used (such as transliteration) or cultural or linguistic conventions (creation of abbreviated or shortened or variant forms)."@en ;
    rdfs:domain lrmer:E9 ;
    rdfs:isDefinedBy <http://iflastandards.info/ns/lrm/lrmer> ;
    rdfs:label "is derivation nomen of"@en ;
    rdfs:range lrmer:E9 ;
    rdfs:subPropertyOf lrmer:R1 ;
    owl:inverseOf lrmer:R17i ;
    skos:definition "Relates a nomen with another nomen that was used as the basis for the first nomen, both of which are appellations of the same res"@en .

lrmer:R17i
    reg:lexicalAlias lrmer:hasDerivationNomen ;
    reg:name "hasDerivationNomen" ;
    reg:status <http://metadataregistry.org/uri/RegStatus/1001> ;
    a rdf:Property ;
    rdfs:comment "A nomen may be derived from another due to formal modifications in the notation used (such as transliteration) or cultural or linguistic conventions (creation of abbreviated or shortened or variant forms)."@en ;
    rdfs:domain lrmer:E9 ;
    rdfs:isDefinedBy <http://iflastandards.info/ns/lrm/lrmer> ;
    rdfs:label "has derivation nomen"@en ;
    rdfs:range lrmer:E9 ;
    rdfs:subPropertyOf lrmer:R1 ;
    owl:inverseOf lrmer:R17 ;
    skos:definition "Relates a nomen with another nomen for which the first nomen formed the basis, both of which are appellations of the same res"@en .

lrmer:R18
    reg:lexicalAlias lrmer:hasPartWork ;
    reg:name "hasPartWork" ;
    reg:status <http://metadataregistry.org/uri/RegStatus/1001> ;
    a rdf:Property ;
    rdfs:comment "This applies when the component-to-whole relationship is an inherent aspect of the works and holds for all the expressions and manifestations of the larger work and of its component works, whether the expression or manifestation comprises the full larger work or just one or more (but not all) of the component works. Examples include movements of concertos, poems within poetry cycles, multipart novels, triptychs."@en ;
    rdfs:domain lrmer:E2 ;
    rdfs:isDefinedBy <http://iflastandards.info/ns/lrm/lrmer> ;
    rdfs:label "has part work"@en ;
    rdfs:range lrmer:E2 ;
    rdfs:subPropertyOf lrmer:R1 ;
    owl:inverseOf lrmer:R18i ;
    skos:definition "Relates two works, where the content of the second is a component of the first"@en .

lrmer:R18i
    reg:lexicalAlias lrmer:isPartWorkOf ;
    reg:name "isPartWorkOf" ;
    reg:status <http://metadataregistry.org/uri/RegStatus/1001> ;
    a rdf:Property ;
    rdfs:comment "This applies when the component-to-whole relationship is an inherent aspect of the works and holds for all the expressions and manifestations of the larger work and of its component works, whether the expression or manifestation comprises the full larger work or just one or more (but not all) of the component works. Examples include movements of concertos, poems within poetry cycles, multipart novels, triptychs."@en ;
    rdfs:domain lrmer:E2 ;
    rdfs:isDefinedBy <http://iflastandards.info/ns/lrm/lrmer> ;
    rdfs:label "is part work of"@en ;
    rdfs:range lrmer:E2 ;
    rdfs:subPropertyOf lrmer:R1 ;
    owl:inverseOf lrmer:R18 ;
    skos:definition "Relates two works, where the content of the first is a component of the other"@en .

lrmer:R19
    reg:lexicalAlias lrmer:precedesWork ;
    reg:name "precedesWork" ;
    reg:status <http://metadataregistry.org/uri/RegStatus/1001> ;
    a rdf:Property ;
    rdfs:comment "The relationship is about a sequence of ideas and should not be confused with the time of creation of the respective works. As this relationship concerns the logical continuation of the content of the respective works, it does not apply to those serial works that transform over time (via major title changes, changes in media type, etc.) yet maintain a continuity in their form or numbering schemes. See the work-transformation relationship, LRM-R22, to express the relationship between one aggregating or serial work and another that modifies and continues it."@en ;
    rdfs:domain lrmer:E2 ;
    rdfs:isDefinedBy <http://iflastandards.info/ns/lrm/lrmer> ;
    rdfs:label "precedes work"@en ;
    rdfs:range lrmer:E2 ;
    rdfs:subPropertyOf lrmer:R1 ;
    owl:inverseOf lrmer:R19i ;
    skos:definition "Relates two works where the content of the second is a logical continuation of the first"@en .

lrmer:R19i
    reg:lexicalAlias lrmer:succeedsWork ;
    reg:name "succeedsWork" ;
    reg:status <http://metadataregistry.org/uri/RegStatus/1001> ;
    a rdf:Property ;
    rdfs:comment "The relationship is about a sequence of ideas and should not be confused with the time of creation of the respective works. As this relationship concerns the logical continuation of the content of the respective works, it does not apply to those serial works that transform over time (via major title changes, changes in media type, etc.) yet maintain a continuity in their form or numbering schemes. See the work-transformation relationship, LRM-R22, to express the relationship between one aggregating or serial work and another that modifies and continues it."@en ;
    rdfs:domain lrmer:E2 ;
    rdfs:isDefinedBy <http://iflastandards.info/ns/lrm/lrmer> ;
    rdfs:label "succeeds work"@en ;
    rdfs:range lrmer:E2 ;
    rdfs:subPropertyOf lrmer:R1 ;
    owl:inverseOf lrmer:R19 ;
    skos:definition "Relates two works where the content of the first is logically continued by the second"@en .

lrmer:R2
    reg:lexicalAlias lrmer:isRealizedThrough ;
    reg:name "isRealizedThrough" ;
    reg:status <http://metadataregistry.org/uri/RegStatus/1001> ;
    a rdf:Property ;
    rdfs:comment "The logical connection between work and expression, as reflected in the model through this relationship, serves as the basis both for identifying the work represented by an individual expression and for ensuring that all expressions of a work are linked to the work. Indirectly the relationships between a work and the various expressions of that work also serve to establish a “sibling” relationship between the various expressions of the work."@en ;
    rdfs:domain lrmer:E2 ;
    rdfs:isDefinedBy <http://iflastandards.info/ns/lrm/lrmer> ;
    rdfs:label "is realized through"@en ;
    rdfs:range lrmer:E3 ;
    rdfs:subPropertyOf lrmer:R1 ;
    owl:inverseOf lrmer:R2i ;
    skos:definition "Relates a work with any of the expressions which convey the same intellectual or artistic content"@en .

lrmer:R20
    reg:lexicalAlias lrmer:accompaniesOrComplements ;
    reg:name "accompaniesOrComplements" ;
    reg:status <http://metadataregistry.org/uri/RegStatus/1001> ;
    a rdf:Property ;
    rdfs:comment "The relationship between two works which are independent, but can also be used in conjunction with each other as complements or companions. The two works may be adding value to each other (in this case the relationship is symmetrical); in other cases one of the works is considered secondary."@en ;
    rdfs:domain lrmer:E2 ;
    rdfs:isDefinedBy <http://iflastandards.info/ns/lrm/lrmer> ;
    rdfs:label "accompanies or complements"@en ;
    rdfs:range lrmer:E2 ;
    rdfs:subPropertyOf lrmer:R1 ;
    owl:inverseOf lrmer:R20i ;
    skos:definition "Relates a work to another work that it accompanies or complements"@en ;
    skos:scopeNote "Source documentation has \"accompanies / complements\"; slash character replaced with \"or\" to improve clarity."@en .

lrmer:R20i
    reg:lexicalAlias lrmer:isAccompaniedOrComplementedBy ;
    reg:name "isAccompaniedOrComplementedBy" ;
    reg:status <http://metadataregistry.org/uri/RegStatus/1001> ;
    a rdf:Property ;
    rdfs:comment "The relationship between two works which are independent, but can also be used in conjunction with each other as complements or companions. The two works may be adding value to each other (in this case the relationship is symmetrical); in other cases one of the works is considered secondary."@en ;
    rdfs:domain lrmer:E2 ;
    rdfs:isDefinedBy <http://iflastandards.info/ns/lrm/lrmer> ;
    rdfs:label "is accompanied or complemented by"@en ;
    rdfs:range lrmer:E2 ;
    rdfs:subPropertyOf lrmer:R1 ;
    owl:inverseOf lrmer:R20 ;
    skos:definition "Relates a work to another work which is accompanied or complemented by the first work"@en ;
    skos:scopeNote "Source documentation has \"is accompanied / complemented by\"; slash character replaced with \"or\" to improve clarity."@en .

lrmer:R21
    reg:lexicalAlias lrmer:isInspirationFor ;
    reg:name "isInspirationFor" ;
    reg:status <http://metadataregistry.org/uri/RegStatus/1001> ;
    a rdf:Property ;
    rdfs:domain lrmer:E2 ;
    rdfs:isDefinedBy <http://iflastandards.info/ns/lrm/lrmer> ;
    rdfs:label "is inspiration for"@en ;
    rdfs:range lrmer:E2 ;
    rdfs:subPropertyOf lrmer:R1 ;
    owl:inverseOf lrmer:R21i ;
    skos:definition "Relates two works where the content of the first served as the source of ideas for the second"@en .

lrmer:R21i
    reg:lexicalAlias lrmer:isInspiredBy ;
    reg:name "isInspiredBy" ;
    reg:status <http://metadataregistry.org/uri/RegStatus/1001> ;
    a rdf:Property ;
    rdfs:domain lrmer:E2 ;
    rdfs:isDefinedBy <http://iflastandards.info/ns/lrm/lrmer> ;
    rdfs:label "is inspired by"@en ;
    rdfs:range lrmer:E2 ;
    rdfs:subPropertyOf lrmer:R1 ;
    owl:inverseOf lrmer:R21 ;
    skos:definition "Relates two works where the source of ideas for the second originated in the content of the first"@en .

lrmer:R22
    reg:lexicalAlias lrmer:isATransformationOf ;
    reg:name "isATransformationOf" ;
    reg:status <http://metadataregistry.org/uri/RegStatus/1001> ;
    a rdf:Property ;
    rdfs:comment "Some transformations may be considered as being only inspired by a previous work."@en ;
    rdfs:domain lrmer:E2 ;
    rdfs:isDefinedBy <http://iflastandards.info/ns/lrm/lrmer> ;
    rdfs:label "is a transformation of"@en ;
    rdfs:range lrmer:E2 ;
    rdfs:subPropertyOf lrmer:R1 ;
    owl:inverseOf lrmer:R22i ;
    skos:definition "Relates a work to a previous work from which it was created by changing the scope or editorial policy (as in a serial or aggregating work), the genre or literary form (dramatization, novelization), target audience (adaptation for children), or style (paraphrase, imitation, parody)"@en .

lrmer:R22i
    reg:lexicalAlias lrmer:wasTransformedInto ;
    reg:name "wasTransformedInto" ;
    reg:status <http://metadataregistry.org/uri/RegStatus/1001> ;
    a rdf:Property ;
    rdfs:comment "Some transformations may be considered as being only inspired by a previous work."@en ;
    rdfs:domain lrmer:E2 ;
    rdfs:isDefinedBy <http://iflastandards.info/ns/lrm/lrmer> ;
    rdfs:label "was transformed into"@en ;
    rdfs:range lrmer:E2 ;
    rdfs:subPropertyOf lrmer:R1 ;
    owl:inverseOf lrmer:R22 ;
    skos:definition "Relates a work to a new work created by changing the scope or editorial policy (as in a serial or aggregating work), the genre or literary form (dramatization, novelization), target audience (adaptation for children), or style (paraphrase, imitation, parody) of the previous work"@en .

lrmer:R23
    reg:lexicalAlias lrmer:hasPartExpression ;
    reg:name "hasPartExpression" ;
    reg:status <http://metadataregistry.org/uri/RegStatus/1001> ;
    a rdf:Property ;
    rdfs:comment "This applies when the component-to-whole relationship is an inherent aspect of the works and holds for all the expressions and manifestations of the larger work and of its component works, whether the expression or manifestation comprises the full larger work or just one or more (but not all) of the component works."@en ;
    rdfs:domain lrmer:E3 ;
    rdfs:isDefinedBy <http://iflastandards.info/ns/lrm/lrmer> ;
    rdfs:label "has part expression"@en ;
    rdfs:range lrmer:E3 ;
    rdfs:subPropertyOf lrmer:R1 ;
    owl:inverseOf lrmer:R23i ;
    skos:definition "Relates two expressions where the second is a component of the first"@en .

lrmer:R23i
    reg:lexicalAlias lrmer:isPartExpressionOf ;
    reg:name "isPartExpressionOf" ;
    reg:status <http://metadataregistry.org/uri/RegStatus/1001> ;
    a rdf:Property ;
    rdfs:comment "This applies when the component-to-whole relationship is an inherent aspect of the works and holds for all the expressions and manifestations of the larger work and of its component works, whether the expression or manifestation comprises the full larger work or just one or more (but not all) of the component works."@en ;
    rdfs:domain lrmer:E3 ;
    rdfs:isDefinedBy <http://iflastandards.info/ns/lrm/lrmer> ;
    rdfs:label "is part expression of"@en ;
    rdfs:range lrmer:E3 ;
    rdfs:subPropertyOf lrmer:R1 ;
    owl:inverseOf lrmer:R23 ;
    skos:definition "Relates two expressions where the first is a component of the other"@en .

lrmer:R24
    reg:lexicalAlias lrmer:isDerivationExpressionOf ;
    reg:name "isDerivationExpressionOf" ;
    reg:status <http://metadataregistry.org/uri/RegStatus/1001> ;
    a rdf:Property ;
    rdfs:comment "In many cases, the exact source of, for example, a translation, adaptation, revision, or arrangement is not known. If it is, it may be an interesting aspect for the end-user. The derivation relationship may be refined to provide more detailed information about the nature of the transformation."@en ;
    rdfs:domain lrmer:E3 ;
    rdfs:isDefinedBy <http://iflastandards.info/ns/lrm/lrmer> ;
    rdfs:label "is derivation expression of"@en ;
    rdfs:range lrmer:E3 ;
    rdfs:subPropertyOf lrmer:R1 ;
    owl:inverseOf lrmer:R24i ;
    skos:definition "Relates two expressions of the same work, where the second was used as the source for the other"@en .

lrmer:R24i
    reg:lexicalAlias lrmer:hasDerivationExpression ;
    reg:name "hasDerivationExpression" ;
    reg:status <http://metadataregistry.org/uri/RegStatus/1001> ;
    a rdf:Property ;
    rdfs:comment "In many cases, the exact source of, for example, a translation, adaptation, revision, or arrangement is not known. If it is, it may be an interesting aspect for the end-user. The derivation relationship may be refined to provide more detailed information about the nature of the transformation."@en ;
    rdfs:domain lrmer:E3 ;
    rdfs:isDefinedBy <http://iflastandards.info/ns/lrm/lrmer> ;
    rdfs:label "has derivation expression"@en ;
    rdfs:range lrmer:E3 ;
    rdfs:subPropertyOf lrmer:R1 ;
    owl:inverseOf lrmer:R24 ;
    skos:definition "Relates two expressions of the same work, where the first was used as the source for the other"@en .

lrmer:R25
    reg:lexicalAlias lrmer:wasAggregatedBy ;
    reg:name "wasAggregatedBy" ;
    reg:status <http://metadataregistry.org/uri/RegStatus/1001> ;
    a rdf:Property ;
    rdfs:comment "An aggregating expression will select multiple specific expressions of other works so that they can be embodied together in an aggregate manifestation. An expression may be chosen by multiple aggregating expressions. This is a shortcut of the relationships illustrated in Figure 5.8, the general model for aggregates. EXPRESSION1 is embodied in MANIFESTATION (aggregate) + MANIFESTATION (aggregate) embodies (aggregating) EXPRESSION. Unlike the whole-part relationship between expressions, the expressions selected to appear together in the aggregate manifestation do not become components of the aggregating expression. Furthermore, the relationship between these expressions is not an inherent feature of the works that these expressions realize, and thus is does not hold in other expressions of those works."@en ;
    rdfs:domain lrmer:E3 ;
    rdfs:isDefinedBy <http://iflastandards.info/ns/lrm/lrmer> ;
    rdfs:label "was aggregated by"@en ;
    rdfs:range lrmer:E3 ;
    rdfs:subPropertyOf lrmer:R1 ;
    owl:inverseOf lrmer:R25i ;
    skos:definition "Relates a specific expression of a work chosen as part of the plan of an aggregating expression to the aggregating expression"@en .

lrmer:R25i
    reg:lexicalAlias lrmer:aggregated ;
    reg:name "aggregated" ;
    reg:status <http://metadataregistry.org/uri/RegStatus/1001> ;
    a rdf:Property ;
    rdfs:comment "An aggregating expression will select multiple specific expressions of other works so that they can be embodied together in an aggregate manifestation. An expression may be chosen by multiple aggregating expressions. This is a shortcut of the relationships illustrated in Figure 5.8, the general model for aggregates. EXPRESSION1 is embodied in MANIFESTATION (aggregate) + MANIFESTATION (aggregate) embodies (aggregating) EXPRESSION. Unlike the whole-part relationship between expressions, the expressions selected to appear together in the aggregate manifestation do not become components of the aggregating expression. Furthermore, the relationship between these expressions is not an inherent feature of the works that these expressions realize, and thus is does not hold in other expressions of those works."@en ;
    rdfs:domain lrmer:E3 ;
    rdfs:isDefinedBy <http://iflastandards.info/ns/lrm/lrmer> ;
    rdfs:label "aggregated"@en ;
    rdfs:range lrmer:E3 ;
    rdfs:subPropertyOf lrmer:R1 ;
    owl:inverseOf lrmer:R25 ;
    skos:definition "Relates an aggregating expression to a specific expression of a work that was chosen as part of the plan of the aggregating expression"@en .

lrmer:R26
    reg:lexicalAlias lrmer:hasPartManifestation ;
    reg:name "hasPartManifestation" ;
    reg:status <http://metadataregistry.org/uri/RegStatus/1001> ;
    a rdf:Property ;
    rdfs:comment "In some cases the components of a manifestation are based on physical considerations relating to the carrier in which the manifestation is intended to be issued (for example, a recording is too long to fit on a single disc and is issued in a two-disc boxed set). An alternate manifestation on another carrier may not display the same components. However, in the case when the component-to-whole relationship is an inherent aspect of the works it holds for all the expressions and manifestations of the larger work and of its component works, whether the expression or manifestation comprises the full larger work or just one or more (but not all) of the component works."@en ;
    rdfs:domain lrmer:E4 ;
    rdfs:isDefinedBy <http://iflastandards.info/ns/lrm/lrmer> ;
    rdfs:label "has part manifestation"@en ;
    rdfs:range lrmer:E4 ;
    rdfs:subPropertyOf lrmer:R1 ;
    owl:inverseOf lrmer:R26i ;
    skos:definition "Relates two manifestations where the second is a component of the first"@en .

lrmer:R26i
    reg:lexicalAlias lrmer:isPartManifestationOf ;
    reg:name "isPartManifestationOf" ;
    reg:status <http://metadataregistry.org/uri/RegStatus/1001> ;
    a rdf:Property ;
    rdfs:comment "In some cases the components of a manifestation are based on physical considerations relating to the carrier in which the manifestation is intended to be issued (for example, a recording is too long to fit on a single disc and is issued in a two-disc boxed set). An alternate manifestation on another carrier may not display the same components. However, in the case when the component-to-whole relationship is an inherent aspect of the works it holds for all the expressions and manifestations of the larger work and of its component works, whether the expression or manifestation comprises the full larger work or just one or more (but not all) of the component works."@en ;
    rdfs:domain lrmer:E4 ;
    rdfs:isDefinedBy <http://iflastandards.info/ns/lrm/lrmer> ;
    rdfs:label "is part manifestation of"@en ;
    rdfs:range lrmer:E4 ;
    rdfs:subPropertyOf lrmer:R1 ;
    owl:inverseOf lrmer:R26 ;
    skos:definition "Relates two manifestations where the first is a component of the other"@en .

lrmer:R27
    reg:lexicalAlias lrmer:hasReproductionManifestation ;
    reg:name "hasReproductionManifestation" ;
    reg:status <http://metadataregistry.org/uri/RegStatus/1001> ;
    a rdf:Property ;
    rdfs:comment "Generally, for reprints and reissues no specific item of the source manifestation is singled out as the source of the reproduction. Furthermore, in these cases, although a particular item may have been used as a source of reproduction, this item should be considered to represent the source manifestation as a whole. The process of reproduction always results in a new manifestation, even when only a single item was produced from that manifestation."@en ;
    rdfs:domain lrmer:E4 ;
    rdfs:isDefinedBy <http://iflastandards.info/ns/lrm/lrmer> ;
    rdfs:label "has reproduction manifestation"@en ;
    rdfs:range lrmer:E4 ;
    rdfs:subPropertyOf lrmer:R1 ;
    owl:inverseOf lrmer:R27i ;
    skos:definition "Relates two manifestations providing the end-user with exactly the same content and where an earlier manifestation has provided a source for the creation of a subsequent manifestation, such as facsimiles, reproductions, reprints, and reissues"@en .

lrmer:R27i
    reg:lexicalAlias lrmer:isReproductionManifestationOf ;
    reg:name "isReproductionManifestationOf" ;
    reg:status <http://metadataregistry.org/uri/RegStatus/1001> ;
    a rdf:Property ;
    rdfs:comment "Generally, for reprints and reissues no specific item of the source manifestation is singled out as the source of the reproduction. Furthermore, in these cases, although a particular item may have been used as a source of reproduction, this item should be considered to represent the source manifestation as a whole. The process of reproduction always results in a new manifestation, even when only a single item was produced from that manifestation."@en ;
    rdfs:domain lrmer:E4 ;
    rdfs:isDefinedBy <http://iflastandards.info/ns/lrm/lrmer> ;
    rdfs:label "is reproduction manifestation of"@en ;
    rdfs:range lrmer:E4 ;
    rdfs:subPropertyOf lrmer:R1 ;
    owl:inverseOf lrmer:R27 ;
    skos:definition "Relates two manifestations providing the end-user with exactly the same content and where a subsequent manifestation was created using an earlier manifestation as a source, such as facsimiles, reproductions, reprints, and reissues"@en .

lrmer:R28
    reg:lexicalAlias lrmer:hasReproductionItem ;
    reg:name "hasReproductionItem" ;
    reg:status <http://metadataregistry.org/uri/RegStatus/1001> ;
    a rdf:Property ;
    rdfs:comment "In this case, the particular item used as a source of reproduction is significant, either by its provenance or due to item-specific characteristics such as annotations or ownership markings. The process of reproduction always results in a new manifestation, even when only a single item was produced from that manifestation."@en ;
    rdfs:domain lrmer:E5 ;
    rdfs:isDefinedBy <http://iflastandards.info/ns/lrm/lrmer> ;
    rdfs:label "has reproduction item"@en ;
    rdfs:range lrmer:E4 ;
    rdfs:subPropertyOf lrmer:R1 ;
    owl:inverseOf lrmer:R28i ;
    skos:definition "Relates an item of one manifestation and another manifestation providing the end-user with exactly the same content and where a specific item has provided a source for the creation of a subsequent manifestation"@en .

lrmer:R28i
    reg:lexicalAlias lrmer:isReproductionItemOf ;
    reg:name "isReproductionItemOf" ;
    reg:status <http://metadataregistry.org/uri/RegStatus/1001> ;
    a rdf:Property ;
    rdfs:comment "In this case, the particular item used as a source of reproduction is significant, either by its provenance or due to item-specific characteristics such as annotations or ownership markings. The process of reproduction always results in a new manifestation, even when only a single item was produced from that manifestation."@en ;
    rdfs:domain lrmer:E4 ;
    rdfs:isDefinedBy <http://iflastandards.info/ns/lrm/lrmer> ;
    rdfs:label "is reproduction item of"@en ;
    rdfs:range lrmer:E5 ;
    rdfs:subPropertyOf lrmer:R1 ;
    owl:inverseOf lrmer:R28 ;
    skos:definition "Relates a manifestation and a specific item of another manifestation which provided a source for the creation of the subsequent manifestation providing the end-user with exactly the same content"@en .

lrmer:R29
    reg:lexicalAlias lrmer:hasAlternate ;
    reg:name "hasAlternate" ;
    reg:status <http://metadataregistry.org/uri/RegStatus/1001> ;
    a rdf:Property ;
    rdfs:comment "Typical cases are when a publication, sound recording, video, etc., is issued in more than one format or when it is released simultaneously by different publishers in different countries."@en ;
    rdfs:domain lrmer:E4 ;
    rdfs:isDefinedBy <http://iflastandards.info/ns/lrm/lrmer> ;
    rdfs:label "has alternate"@en ;
    rdfs:range lrmer:E4 ;
    rdfs:subPropertyOf lrmer:R1 ;
    skos:definition "Relates manifestations that effectively serve as alternatives for each other"@en .

lrmer:R2i
    reg:lexicalAlias lrmer:realizes ;
    reg:name "realizes" ;
    reg:status <http://metadataregistry.org/uri/RegStatus/1001> ;
    a rdf:Property ;
    rdfs:comment "The logical connection between work and expression, as reflected in the model through this relationship, serves as the basis both for identifying the work represented by an individual expression and for ensuring that all expressions of a work are linked to the work. Indirectly the relationships between a work and the various expressions of that work also serve to establish a “sibling” relationship between the various expressions of the work."@en ;
    rdfs:domain lrmer:E3 ;
    rdfs:isDefinedBy <http://iflastandards.info/ns/lrm/lrmer> ;
    rdfs:label "realizes"@en ;
    rdfs:range lrmer:E2 ;
    rdfs:subPropertyOf lrmer:R1 ;
    owl:inverseOf lrmer:R2 ;
    skos:definition "Relates an expression with the work whose intellectual or artistic content it conveys"@en .

lrmer:R3
    reg:lexicalAlias lrmer:isEmbodiedIn ;
    reg:name "isEmbodiedIn" ;
    reg:status <http://metadataregistry.org/uri/RegStatus/1001> ;
    a rdf:Property ;
    rdfs:comment "A manifestation may embody one or more expressions and any expression may be embodied in one or more manifestations. This logical connection serves as the basis both for identifying the specific expression or expressions of a work or works embodied in an individual manifestation and for ensuring that all manifestations of the same expression are linked back to that expression."@en ;
    rdfs:domain lrmer:E3 ;
    rdfs:isDefinedBy <http://iflastandards.info/ns/lrm/lrmer> ;
    rdfs:label "is embodied in"@en ;
    rdfs:range lrmer:E4 ;
    rdfs:subPropertyOf lrmer:R1 ;
    owl:inverseOf lrmer:R3i ;
    skos:definition "Relates an expression with a manifestation in which the expression appears"@en .

lrmer:R30
    reg:lexicalAlias lrmer:isMemberOf ;
    reg:name "isMemberOf" ;
    reg:status <http://metadataregistry.org/uri/RegStatus/1001> ;
    a rdf:Property ;
    rdfs:comment "A person may explicitly join an organization or association. A person may implicitly become a member of a family by birth, adoption, marriage, etc. A collective agent may join another collective agent as a member."@en ;
    rdfs:domain lrmer:E6 ;
    rdfs:isDefinedBy <http://iflastandards.info/ns/lrm/lrmer> ;
    rdfs:label "is member of"@en ;
    rdfs:range lrmer:E8 ;
    rdfs:subPropertyOf lrmer:R1 ;
    owl:inverseOf lrmer:R30i ;
    skos:definition "Relates an agent and a collective agent that the agent joined as a member"@en .

lrmer:R30i
    reg:lexicalAlias lrmer:hasMember ;
    reg:name "hasMember" ;
    reg:status <http://metadataregistry.org/uri/RegStatus/1001> ;
    a rdf:Property ;
    rdfs:comment "A person may explicitly join an organization or association. A person may implicitly become a member of a family by birth, adoption, marriage, etc. A collective agent may join another collective agent as a member."@en ;
    rdfs:domain lrmer:E8 ;
    rdfs:isDefinedBy <http://iflastandards.info/ns/lrm/lrmer> ;
    rdfs:label "has member"@en ;
    rdfs:range lrmer:E6 ;
    rdfs:subPropertyOf lrmer:R1 ;
    owl:inverseOf lrmer:R30 ;
    skos:definition "Relates a collective agent to an agent that joined the collective agent as a member"@en .

lrmer:R31
    reg:lexicalAlias lrmer:hasPartCollectiveAgent ;
    reg:name "hasPartCollectiveAgent" ;
    reg:status <http://metadataregistry.org/uri/RegStatus/1001> ;
    a rdf:Property ;
    rdfs:comment "This is a relationship between two collective agents where one is a component of the other"@en ;
    rdfs:domain lrmer:E8 ;
    rdfs:isDefinedBy <http://iflastandards.info/ns/lrm/lrmer> ;
    rdfs:label "has part collective agent"@en ;
    rdfs:range lrmer:E8 ;
    rdfs:subPropertyOf lrmer:R1 ;
    owl:inverseOf lrmer:R31i ;
    skos:definition "Relates two collective agents where the second is a component of the first"@en .

lrmer:R31i
    reg:lexicalAlias lrmer:isPartCollectiveAgentOf ;
    reg:name "isPartCollectiveAgentOf" ;
    reg:status <http://metadataregistry.org/uri/RegStatus/1001> ;
    a rdf:Property ;
    rdfs:comment "This is a relationship between two collective agents where one is a component of the other"@en ;
    rdfs:domain lrmer:E8 ;
    rdfs:isDefinedBy <http://iflastandards.info/ns/lrm/lrmer> ;
    rdfs:label "is part collective agent of"@en ;
    rdfs:range lrmer:E8 ;
    rdfs:subPropertyOf lrmer:R1 ;
    owl:inverseOf lrmer:R31 ;
    skos:definition "Relates two collective agents where the first is a component of the other"@en .

lrmer:R32
    reg:lexicalAlias lrmer:precedesCollectiveAgent ;
    reg:name "precedesCollectiveAgent" ;
    reg:status <http://metadataregistry.org/uri/RegStatus/1001> ;
    a rdf:Property ;
    rdfs:comment "A single instance of this relationship can record a simple transformation of a single collective agent into a single successor. Multiple instances of this relationship can be used together to capture the more complex mergers and splits that can occur between and among collective agents."@en ;
    rdfs:domain lrmer:E8 ;
    rdfs:isDefinedBy <http://iflastandards.info/ns/lrm/lrmer> ;
    rdfs:label "precedes collective agent"@en ;
    rdfs:range lrmer:E8 ;
    rdfs:subPropertyOf lrmer:R1 ;
    owl:inverseOf lrmer:R32i ;
    skos:definition "Relates two collective agents where the first was transformed into the second"@en .

lrmer:R32i
    reg:lexicalAlias lrmer:succeedsCollectiveAgent ;
    reg:name "succeedsCollectiveAgent" ;
    reg:status <http://metadataregistry.org/uri/RegStatus/1001> ;
    a rdf:Property ;
    rdfs:comment "A single instance of this relationship can record a simple transformation of a single collective agent into a single successor. Multiple instances of this relationship can be used together to capture the more complex mergers and splits that can occur between and among collective agents."@en ;
    rdfs:domain lrmer:E8 ;
    rdfs:isDefinedBy <http://iflastandards.info/ns/lrm/lrmer> ;
    rdfs:label "succeeds collective agent"@en ;
    rdfs:range lrmer:E8 ;
    rdfs:subPropertyOf lrmer:R1 ;
    owl:inverseOf lrmer:R32 ;
    skos:definition "Relates two collective agents where the second came into being as a transformation of the first"@en .

lrmer:R33
    reg:lexicalAlias lrmer:hasAssociationWithPlace ;
    reg:name "hasAssociationWithPlace" ;
    reg:status <http://metadataregistry.org/uri/RegStatus/1001> ;
    a rdf:Property ;
    rdfs:comment "In most implementations this relationship would be refined to reflect the exact nature of the association, for example, place of work conception or creation, place of expression creation (e.g., place of musical performance), place of publication or manufacture, current or former location of an item, and location of an agent."@en ;
    rdfs:domain lrmer:E1 ;
    rdfs:isDefinedBy <http://iflastandards.info/ns/lrm/lrmer> ;
    rdfs:label "has association with place"@en ;
    rdfs:range lrmer:E10 ;
    rdfs:subPropertyOf lrmer:R1 ;
    owl:inverseOf lrmer:R33i ;
    skos:definition "Relates any entity with a given extent of space"@en .

lrmer:R33i
    reg:lexicalAlias lrmer:isAssociatedWithPlace ;
    reg:name "isAssociatedWithPlace" ;
    reg:status <http://metadataregistry.org/uri/RegStatus/1001> ;
    a rdf:Property ;
    rdfs:comment "In most implementations this relationship would be refined to reflect the exact nature of the association, for example, place of work conception or creation, place of expression creation (e.g., place of musical performance), place of publication or manufacture, current or former location of an item, and location of an agent."@en ;
    rdfs:domain lrmer:E10 ;
    rdfs:isDefinedBy <http://iflastandards.info/ns/lrm/lrmer> ;
    rdfs:label "is associated with place"@en ;
    rdfs:range lrmer:E1 ;
    rdfs:subPropertyOf lrmer:R1 ;
    owl:inverseOf lrmer:R33 ;
    skos:definition "Relates a place with any entity"@en .

lrmer:R34
    reg:lexicalAlias lrmer:hasPartPlace ;
    reg:name "hasPartPlace" ;
    reg:status <http://metadataregistry.org/uri/RegStatus/1001> ;
    a rdf:Property ;
    rdfs:comment "This is a relationship between two places where one is a component of the other"@en ;
    rdfs:domain lrmer:E10 ;
    rdfs:isDefinedBy <http://iflastandards.info/ns/lrm/lrmer> ;
    rdfs:label "has part place"@en ;
    rdfs:range lrmer:E10 ;
    rdfs:subPropertyOf lrmer:R1 ;
    owl:inverseOf lrmer:R34i ;
    skos:definition "Relates two places where the second is a component of the first"@en .

lrmer:R34i
    reg:lexicalAlias lrmer:isPartPlaceOf ;
    reg:name "isPartPlaceOf" ;
    reg:status <http://metadataregistry.org/uri/RegStatus/1001> ;
    a rdf:Property ;
    rdfs:comment "This is a relationship between two places where one is a component of the other"@en ;
    rdfs:domain lrmer:E10 ;
    rdfs:isDefinedBy <http://iflastandards.info/ns/lrm/lrmer> ;
    rdfs:label "is part place of"@en ;
    rdfs:range lrmer:E10 ;
    rdfs:subPropertyOf lrmer:R1 ;
    owl:inverseOf lrmer:R34 ;
    skos:definition "Relates two places where the first is a component of the other"@en .

lrmer:R35
    reg:lexicalAlias lrmer:HasAssociationWithTime-span ;
    reg:name "HasAssociationWithTime-span" ;
    reg:status <http://metadataregistry.org/uri/RegStatus/1001> ;
    a rdf:Property ;
    rdfs:comment "In most implementations this relationship would be refined to reflect the exact nature of the association, for example, time of work conception or creation, time of expression creation (e.g., date/time of musical performance), time of publication or manufacture, period of ownership of an item, date of birth of a person, time of validity of the nomen for a particular res."@en ;
    rdfs:domain lrmer:E1 ;
    rdfs:isDefinedBy <http://iflastandards.info/ns/lrm/lrmer> ;
    rdfs:label "has association with time-span"@en ;
    rdfs:range lrmer:E11 ;
    rdfs:subPropertyOf lrmer:R1 ;
    owl:inverseOf lrmer:R35i ;
    skos:definition "Relates any entity with a temporal extent"@en .

lrmer:R35i
    reg:lexicalAlias lrmer:IsAssociatedWithTime-span ;
    reg:name "IsAssociatedWithTime-span" ;
    reg:status <http://metadataregistry.org/uri/RegStatus/1001> ;
    a rdf:Property ;
    rdfs:comment "In most implementations this relationship would be refined to reflect the exact nature of the association, for example, time of work conception or creation, time of expression creation (e.g., date/time of musical performance), time of publication or manufacture, period of ownership of an item, date of birth of a person, time of validity of the nomen for a particular res."@en ;
    rdfs:domain lrmer:E11 ;
    rdfs:isDefinedBy <http://iflastandards.info/ns/lrm/lrmer> ;
    rdfs:label "is associated with time-span"@en ;
    rdfs:range lrmer:E1 ;
    rdfs:subPropertyOf lrmer:R1 ;
    owl:inverseOf lrmer:R35 ;
    skos:definition "Relates a time-span with any entity"@en .

lrmer:R36
    reg:lexicalAlias lrmer:hasPartTime-span ;
    reg:name "hasPartTime-span" ;
    reg:status <http://metadataregistry.org/uri/RegStatus/1001> ;
    a rdf:Property ;
    rdfs:comment "This is a relationship between two time-spans where one is a component of the other"@en ;
    rdfs:domain lrmer:E11 ;
    rdfs:isDefinedBy <http://iflastandards.info/ns/lrm/lrmer> ;
    rdfs:label "has part time-span"@en ;
    rdfs:range lrmer:E11 ;
    rdfs:subPropertyOf lrmer:R1 ;
    owl:inverseOf lrmer:R36i ;
    skos:definition "Relates two time-spans where the second is a component of the first"@en .

lrmer:R36i
    reg:lexicalAlias lrmer:IsPartTime-spanOf ;
    reg:name "IsPartTime-spanOf" ;
    reg:status <http://metadataregistry.org/uri/RegStatus/1001> ;
    a rdf:Property ;
    rdfs:comment "This is a relationship between two time-spans where one is a component of the other"@en ;
    rdfs:domain lrmer:E11 ;
    rdfs:isDefinedBy <http://iflastandards.info/ns/lrm/lrmer> ;
    rdfs:label "is part time-span of"@en ;
    rdfs:range lrmer:E11 ;
    rdfs:subPropertyOf lrmer:R1 ;
    owl:inverseOf lrmer:R36 ;
    skos:definition "Relates two time-spans where the first is a component of the other"@en .

lrmer:R3i
    reg:lexicalAlias lrmer:embodies ;
    reg:name "embodies" ;
    reg:status <http://metadataregistry.org/uri/RegStatus/1001> ;
    a rdf:Property ;
    rdfs:comment "A manifestation may embody one or more expressions and any expression may be embodied in one or more manifestations. This logical connection serves as the basis both for identifying the specific expression or expressions of a work or works embodied in an individual manifestation and for ensuring that all manifestations of the same expression are linked back to that expression."@en ;
    rdfs:domain lrmer:E4 ;
    rdfs:isDefinedBy <http://iflastandards.info/ns/lrm/lrmer> ;
    rdfs:label "embodies"@en ;
    rdfs:range lrmer:E3 ;
    rdfs:subPropertyOf lrmer:R1 ;
    owl:inverseOf lrmer:R3 ;
    skos:definition "Relates a manifestation with an expression which appears in the manifestation"@en .

lrmer:R4
    reg:lexicalAlias lrmer:isExemplifiedBy ;
    reg:name "isExemplifiedBy" ;
    reg:status <http://metadataregistry.org/uri/RegStatus/1001> ;
    a rdf:Property ;
    rdfs:comment "The logical connection serves as the basis both for identifying the manifestation exemplified by an individual item and for ensuring that all items of the same manifestation are linked to that manifestation. Indirectly the relationships between a manifestation and the various items exemplifying that manifestation also serve to establish a “sibling” relationship between the various items of a manifestation."@en ;
    rdfs:domain lrmer:E4 ;
    rdfs:isDefinedBy <http://iflastandards.info/ns/lrm/lrmer> ;
    rdfs:label "is exemplified by"@en ;
    rdfs:range lrmer:E5 ;
    rdfs:subPropertyOf lrmer:R1 ;
    owl:inverseOf lrmer:R4i ;
    skos:definition "Relates a manifestation with any item that reflects the characteristics of that manifestation"@en .

lrmer:R4i
    reg:lexicalAlias lrmer:exemplifies ;
    reg:name "exemplifies" ;
    reg:status <http://metadataregistry.org/uri/RegStatus/1001> ;
    a rdf:Property ;
    rdfs:comment "The logical connection serves as the basis both for identifying the manifestation exemplified by an individual item and for ensuring that all items of the same manifestation are linked to that manifestation. Indirectly the relationships between a manifestation and the various items exemplifying that manifestation also serve to establish a “sibling” relationship between the various items of a manifestation."@en ;
    rdfs:domain lrmer:E5 ;
    rdfs:isDefinedBy <http://iflastandards.info/ns/lrm/lrmer> ;
    rdfs:label "exemplifies"@en ;
    rdfs:range lrmer:E4 ;
    rdfs:subPropertyOf lrmer:R1 ;
    owl:inverseOf lrmer:R4 ;
    skos:definition "Relates an item with the manifestation whose characteristics are reflected in the item"@en .

lrmer:R5
    reg:lexicalAlias lrmer:wasCreatedByWork ;
    reg:name "wasCreatedByWork" ;
    reg:status <http://metadataregistry.org/uri/RegStatus/1001> ;
    a rdf:Property ;
    rdfs:comment "The logical connection between a work and a related agent serves as the basis both for identifying an agent responsible for an individual work and for ensuring that all works by a particular agent are linked to that agent."@en ;
    rdfs:domain lrmer:E2 ;
    rdfs:isDefinedBy <http://iflastandards.info/ns/lrm/lrmer> ;
    rdfs:label "was created by work"@en ;
    rdfs:range lrmer:E6 ;
    rdfs:subPropertyOf lrmer:R1 ;
    owl:inverseOf lrmer:R5i ;
    skos:definition "Relates a work to an agent responsible for the creation of the intellectual or artistic content"@en .

lrmer:R5i
    reg:lexicalAlias lrmer:createdWork ;
    reg:name "createdWork" ;
    reg:status <http://metadataregistry.org/uri/RegStatus/1001> ;
    a rdf:Property ;
    rdfs:comment "The logical connection between a work and a related agent serves as the basis both for identifying an agent responsible for an individual work and for ensuring that all works by a particular agent are linked to that agent."@en ;
    rdfs:domain lrmer:E6 ;
    rdfs:isDefinedBy <http://iflastandards.info/ns/lrm/lrmer> ;
    rdfs:label "created work"@en ;
    rdfs:range lrmer:E2 ;
    rdfs:subPropertyOf lrmer:R1 ;
    owl:inverseOf lrmer:R5 ;
    skos:definition "Relates an agent to a work for which the agent is responsible for the creation of intellectual or artistic content"@en .

lrmer:R6
    reg:lexicalAlias lrmer:wasCreatedByExpression ;
    reg:name "wasCreatedByExpression" ;
    reg:status <http://metadataregistry.org/uri/RegStatus/1001> ;
    a rdf:Property ;
    rdfs:comment "This relationship applies both to the creation of the original expression and any subsequent modifications such as translations, revisions and performances. An agent responsible for the intellectual or artistic content of a work is responsible for the conception of the work as an abstract entity; an agent responsible for the expression of the work is responsible for the specifics of the intellectual or artistic realization or execution of the expression. The logical connection between an expression and a related agent serves as the basis both for identifying an agent responsible for an individual expression and for ensuring that all expressions realized by an agent are linked to that agent."@en ;
    rdfs:domain lrmer:E3 ;
    rdfs:isDefinedBy <http://iflastandards.info/ns/lrm/lrmer> ;
    rdfs:label "was created by expression"@en ;
    rdfs:range lrmer:E6 ;
    rdfs:subPropertyOf lrmer:R1 ;
    owl:inverseOf lrmer:R6i ;
    skos:definition "Relates an expression to an agent responsible for the realization of a work"@en .

lrmer:R6i
    reg:lexicalAlias lrmer:createdExpression ;
    reg:name "createdExpression" ;
    reg:status <http://metadataregistry.org/uri/RegStatus/1001> ;
    a rdf:Property ;
    rdfs:comment "This relationship applies both to the creation of the original expression and any subsequent modifications such as translations, revisions and performances. An agent responsible for the intellectual or artistic content of a work is responsible for the conception of the work as an abstract entity; an agent responsible for the expression of the work is responsible for the specifics of the intellectual or artistic realization or execution of the expression. The logical connection between an expression and a related agent serves as the basis both for identifying an agent responsible for an individual expression and for ensuring that all expressions realized by an agent are linked to that agent."@en ;
    rdfs:domain lrmer:E6 ;
    rdfs:isDefinedBy <http://iflastandards.info/ns/lrm/lrmer> ;
    rdfs:label "created expression"@en ;
    rdfs:range lrmer:E3 ;
    rdfs:subPropertyOf lrmer:R1 ;
    owl:inverseOf lrmer:R6 ;
    skos:definition "Relates an agent to an expression in which the agent is responsible for the realization of a work"@en .

lrmer:R7
    reg:lexicalAlias lrmer:wasCreatedByManifestation ;
    reg:name "wasCreatedByManifestation" ;
    reg:status <http://metadataregistry.org/uri/RegStatus/1001> ;
    a rdf:Property ;
    rdfs:comment "For a manifestation, the notion of creation broadly includes the publication process for published manifestations. The logical connection between a manifestation and a related agent serves as the basis both for identifying an agent responsible for creating a manifestation and for ensuring that all manifestations created by an agent are linked to that agent."@en ;
    rdfs:domain lrmer:E4 ;
    rdfs:isDefinedBy <http://iflastandards.info/ns/lrm/lrmer> ;
    rdfs:label "was created by manifestation"@en ;
    rdfs:range lrmer:E6 ;
    rdfs:subPropertyOf lrmer:R1 ;
    owl:inverseOf lrmer:R7i ;
    skos:definition "Relates a manifestation to an agent responsible for creating the manifestation"@en .

lrmer:R7i
    reg:lexicalAlias lrmer:createdManifestation ;
    reg:name "createdManifestation" ;
    reg:status <http://metadataregistry.org/uri/RegStatus/1001> ;
    a rdf:Property ;
    rdfs:comment "For a manifestation, the notion of creation broadly includes the publication process for published manifestations. The logical connection between a manifestation and a related agent serves as the basis both for identifying an agent responsible for creating a manifestation and for ensuring that all manifestations created by an agent are linked to that agent."@en ;
    rdfs:domain lrmer:E6 ;
    rdfs:isDefinedBy <http://iflastandards.info/ns/lrm/lrmer> ;
    rdfs:label "created manifestation"@en ;
    rdfs:range lrmer:E4 ;
    rdfs:subPropertyOf lrmer:R1 ;
    owl:inverseOf lrmer:R7 ;
    skos:definition "Relates an agent to a manifestation that the agent is responsible for creating"@en .

lrmer:R8
    reg:lexicalAlias lrmer:wasManufacturedBy ;
    reg:name "wasManufacturedBy" ;
    reg:status <http://metadataregistry.org/uri/RegStatus/1001> ;
    a rdf:Property ;
    rdfs:comment "The manifestation may be manufactured or produced through industrial processes or through artisanal methods."@en ;
    rdfs:domain lrmer:E4 ;
    rdfs:isDefinedBy <http://iflastandards.info/ns/lrm/lrmer> ;
    rdfs:label "was manufactured by"@en ;
    rdfs:range lrmer:E6 ;
    rdfs:subPropertyOf lrmer:R1 ;
    owl:inverseOf lrmer:R8i ;
    skos:definition "Relates a manifestation to an agent responsible for the fabrication, production or manufacture of the items of that manifestation"@en .

lrmer:R8i
    reg:lexicalAlias lrmer:manufactured ;
    reg:name "manufactured" ;
    reg:status <http://metadataregistry.org/uri/RegStatus/1001> ;
    a rdf:Property ;
    rdfs:comment "The manifestation may be manufactured or produced through industrial processes or through artisanal methods."@en ;
    rdfs:domain lrmer:E6 ;
    rdfs:isDefinedBy <http://iflastandards.info/ns/lrm/lrmer> ;
    rdfs:label "manufactured"@en ;
    rdfs:range lrmer:E4 ;
    rdfs:subPropertyOf lrmer:R1 ;
    owl:inverseOf lrmer:R8 ;
    skos:definition "Relates an agent to a manifestation for which the agent is responsible for the fabrication, production or manufacture of items"@en .

lrmer:R9
    reg:lexicalAlias lrmer:isDistributedBy ;
    reg:name "isDistributedBy" ;
    reg:status <http://metadataregistry.org/uri/RegStatus/1001> ;
    a rdf:Property ;
    rdfs:comment "The items can be made available through the traditional distribution processes for physical items, or by making electronic items available for download, streaming, etc."@en ;
    rdfs:domain lrmer:E4 ;
    rdfs:isDefinedBy <http://iflastandards.info/ns/lrm/lrmer> ;
    rdfs:label "is distributed by"@en ;
    rdfs:range lrmer:E6 ;
    rdfs:subPropertyOf lrmer:R1 ;
    owl:inverseOf lrmer:R9i ;
    skos:definition "Relates a manifestation to an agent responsible for making items of that manifestation available"@en .

lrmer:R9i
    reg:lexicalAlias lrmer:distributes ;
    reg:name "distributes" ;
    reg:status <http://metadataregistry.org/uri/RegStatus/1001> ;
    a rdf:Property ;
    rdfs:comment "The items can be made available through the traditional distribution processes for physical items, or by making electronic items available for download, streaming, etc."@en ;
    rdfs:domain lrmer:E6 ;
    rdfs:isDefinedBy <http://iflastandards.info/ns/lrm/lrmer> ;
    rdfs:label "distributes"@en ;
    rdfs:range lrmer:E4 ;
    rdfs:subPropertyOf lrmer:R1 ;
    owl:inverseOf lrmer:R9 ;
    skos:definition "Relates an agent to a manifestation for which the agent is responsible for making items of that manifestation available"@en .

<http://metadataregistry.org/uri/RegStatus/1001>
    a skos:Concept ;
    skos:prefLabel "Published"@en .

